@prefix : <https://w3id.org/enigma#> .
@prefix owl: <http://www.w3.org/2002/07/owl#> .
@prefix rdf: <http://www.w3.org/1999/02/22-rdf-syntax-ns#> .
@prefix xml: <http://www.w3.org/XML/1998/namespace> .
@prefix xsd: <http://www.w3.org/2001/XMLSchema#> .
@prefix rdfs: <http://www.w3.org/2000/01/rdf-schema#> .
@base <https://w3id.org/enigma> .

<https://w3id.org/enigma> rdf:type owl:Ontology ;
                           owl:versionIRI <https://w3id.org/enigma/cohort/1.0.0> ;
                           <http://purl.org/dc/terms/contributor> "Agnes McMahon"^^xsd:string ,
                                                                  "Daniel Garijo"^^xsd:string ,
                                                                  "Yolanda Gil"^^xsd:string ;
                           <http://purl.org/dc/terms/creator> "MiHyun Jang"^^xsd:string ,
                                                              "Neda Jahanshad"^^xsd:string ,
                                                              "Ryan Espiritu"^^xsd:string ;
                           <http://purl.org/dc/terms/description> "An ontology to describe cohorts of patients participating in ENIGMA projects."@en ;
                           <http://purl.org/dc/terms/license> <http://creativecommons.org/licenses/by/2.0/> ;
                           <http://purl.org/dc/terms/title> "The Cohort Ontology"@en ;
                           <http://purl.org/vocab/vann/preferredNamespacePrefix> "enigma"^^xsd:string ;
                           <http://purl.org/vocab/vann/preferredNamespaceUri> : ;
                           owl:versionInfo "v1.0.0"^^xsd:string .

#################################################################
#    Annotation properties
#################################################################

###  http://purl.org/dc/terms/contributor
<http://purl.org/dc/terms/contributor> rdf:type owl:AnnotationProperty .


###  http://purl.org/dc/terms/creator
<http://purl.org/dc/terms/creator> rdf:type owl:AnnotationProperty .


###  http://purl.org/dc/terms/description
<http://purl.org/dc/terms/description> rdf:type owl:AnnotationProperty .


###  http://purl.org/dc/terms/license
<http://purl.org/dc/terms/license> rdf:type owl:AnnotationProperty .


###  http://purl.org/dc/terms/title
<http://purl.org/dc/terms/title> rdf:type owl:AnnotationProperty .


###  http://purl.org/vocab/vann/example
<http://purl.org/vocab/vann/example> rdf:type owl:AnnotationProperty .


###  http://purl.org/vocab/vann/preferredNamespacePrefix
<http://purl.org/vocab/vann/preferredNamespacePrefix> rdf:type owl:AnnotationProperty .


###  http://purl.org/vocab/vann/preferredNamespaceUri
<http://purl.org/vocab/vann/preferredNamespaceUri> rdf:type owl:AnnotationProperty .


###  http://www.linkedmodel.org/schema/vaem#rationale
<http://www.linkedmodel.org/schema/vaem#rationale> rdf:type owl:AnnotationProperty .


#################################################################
#    Datatypes
#################################################################

###  http://www.w3.org/2001/XMLSchema#gYear
xsd:gYear rdf:type rdfs:Datatype .


#################################################################
#    Object Properties
#################################################################

###  http://xmlns.com/foaf/0.1/homepage
<http://xmlns.com/foaf/0.1/homepage> rdf:type owl:ObjectProperty ;
                                     rdfs:comment "A homepage for some thing."^^xsd:string ;
                                     rdfs:isDefinedBy <http://xmlns.com/foaf/0.1/> .


###  https://w3id.org/enigma#didNotHaveFirstEpisodeOf
:didNotHaveFirstEpisodeOf rdf:type owl:ObjectProperty ;
                          rdfs:subPropertyOf :doesNotHavePersonalHistoryOf ;
                          rdfs:domain :CohortGroup ;
                          rdfs:range :Disorder ;
                          owl:propertyDisjointWith :hasFirstEpisodeOf ;
                          <http://purl.org/vocab/vann/example> "CohortGroup1 didNotHaveFirstEpisodeOf Psychosis --> CohortGroup1 excludes people who had a first episode of psychosis"@en ;
                          rdfs:comment "Describes which diseases the cohort group members did NOT have a first episode of"@en ;
                          rdfs:label "did not have first episode of"@en .


###  https://w3id.org/enigma#doesNotHaveCondition
:doesNotHaveCondition rdf:type owl:ObjectProperty ;
                      rdfs:domain :CohortGroup ;
                      rdfs:range :Condition ;
                      owl:propertyDisjointWith :hasCondition ;
                      <http://purl.org/vocab/vann/example> "Cohort1 doesNotHaveCondition euthymia"@en ;
                      rdfs:comment "Describes which disease conditions are excluded in a given cohort group"@en ;
                      rdfs:label "does not have condition"@en .


###  https://w3id.org/enigma#doesNotHaveDisorder
:doesNotHaveDisorder rdf:type owl:ObjectProperty ;
                     rdfs:domain :CohortGroup ;
                     rdfs:range :Disorder ;
                     owl:propertyDisjointWith :hasDisorder ;
                     <http://purl.org/vocab/vann/example> "CohortGroup1 doesNotHaveDisorder Cancer --> CohortGroup1 excludes people who have cancer"@en ;
                     rdfs:comment "Describes which disorders are excluded in a given cohort group"@en ;
                     rdfs:label "does not have disorder"@en .


###  https://w3id.org/enigma#doesNotHaveFamilyHistoryOf
:doesNotHaveFamilyHistoryOf rdf:type owl:ObjectProperty ;
                            rdfs:domain :CohortGroup ;
                            rdfs:range :Disorder ;
                            owl:propertyDisjointWith :hasFamilyHistoryOf ;
                            <http://purl.org/vocab/vann/example> "CohortGroup1 doesNotHaveFamilyHistoryOf Schizophrenia --> CohortGroup1 excludes people who have a family history of schizophrenia"@en ;
                            rdfs:comment "Describes which diseases the cohort group members do NOT have a family history of"@en ;
                            rdfs:label "does not family history of"@en .


###  https://w3id.org/enigma#doesNotHaveFirstDegreeRelativeWithDisorder
:doesNotHaveFirstDegreeRelativeWithDisorder rdf:type owl:ObjectProperty ;
                                            rdfs:subPropertyOf :doesNotHaveFamilyHistoryOf ;
                                            rdfs:domain :CohortGroup ;
                                            rdfs:range :Disorder ;
                                            owl:propertyDisjointWith :hasFirstDegreeRelativeWithDisorder ;
                                            <http://purl.org/vocab/vann/example> "CohortGroup1 doesNotHaveFirstDegreeRelativeWithDisorder BipolarDisorder --> CohortGroup1 excludes people who have a first degree relative with bipolar disorder"@en ;
                                            rdfs:comment "Describes which diseases the first degree relatives of cohort group members do NOT have"@en ;
                                            rdfs:label "does not first degree relative with disorder"@en .


###  https://w3id.org/enigma#doesNotHavePersonalHistoryOf
:doesNotHavePersonalHistoryOf rdf:type owl:ObjectProperty ;
                              rdfs:domain :CohortGroup ;
                              rdfs:range :Disorder ;
                              owl:propertyDisjointWith :hasPersonalHistoryOf ;
                              <http://purl.org/vocab/vann/example> "CohortGroup1 doesNotHaveHistoryOf NeurologicalDisease --> CohortGroup1 excludes people who have neurological disease"@en ;
                              rdfs:comment "Describes the diseases that the cohort group members do NOT have a history of"@en ;
                              rdfs:label "does not have personal history of"@en .


###  https://w3id.org/enigma#doesNotUseTreatment
:doesNotUseTreatment rdf:type owl:ObjectProperty ;
                     rdfs:domain :CohortGroup ;
                     rdfs:range :Treatment ;
                     owl:propertyDisjointWith :usesTreatment ;
                     <http://purl.org/vocab/vann/example> "CohortGroup1 doesNotUseTreatment Antidepressants --> CohortGroup1 excludes people who use antidepressants"@en ;
                     rdfs:comment "Describes which medications or therapies that the cohort group members are NOT using"@en ;
                     rdfs:label "does not use treatment"@en .


###  https://w3id.org/enigma#fulfillsDiagnosticCriteria
:fulfillsDiagnosticCriteria rdf:type owl:ObjectProperty ;
                            rdfs:domain :Disorder ;
                            rdfs:range :DiagnosticCriteria ;
                            <http://purl.org/vocab/vann/example> "bipolarDisorder fulfillsDiagnosticCriteria diagnosticAndStatisticalManualOfMentalDisorders --> The diagnosis of bipolar disorder fulfills the criteria of the DSM"@en ;
                            rdfs:comment "Describes the criteria used to diagnose the disorder"@en ;
                            rdfs:label "fulfills diagnostic criteria"@en .


###  https://w3id.org/enigma#hasBrainScanDataType
:hasBrainScanDataType rdf:type owl:ObjectProperty ;
                      rdfs:subPropertyOf :hasDataType ;
                      rdfs:domain [ rdf:type owl:Class ;
                                    owl:unionOf ( :Cohort
                                                  :Project
                                                )
                                  ] ;
                      rdfs:range :BrainScanDataType ;
                      <http://purl.org/vocab/vann/example> "Cohort1 hasBrainScanDataType MRI"@en ;
                      rdfs:comment "Describes the brain scan data types that were collected for a cohort or project"@en ;
                      rdfs:label "has brain scan data type"@en .


###  https://w3id.org/enigma#hasCondition
:hasCondition rdf:type owl:ObjectProperty ;
              rdfs:domain :CohortGroup ;
              rdfs:range :Condition ;
              <http://purl.org/vocab/vann/example> "Cohort1 hasCondition euthymia"@en ;
              rdfs:comment "Describes which diease conditions are included in a given cohort group"@en ;
              rdfs:label "has condition"@en .


###  https://w3id.org/enigma#hasContact
:hasContact rdf:type owl:ObjectProperty ;
            rdfs:domain [ rdf:type owl:Class ;
                          owl:unionOf ( :Cohort
                                        :Project
                                      )
                        ] ;
            rdfs:range :Person ;
            <http://purl.org/vocab/vann/example> "BipolarCohort hasContact JohnSmith"@en ;
            rdfs:comment "Property that points to the person that is a contact for the project or cohort"@en ;
            rdfs:label "has contact"@en .


###  https://w3id.org/enigma#hasControlGroup
:hasControlGroup rdf:type owl:ObjectProperty ;
                 rdfs:domain :Cohort ;
                 rdfs:range :CohortGroup ;
                 <http://purl.org/vocab/vann/example> "BipolarCohort hasControlGroup BipolarControlGroup"@en ;
                 rdfs:comment "Describes the control group of a cohort"@en ;
                 rdfs:label "has control group"@en .


###  https://w3id.org/enigma#hasDataType
:hasDataType rdf:type owl:ObjectProperty ;
             rdfs:domain [ rdf:type owl:Class ;
                           owl:unionOf ( :Cohort
                                         :Project
                                       )
                         ] ;
             rdfs:range :DataType ;
             <http://purl.org/vocab/vann/example> "Cohort1 hasDataType dataType1"@en ;
             rdfs:comment "Describes the data types that a cohort or project collected"@en ;
             rdfs:label "has data type"@en .


###  https://w3id.org/enigma#hasDiagnosisInstrument
:hasDiagnosisInstrument rdf:type owl:ObjectProperty ;
                        rdfs:domain :Cohort ;
                        rdfs:range :DiagnosisInstrument ;
                        <http://purl.org/vocab/vann/example> "Cohort1 hasDiagnosisInstrument miniInternationalNeuropychiatricInterview --> The members of Cohort1 are diagnosed with Mini International Neuropychiatric Interview"@en ;
                        rdfs:comment "Describes what instrument is used to diagnose the members of the cohort"@en ;
                        rdfs:label "has diagnosis instrument"@en .


###  https://w3id.org/enigma#hasDiagnosticGroup
:hasDiagnosticGroup rdf:type owl:ObjectProperty ;
                    rdfs:domain :Cohort ;
                    rdfs:range :CohortGroup ;
                    <http://purl.org/vocab/vann/example> "BipolarCohort hasPatientGroup BipolarPatientGroup"@en ;
                    rdfs:comment "Describes the patient group of a cohort"@en ;
                    rdfs:label "has diagnostic group"@en .


###  https://w3id.org/enigma#hasDisorder
:hasDisorder rdf:type owl:ObjectProperty ;
             rdfs:domain :CohortGroup ;
             rdfs:range :Disorder ;
             <http://purl.org/vocab/vann/example> "CohortGroup1 hasDisorder Cancer --> CohortGroup1 only includes people who have cancer"@en ;
             rdfs:comment "Describes what disease(s) the members of the cohort group have"@en ;
             rdfs:label "has disorder"@en .


###  https://w3id.org/enigma#hasDisorderDetails
:hasDisorderDetails rdf:type owl:ObjectProperty ;
                    rdfs:domain :CohortGroup ;
                    rdfs:range :SpecificDisorderInfo ;
                    <http://purl.org/vocab/vann/example> "CohortGroup1 hasDisorderDetails SZ20938"@en ;
                    rdfs:comment "Describes the details of a particular disorder that a cohort group has"@en ;
                    rdfs:label "has disorder details"@en .


###  https://w3id.org/enigma#hasFamilyHistoryOf
:hasFamilyHistoryOf rdf:type owl:ObjectProperty ;
                    rdfs:domain :CohortGroup ;
                    rdfs:range :Disorder ;
                    <http://purl.org/vocab/vann/example> "CohortGroup1 hasFamilyHistoryOf CardiovascularDisease --> CohortGroup1 only includes people who have a family history of cardiovascular diseases"@en ;
                    rdfs:comment "Describes what diseases the members of the cohort group have a family history of"@en ;
                    rdfs:label "has family history of"@en .


###  https://w3id.org/enigma#hasFirstDegreeRelativeWithDisorder
:hasFirstDegreeRelativeWithDisorder rdf:type owl:ObjectProperty ;
                                    rdfs:subPropertyOf :hasFamilyHistoryOf ;
                                    rdfs:domain :CohortGroup ;
                                    rdfs:range :Disorder ;
                                    <http://purl.org/vocab/vann/example> "CohortGroup1 hasFirstDegreeRelativeWithDisorder Psychosis --> CohortGroup1 only includes people who have a first degree relative with psychosis"@en ;
                                    rdfs:comment "Describes what diseases the first degree relatives of the members of the cohort group have"@en ;
                                    rdfs:label "has first degree relative with disorder"@en .


###  https://w3id.org/enigma#hasFirstEpisodeOf
:hasFirstEpisodeOf rdf:type owl:ObjectProperty ;
                   rdfs:subPropertyOf :hasPersonalHistoryOf ;
                   rdfs:domain :CohortGroup ;
                   rdfs:range :Disorder ;
                   <http://purl.org/vocab/vann/example> "CohortGroup1 hasFirstEpisodeOf Psychosis --> CohortGroup1 only includes people who had a first episode of psychosis"@en ;
                   rdfs:comment "Describes what disease the members of the cohort group had a first episode of"@en ;
                   rdfs:label "has first episode of"@en .


###  https://w3id.org/enigma#hasGeneticDataType
:hasGeneticDataType rdf:type owl:ObjectProperty ;
                    rdfs:subPropertyOf :hasDataType ;
                    rdfs:domain [ rdf:type owl:Class ;
                                  owl:unionOf ( :Cohort
                                                :Project
                                              )
                                ] ;
                    rdfs:range :GeneticDataType ;
                    <http://purl.org/vocab/vann/example> "Cohort1 hasGeneticDataType epigenetic"@en ;
                    rdfs:comment "Describes the genetic data types that were collected for a cohort or project"@en ;
                    rdfs:label "has genetic data type"@en .


###  https://w3id.org/enigma#hasHomePage
:hasHomePage rdf:type owl:ObjectProperty ;
             rdfs:subPropertyOf <http://xmlns.com/foaf/0.1/homepage> ;
             rdfs:domain [ rdf:type owl:Class ;
                           owl:unionOf ( :Cohort
                                         :Person
                                       )
                         ] ;
             rdfs:range owl:Thing ;
             <http://www.linkedmodel.org/schema/vaem#rationale> "Property added to facilitate interaction with domain and ranges in the wiki. It's equivalent to foaf:homePage"@en ;
             rdfs:comment "Property that describes the home page of a cohort or person"@en ;
             rdfs:label "has home page"@en .


###  https://w3id.org/enigma#hasImageAcquisitionProtocol
:hasImageAcquisitionProtocol rdf:type owl:ObjectProperty ;
                             rdfs:domain :Cohort ;
                             rdfs:range :ImageAcquisitionProtocol ;
                             <http://purl.org/vocab/vann/example> "Cohort1 hasImageAcquisitionProtocol AcquisitionProtocol1"@en ;
                             rdfs:comment "Describes the acquisition protocol that was used to scan the data of a cohort"@en ;
                             rdfs:label "has image acquisition protocol"@en .


###  https://w3id.org/enigma#hasInformationMethod
:hasInformationMethod rdf:type owl:ObjectProperty ;
                      rdfs:domain :Cohort ;
                      rdfs:range :InformationObtainmentMethod ;
                      <http://purl.org/vocab/vann/example> "Cohort1 hasInformationMethod selfReport --> The information of the members of Cohort1 was obtained through self report"@en ;
                      rdfs:comment "Describes the method for obtaining the medical information of a cohort"@en ;
                      rdfs:label "has information method"@en .


###  https://w3id.org/enigma#hasInvestigator
:hasInvestigator rdf:type owl:ObjectProperty ;
                 rdfs:domain :Cohort ;
                 rdfs:range :Person ;
                 <http://purl.org/vocab/vann/example> "BipolarCohort hasInvestigator JohnSmith"@en ;
                 rdfs:comment "Describe the investigators of a cohort"@en ;
                 rdfs:label "has investigator"@en .


###  https://w3id.org/enigma#hasMainPrincipalInvestigator
:hasMainPrincipalInvestigator rdf:type owl:ObjectProperty ;
                              rdfs:subPropertyOf :hasPrincipalInvestigator ;
                              rdfs:domain :Cohort ;
                              rdfs:range :Person ;
                              <http://purl.org/vocab/vann/example> "Cohort1 hasMainPrincipalInvestigatorof JohnSmith"@en ;
                              rdfs:comment "Describes which cohorts somone is a main PI of"@en ;
                              rdfs:label "has main principal investigator"@en .


###  https://w3id.org/enigma#hasMedicalRatingDetails
:hasMedicalRatingDetails rdf:type owl:ObjectProperty ;
                         rdfs:domain :CohortGroup ;
                         rdfs:range :SpecificMedicalRatingInfo ;
                         <http://purl.org/vocab/vann/example> "CohortDisorderGroup hasMedicalRatingDetails YMRS3010"@en ;
                         rdfs:comment "Describes the min and max values of the medical rating criteria"@en ;
                         rdfs:label "has medical rating details"@en .


###  https://w3id.org/enigma#hasMembersWithRecentIssue
:hasMembersWithRecentIssue rdf:type owl:ObjectProperty ;
                           rdfs:domain :Cohort ;
                           rdfs:range [ rdf:type owl:Class ;
                                        owl:unionOf ( :Condition
                                                      :Disorder
                                                      :Treatment
                                                    )
                                      ] ;
                           <http://purl.org/vocab/vann/example> "Cohort1TreatmentInfo usesTreatment Benzodiazepine inThePastMonths 6 --> Cohort1 only includes people who used benzodiazepine in the past6 months"@en ;
                           rdfs:comment "Describes whether or not the members of the cohort had an issue (condition, disorder, or treatment-related)  within the past few months"@en ;
                           rdfs:label "has members with recent issue"@en .


###  https://w3id.org/enigma#hasPersonalHistoryOf
:hasPersonalHistoryOf rdf:type owl:ObjectProperty ;
                      rdfs:domain :CohortGroup ;
                      rdfs:range :Disorder ;
                      <http://purl.org/vocab/vann/example> "CohortGroup1 hasHistoryOf NeurologicalDisease --> CohortGroup1 only includes people who have history of neurological disorders"@en ;
                      rdfs:comment "Describes the disease that the members of the cohort group have a history of"@en ;
                      rdfs:label "has personal history of"@en .


###  https://w3id.org/enigma#hasPopulationGroup
:hasPopulationGroup rdf:type owl:ObjectProperty ;
                    rdfs:domain :Cohort ;
                    rdfs:range :CohortGroup ;
                    <http://purl.org/vocab/vann/example> "BipolarCohort hasPopulationGroup USCPopulationGroup"@en ;
                    rdfs:comment "Describes the population group of a population-based cohort"@en ;
                    rdfs:label "has population group"@en .


###  https://w3id.org/enigma#hasPrincipalInvestigator
:hasPrincipalInvestigator rdf:type owl:ObjectProperty ;
                          rdfs:subPropertyOf :hasInvestigator ;
                          rdfs:domain :Cohort ;
                          rdfs:range :Person ;
                          <http://purl.org/vocab/vann/example> "Cohort1 hasPrincipalInvestigator John --> the principal investigator of Cohort1 is John"@en ;
                          rdfs:comment "Describes the principal investigator of the cohort"@en ;
                          rdfs:label "has principal investigator"@en .


###  https://w3id.org/enigma#hasProjectCohort
:hasProjectCohort rdf:type owl:ObjectProperty ;
                  rdfs:domain :Cohort ;
                  rdfs:range :ProjectCohort ;
                  <http://purl.org/vocab/vann/example> "BipolarCohort hasProjectCohort BipolarBarcelonaCohort"@en ;
                  rdfs:comment "Describes the subcohorts, specific to a given project, that are part of that cohort"@en ;
                  rdfs:label "has project cohort"@en .


###  https://w3id.org/enigma#hasTreatmentDetails
:hasTreatmentDetails rdf:type owl:ObjectProperty ;
                     rdfs:domain :CohortGroup ;
                     rdfs:range :SpecificTreatmentInfo ;
                     <http://purl.org/vocab/vann/example> "CohortGroup hasTreatmentDetails antidepressants42"@en ;
                     rdfs:comment "Describes the details of the treatment that a cohort group is using"@en ;
                     rdfs:label "has treatment details"@en .


###  https://w3id.org/enigma#usesGenotypePlatform
:usesGenotypePlatform rdf:type owl:ObjectProperty ;
                      rdfs:domain :Cohort ;
                      rdfs:range :GenotypePlatform ;
                      <http://purl.org/vocab/vann/example> "Cohort1 analyzedWithGenotypePlatform IllumniaOnmiExpress --> Illumina OnmiExpress was used to analyze cohort1"@en ;
                      rdfs:comment "Describes what genotype platform was used to analyze the members of the cohort"@en ;
                      rdfs:label "uses genotype platform"@en .


###  https://w3id.org/enigma#usesTreatment
:usesTreatment rdf:type owl:ObjectProperty ;
               rdfs:domain :CohortGroup ;
               rdfs:range :Treatment ;
               <http://purl.org/vocab/vann/example> "CohortGroup1 usesTreatment Antidepressants --> CohortGroup1 only includes people who currently use antidepressants"@en ;
               rdfs:comment "Describes which medications or therapies that the members of the cohort group are using"@en ;
               rdfs:label "uses treatment"@en .


#################################################################
#    Data properties
#################################################################

###  https://w3id.org/enigma#doesNotHaveComorbidity
:doesNotHaveComorbidity rdf:type owl:DatatypeProperty ;
                        rdfs:domain :CohortGroup ;
                        rdfs:range xsd:boolean ;
                        owl:propertyDisjointWith :hasComorbidity ;
                        <http://purl.org/vocab/vann/example> "CohortGroup1 doesNotHaveComorbidity true --> CohortGroup1 excludes people who are comorbid"@en ;
                        rdfs:comment "Describes if the members of a cohort group do not have a comorbidity"@en ;
                        rdfs:label "does not have comorbidity"@en .


###  https://w3id.org/enigma#doesNotHaveContraindicationToMRI
:doesNotHaveContraindicationToMRI rdf:type owl:DatatypeProperty ;
                                  rdfs:domain :CohortGroup ;
                                  rdfs:range xsd:boolean ;
                                  <http://purl.org/vocab/vann/example> "CohortGroup1 doesNotHaveContraindicationToMRI yes --> CohortGroup1 excludes people who do have contraindication to MRI"@en ;
                                  rdfs:comment "Describes if individuals who have contraindication to MRI are excluded"@en ;
                                  rdfs:label "does not have contraindiction to MRI"@en .


###  https://w3id.org/enigma#doesNotHaveIntellectualDisability
:doesNotHaveIntellectualDisability rdf:type owl:DatatypeProperty ;
                                   rdfs:domain :CohortGroup ;
                                   rdfs:range xsd:boolean ;
                                   <http://purl.org/vocab/vann/example> "Cohort1 doesNotHaveIntellectualDisability true"@en ;
                                   rdfs:comment "Describes whether a cohort excludes people with an intellectual disability"@en ;
                                   rdfs:label "does not have intellectual disability"@en .


###  https://w3id.org/enigma#doesNotHaveNeurologicalComorbidity
:doesNotHaveNeurologicalComorbidity rdf:type owl:DatatypeProperty ;
                                    rdfs:subPropertyOf :doesNotHaveComorbidity ;
                                    rdfs:domain :CohortGroup ;
                                    rdfs:range xsd:boolean ;
                                    owl:propertyDisjointWith :hasNeurologicalComorbidity ;
                                    <http://purl.org/vocab/vann/example> "CohortGroup1 doesNotHaveNeurologicalComorbidity true --> CohortGroup1 does not include people who have two or more neurological disorders"@en ;
                                    rdfs:comment "Describes if the members of a cohort group do not have a neurological comorbidity"@en ;
                                    rdfs:label "does not have neurological comorbidity"@en .


###  https://w3id.org/enigma#doesNotHavePsychiatricComorbidity
:doesNotHavePsychiatricComorbidity rdf:type owl:DatatypeProperty ;
                                   rdfs:subPropertyOf :doesNotHaveComorbidity ;
                                   rdfs:domain :CohortGroup ;
                                   rdfs:range xsd:boolean ;
                                   owl:propertyDisjointWith :hasPsychiatricComorbidity ;
                                   <http://purl.org/vocab/vann/example> "CohortGroup1 doesNotHavePsychiatricComorbidity true --> CohortGroup1 does not include people who have two or more psychiatric disorders"^^xsd:string ;
                                   rdfs:comment "Describes if the members of a cohort group do not have a psychiatric comorbidity"^^xsd:string ;
                                   rdfs:label "does not have psychiatric comorbidity"@en .


###  https://w3id.org/enigma#excludesLeftHands
:excludesLeftHands rdf:type owl:DatatypeProperty ;
                   rdfs:domain :CohortGroup ;
                   rdfs:range xsd:boolean ;
                   <http://purl.org/vocab/vann/example> "CohortGroup1 excludesLeftHanded true"@en ;
                   rdfs:comment "Describes if left handed people were excluded from the study"@en ;
                   rdfs:label "excludes left hands"@en .


###  https://w3id.org/enigma#excludesRightHands
:excludesRightHands rdf:type owl:DatatypeProperty ;
                    rdfs:domain :CohortGroup ;
                    rdfs:range xsd:boolean ;
                    <http://purl.org/vocab/vann/example> "CohortGroup1 excludesRightHands true"@en ;
                    rdfs:comment "Describes if right handed people were excluded from the study"@en ;
                    rdfs:label "excludes right hands"@en .


###  https://w3id.org/enigma#hasAdditionalDemographic
:hasAdditionalDemographic rdf:type owl:DatatypeProperty ;
                          rdfs:domain :CohortGroup ;
                          rdfs:range xsd:string ;
                          <http://purl.org/vocab/vann/example> "CohortGroup1 hasAdditionalDemographic \"handedness, IQ\""@en ;
                          rdfs:comment "Describes the additional demographics defining a given cohort group (Height; Weight; Ethnicity; IQ; ParentalSES; IndividualSES)"@en ;
                          rdfs:label "has additional demographic"@en .


###  https://w3id.org/enigma#hasAgeGroup
:hasAgeGroup rdf:type owl:DatatypeProperty ;
             rdfs:domain :CohortGroup ;
             rdfs:range xsd:string ;
             <http://purl.org/vocab/vann/example> "Cohort1 hasAgeGroup \"22-45\""@en ;
             rdfs:comment "Describes the age groupings of individuals within a cohort group"@en ;
             rdfs:label "has age group"@en .


###  https://w3id.org/enigma#hasAgeStandardDeviation
:hasAgeStandardDeviation rdf:type owl:DatatypeProperty ;
                         rdfs:domain :Cohort ;
                         rdfs:range xsd:double ;
                         <http://purl.org/vocab/vann/example> "Cohort1 hasAgeStandardDeviation 5.0"@en ;
                         rdfs:comment "Describes the standard deviation of the age of a cohort"@en ;
                         rdfs:label "has age standard deviation"@en .


###  https://w3id.org/enigma#hasBrainStructuralData
:hasBrainStructuralData rdf:type owl:DatatypeProperty ;
                        rdfs:domain :CohortGroup ;
                        rdfs:range xsd:string ;
                        <http://purl.org/vocab/vann/example> "CohortGroupSZ hasBrainStructuralData \"T1w, CT\""@en ;
                        rdfs:comment "Describes the types of brain structural/functional data collected by a cohort group (T1w; dMRI; T2w; SWI; rsfMRI; tbfMRI; ASL; EEG; MEG; Histology; CT; Head Circumference; Cognitive/Behavior assessments)"@en ;
                        rdfs:label "has brain structural data"@en .


###  https://w3id.org/enigma#hasBriefDescription
:hasBriefDescription rdf:type owl:DatatypeProperty ;
                     rdfs:domain [ rdf:type owl:Class ;
                                   owl:unionOf ( :Cohort
                                                 :Project
                                                 :WorkingGroup
                                               )
                                 ] ;
                     rdfs:range xsd:string ;
                     <http://purl.org/vocab/vann/example> "SZCohort hasBriefDescription \"finds correlations between schizophrenia and other conditions\""@en ;
                     rdfs:comment "Provides a brief description of the working group or project or cohort"@en ;
                     rdfs:label "has brief description"@en .


###  https://w3id.org/enigma#hasCohortStatus
:hasCohortStatus rdf:type owl:DatatypeProperty ;
                 rdfs:domain :Cohort ;
                 rdfs:range [ rdf:type rdfs:Datatype ;
                              owl:oneOf [ rdf:type rdf:List ;
                                          rdf:first "gathering participants"^^xsd:string ;
                                          rdf:rest [ rdf:type rdf:List ;
                                                     rdf:first "protocol preparation"^^xsd:string ;
                                                     rdf:rest [ rdf:type rdf:List ;
                                                                rdf:first "published"^^xsd:string ;
                                                                rdf:rest [ rdf:type rdf:List ;
                                                                           rdf:first "revision"^^xsd:string ;
                                                                           rdf:rest rdf:nil
                                                                         ]
                                                              ]
                                                   ]
                                        ]
                            ] ;
                 <http://purl.org/vocab/vann/example> "CohortGroup1 hasCohortStatus published"@en ;
                 rdfs:comment "Describes the current status of a cohort"@en ;
                 rdfs:label "has cohort status"@en .


###  https://w3id.org/enigma#hasCollectionSite
:hasCollectionSite rdf:type owl:DatatypeProperty ;
                   rdfs:domain :Cohort ;
                   rdfs:range xsd:string ;
                   <http://purl.org/vocab/vann/example> "Cohort1 hasCollectionSite Toronto"@en ;
                   rdfs:comment "Describes where the data of the cohort was collected"@en ;
                   rdfs:label "has collection site"@en .


###  https://w3id.org/enigma#hasComorbidity
:hasComorbidity rdf:type owl:DatatypeProperty ;
                rdfs:domain :CohortGroup ;
                rdfs:range xsd:boolean ;
                <http://purl.org/vocab/vann/example> "CohortGroup1 hasComorbidity true --> CohortGroup1 only includes people who are comorbid"@en ;
                rdfs:comment "Describes if the members of a cohort group have a comorbidity"@en ;
                rdfs:label "has comorbidity"@en .


###  https://w3id.org/enigma#hasDataCollectionPeriodEnd
:hasDataCollectionPeriodEnd rdf:type owl:DatatypeProperty ;
                            rdfs:domain :Cohort ;
                            rdfs:range xsd:gYear ;
                            <http://purl.org/vocab/vann/example> "Cohort1 hasDataCollectionPeriodEnd 2008"@en ;
                            rdfs:comment "Describes the end year of the data collection period of the cohort"@en ;
                            rdfs:label "has data collection period end"@en .


###  https://w3id.org/enigma#hasDataCollectionPeriodStart
:hasDataCollectionPeriodStart rdf:type owl:DatatypeProperty ;
                              rdfs:domain :Cohort ;
                              rdfs:range xsd:gYear ;
                              <http://purl.org/vocab/vann/example> "Cohort1 hasDataCollectionPeriodStart 2005"@en ;
                              rdfs:comment "Describes the start year of the data collection period of the cohort"@en ;
                              rdfs:label "has data collection period start"@en .


###  https://w3id.org/enigma#hasDiagnosisDisorder
:hasDiagnosisDisorder rdf:type owl:DatatypeProperty ;
                      rdfs:domain :CohortGroup ;
                      rdfs:range xsd:string ;
                      <http://purl.org/vocab/vann/example> "CohortGroup hasDiagnosisDisorder \"MDD, Bipolar Disorder\""@en ;
                      rdfs:comment """Describing the diagnosis disorder of a cohort group 

(MDD; Bipolar Disorder; Schizophrenia; OCD; ADHD; HIV; Autism; Addiction / SUD; Epilepsy; Anorexia / Eating Disorders; Parkinson; PTSD; Irritability; Stroke Recovery; Cerebellar Ataxia; Generalized anxiety; Panic disorder; Social anxiety; Early Onset Psychosis; Tourette's Syndrome; Brain Injury; Cancer & Chemotherapy; Sleep; Suicidal Thoughts and Behaviors; Lysosome Storage Diseases; 22q DS; CNVs)"""@en ;
                      rdfs:label "has diagnosis disorder"@en .


###  https://w3id.org/enigma#hasEthnicGroup
:hasEthnicGroup rdf:type owl:DatatypeProperty ;
                rdfs:domain :Cohort ;
                rdfs:range [ rdf:type rdfs:Datatype ;
                             owl:oneOf [ rdf:type rdf:List ;
                                         rdf:first "African American"^^xsd:string ;
                                         rdf:rest [ rdf:type rdf:List ;
                                                    rdf:first "Asian"^^xsd:string ;
                                                    rdf:rest [ rdf:type rdf:List ;
                                                               rdf:first "European"^^xsd:string ;
                                                               rdf:rest [ rdf:type rdf:List ;
                                                                          rdf:first "Latino"^^xsd:string ;
                                                                          rdf:rest [ rdf:type rdf:List ;
                                                                                     rdf:first "Two or More Races"^^xsd:string ;
                                                                                     rdf:rest rdf:nil
                                                                                   ]
                                                                        ]
                                                             ]
                                                  ]
                                       ]
                           ] ;
                <http://purl.org/vocab/vann/example> "Cohort1 hasEthnicGroup \"European\""@en ;
                rdfs:comment "Describes the ethnic group that the participants of the cohort are in"@en ;
                rdfs:label "has ethnic group"@en .


###  https://w3id.org/enigma#hasFamilialRelations
:hasFamilialRelations rdf:type owl:DatatypeProperty ;
                      rdfs:domain :Cohort ;
                      rdfs:range [ rdf:type rdfs:Datatype ;
                                   owl:oneOf [ rdf:type rdf:List ;
                                               rdf:first "No Relations"^^xsd:string ;
                                               rdf:rest [ rdf:type rdf:List ;
                                                          rdf:first "Pedigree"^^xsd:string ;
                                                          rdf:rest [ rdf:type rdf:List ;
                                                                     rdf:first "Siblings"^^xsd:string ;
                                                                     rdf:rest [ rdf:type rdf:List ;
                                                                                rdf:first "Singletons"^^xsd:string ;
                                                                                rdf:rest [ rdf:type rdf:List ;
                                                                                           rdf:first "Twins"^^xsd:string ;
                                                                                           rdf:rest rdf:nil
                                                                                         ]
                                                                              ]
                                                                   ]
                                                        ]
                                             ]
                                 ] ;
                      <http://purl.org/vocab/vann/example> "CohortA hasRelations \"Twins\""@en ;
                      rdfs:comment "Describes the relations between the individuals of a cohort"@en ;
                      rdfs:label "has familial relations"@en .


###  https://w3id.org/enigma#hasFundingSource
:hasFundingSource rdf:type owl:DatatypeProperty ;
                  rdfs:domain :Cohort ;
                  rdfs:range xsd:string ;
                  <http://purl.org/vocab/vann/example> "Cohort1 hasFundingSource \"NIMH, 5P50MH080272\""@en ;
                  rdfs:comment "Describes the funding source of the cohort"@en ;
                  rdfs:label "has funding source"@en .


###  https://w3id.org/enigma#hasHandedness
:hasHandedness rdf:type owl:DatatypeProperty ;
               rdfs:domain :CohortGroup ;
               rdfs:range xsd:string ;
               <http://purl.org/vocab/vann/example> "CohortGroup1 hasHandedness \"RH only\""@en ;
               rdfs:comment "Describes the handedness criteria for individuals in a cohort group (RH only; LH only; matched; assessed but not used as selection criteria; not assessed)"@en ;
               rdfs:label "has handedness"@en .


###  https://w3id.org/enigma#hasLongitudinalTimepoint
:hasLongitudinalTimepoint rdf:type owl:DatatypeProperty ;
                          rdfs:domain :Cohort ;
                          rdfs:range xsd:nonNegativeInteger ;
                          <http://purl.org/vocab/vann/example> "BipolarCorticolCohort hasLongitudinalTimepoint 3"@en ;
                          rdfs:comment "Describes the number of times a patient has been examined across time"@en ;
                          rdfs:label "has longitudinal timepoint"@en .


###  https://w3id.org/enigma#hasMaxAge
:hasMaxAge rdf:type owl:DatatypeProperty ;
           rdfs:domain :CohortGroup ;
           rdfs:range xsd:positiveInteger ;
           <http://purl.org/vocab/vann/example> "CohortGroup1 hasMaxAge 60"@en ;
           rdfs:comment "Describes inclusion criteria for maximum age of participants in a CohortGroup"@en ;
           rdfs:label "has max age"@en .


###  https://w3id.org/enigma#hasMaxIQ
:hasMaxIQ rdf:type owl:DatatypeProperty ;
          rdfs:domain :CohortGroup ;
          rdfs:range xsd:positiveInteger ;
          <http://purl.org/vocab/vann/example> "CohortGroup1 hasMaxIQ 120"@en ;
          rdfs:comment "Describes inclusion criteria for maximum IQ of participants in a CohortGroup"@en ;
          rdfs:label "has max IQ"@en .


###  https://w3id.org/enigma#hasMeanAge
:hasMeanAge rdf:type owl:DatatypeProperty ;
            rdfs:domain :Cohort ;
            rdfs:range xsd:double ;
            <http://purl.org/vocab/vann/example> "Cohort1 hasMeanAge 21.0"@en ;
            rdfs:comment "Describes the mean age of the cohort"@en ;
            rdfs:label "has mean age"@en .


###  https://w3id.org/enigma#hasMinAge
:hasMinAge rdf:type owl:DatatypeProperty ;
           rdfs:domain :CohortGroup ;
           rdfs:range xsd:positiveInteger ;
           <http://purl.org/vocab/vann/example> "CohortGroup1 hasMinAge 12"@en ;
           rdfs:comment "Describes inclusion criteria for minimum age of participants in a CohortGroup"@en ;
           rdfs:label "has min age"@en .


###  https://w3id.org/enigma#hasMinIQ
:hasMinIQ rdf:type owl:DatatypeProperty ;
          rdfs:domain :CohortGroup ;
          rdfs:range xsd:positiveInteger ;
          <http://purl.org/vocab/vann/example> "CohortGroup1 hasMinIQ 70"@en ;
          rdfs:comment "Describes inclusion criteria for minimum IQ of participants in a CohortGroup"@en ;
          rdfs:label "has min IQ"@en .


###  https://w3id.org/enigma#hasNeurologicalComorbidity
:hasNeurologicalComorbidity rdf:type owl:DatatypeProperty ;
                            rdfs:subPropertyOf :hasComorbidity ;
                            rdfs:domain :CohortGroup ;
                            rdfs:range xsd:boolean ;
                            <http://purl.org/vocab/vann/example> "CohortGroup1 hasNeurologicalComorbidity true --> CohortGroup1 only includes people who have two or more neurological disorders"@en ;
                            rdfs:comment "Describes if the members of a cohort group have a neurological comorbidity"@en ;
                            rdfs:label "has neurological comorbidity"@en .


###  https://w3id.org/enigma#hasNumberOfASL
:hasNumberOfASL rdf:type owl:DatatypeProperty ;
                rdfs:domain :ProjectCohort ;
                rdfs:range xsd:nonNegativeInteger ;
                <http://purl.org/vocab/vann/example> "ProjectCohortSZ hasNumberOfASL 21"@en ;
                rdfs:comment "Describes the amount of arterial spin labeling image data collected by a project cohort"@en ;
                rdfs:label "has number of ASL"@en .


###  https://w3id.org/enigma#hasNumberOfCisFemale
:hasNumberOfCisFemale rdf:type owl:DatatypeProperty ;
                      rdfs:domain :CohortGroup ;
                      rdfs:range xsd:nonNegativeInteger ;
                      <http://purl.org/vocab/vann/example> "CohortGroup1 hasNumberOfCisFemale 12"@en ;
                      rdfs:comment "Describes the number of cis female individuals in a cohort group"@en ;
                      rdfs:label "has number of cis female"@en .


###  https://w3id.org/enigma#hasNumberOfCisMale
:hasNumberOfCisMale rdf:type owl:DatatypeProperty ;
                    rdfs:domain :CohortGroup ;
                    rdfs:range xsd:nonNegativeInteger ;
                    <http://purl.org/vocab/vann/example> "CohortGroup1 hasNumberOfCisMale 12"@en ;
                    rdfs:comment "Describes the number of cis male individuals in a cohort group"@en ;
                    rdfs:label "has number of cis male"@en .


###  https://w3id.org/enigma#hasNumberOfEEG
:hasNumberOfEEG rdf:type owl:DatatypeProperty ;
                rdfs:domain :ProjectCohort ;
                rdfs:range xsd:nonNegativeInteger ;
                <http://purl.org/vocab/vann/example> "ProjectCohortSZ hasNumberOfEEG 30"@en ;
                rdfs:comment "Describes the amount of electroencephalography image data collected by a project cohort"@en ;
                rdfs:label "has number of EEG"@en .


###  https://w3id.org/enigma#hasNumberOfFemale
:hasNumberOfFemale rdf:type owl:DatatypeProperty ;
                   rdfs:domain :CohortGroup ;
                   rdfs:range xsd:nonNegativeInteger ;
                   <http://purl.org/vocab/vann/example> "CohortGroup1 hasNumberOfFemale 50"@en ;
                   rdfs:comment "Describes the number of females in a cohort group"@en ;
                   rdfs:label "has number of female"@en .


###  https://w3id.org/enigma#hasNumberOfMale
:hasNumberOfMale rdf:type owl:DatatypeProperty ;
                 rdfs:domain :CohortGroup ;
                 rdfs:range xsd:nonNegativeInteger ;
                 <http://purl.org/vocab/vann/example> "CohortGroup1 hasNumberOfMale 50"@en ;
                 rdfs:comment "Describes the number of males in the cohort group"@en ;
                 rdfs:label "has number of male"@en .


###  https://w3id.org/enigma#hasNumberOfParticipants
:hasNumberOfParticipants rdf:type owl:DatatypeProperty ;
                         rdfs:domain :Cohort ;
                         rdfs:range xsd:positiveInteger ;
                         <http://purl.org/vocab/vann/example> "Cohort1 hasNumberOfParticipants 500 --> Cohort1 is made up of approximately 500 patients"@en ;
                         rdfs:comment "Describes the number of participants in the cohort"@en ;
                         rdfs:label "has number of participants"@en .


###  https://w3id.org/enigma#hasNumberOfSWI
:hasNumberOfSWI rdf:type owl:DatatypeProperty ;
                rdfs:domain :ProjectCohort ;
                rdfs:range xsd:nonNegativeInteger ;
                <http://purl.org/vocab/vann/example> "ProjectCohortSZ hasNumberOfSWI 20"@en ;
                rdfs:comment "Describes the amount of susceptibility weighted imaging image data collected by a project cohort"@en ;
                rdfs:label "has number of SWI"@en .


###  https://w3id.org/enigma#hasNumberOfT1w
:hasNumberOfT1w rdf:type owl:DatatypeProperty ;
                rdfs:domain :ProjectCohort ;
                rdfs:range xsd:nonNegativeInteger ;
                <http://purl.org/vocab/vann/example> "ProjectCohortSZ hasNumberOfT1w 8"@en ;
                rdfs:comment "Describes the amount of T1-weighted image data collected by a project cohort"@en ;
                rdfs:label "has number of T1w"@en .


###  https://w3id.org/enigma#hasNumberOfT2
:hasNumberOfT2 rdf:type owl:DatatypeProperty ;
               rdfs:domain :ProjectCohort ;
               rdfs:range xsd:nonNegativeInteger ;
               <http://purl.org/vocab/vann/example> "ProjectCohortSZ hasNumberOfT2 10"@en ;
               rdfs:comment "Describes the amount of T2 image data  collected by a project cohort"@en ;
               rdfs:label "has number of T2"@en .


###  https://w3id.org/enigma#hasNumberOfTransgenderFtoM
:hasNumberOfTransgenderFtoM rdf:type owl:DatatypeProperty ;
                            rdfs:domain :CohortGroup ;
                            rdfs:range xsd:nonNegativeInteger ;
                            <http://purl.org/vocab/vann/example> "CohortGroup2 hasNumberOfTransgenderFtoM 14"@en ;
                            rdfs:comment "Describing the number of female to male transgender individuals in a cohort group"@en ;
                            rdfs:label "has number of transgender F to M"@en .


###  https://w3id.org/enigma#hasNumberOfTransgenderMtoF
:hasNumberOfTransgenderMtoF rdf:type owl:DatatypeProperty ;
                            rdfs:domain :CohortGroup ;
                            rdfs:range xsd:nonNegativeInteger ;
                            <http://purl.org/vocab/vann/example> "CohortGroup1 hasNumberOfTransgenderMtoF 20"@en ;
                            rdfs:comment "Describing the number of male to female transgender individuals in a cohort group"@en ;
                            rdfs:label "has number of transgender m to f"@en .


###  https://w3id.org/enigma#hasNumberOfUndisclosedGender
:hasNumberOfUndisclosedGender rdf:type owl:DatatypeProperty ;
                              rdfs:domain :CohortGroup ;
                              rdfs:range xsd:nonNegativeInteger ;
                              <http://purl.org/vocab/vann/example> "CohortGroup1 hasNumberOfUndisclosedGender 50"@en ;
                              rdfs:comment "Describing the number of individuals of undisclosed gender in a cohort group"@en ;
                              rdfs:label "has number of undisclosed gender"@en .


###  https://w3id.org/enigma#hasNumberOfdMRI
:hasNumberOfdMRI rdf:type owl:DatatypeProperty ;
                 rdfs:domain :ProjectCohort ;
                 rdfs:range xsd:nonNegativeInteger ;
                 <http://purl.org/vocab/vann/example> "ProjectCohortSZ hasNumberOfdMRI 10"@en ;
                 rdfs:comment "Describes the amount of diffusion MRI image data  collected by a project cohort"@en ;
                 rdfs:label "has number of dMRI"@en .


###  https://w3id.org/enigma#hasNumberOfrsfMRI
:hasNumberOfrsfMRI rdf:type owl:DatatypeProperty ;
                   rdfs:domain :ProjectCohort ;
                   rdfs:range xsd:nonNegativeInteger ;
                   <http://purl.org/vocab/vann/example> "ProjectCohortSZ hasNumberOfrsfMRI 17"@en ;
                   rdfs:comment "Describes the amount of resting state fMRI image data collected by a project cohort"@en ;
                   rdfs:label "has number of rsfMRI"@en .


###  https://w3id.org/enigma#hasNumberOftbfMRI
:hasNumberOftbfMRI rdf:type owl:DatatypeProperty ;
                   rdfs:domain :ProjectCohort ;
                   rdfs:range xsd:nonNegativeInteger ;
                   <http://purl.org/vocab/vann/example> "ProjectCohortSZ hasNumberOftbfMRI 17"@en ;
                   rdfs:comment "Describes the amount of total body fat measured on MRI image data collected by a project cohort"@en ;
                   rdfs:label "has number of tbfMRI"@en .


###  https://w3id.org/enigma#hasPercentBloodSalivaCollection
:hasPercentBloodSalivaCollection rdf:type owl:DatatypeProperty ;
                                 rdfs:domain :CohortGroup ;
                                 rdfs:range xsd:double ;
                                 <http://purl.org/vocab/vann/example> "CohortGroupSZ hasPercentBloodSalivaCollection 12.0"@en ;
                                 rdfs:comment "Describes the percent of cohort group biosamples which are from blood/saliva collected/stored with NO DNA extracted"@en ;
                                 rdfs:label "has percent blood saliva collection"@en .


###  https://w3id.org/enigma#hasPercentDNAExtractionNoGenotyping
:hasPercentDNAExtractionNoGenotyping rdf:type owl:DatatypeProperty ;
                                     rdfs:domain :CohortGroup ;
                                     rdfs:range xsd:double ;
                                     <http://purl.org/vocab/vann/example> "CohortGroupSZ hasPercentDNAExtractionNoGenotyping 30.0"@en ;
                                     rdfs:comment "Describes the percent of cohort group biosamples which are from DNA extraction with no genotyping"@en ;
                                     rdfs:label "has percent DNA extraction no genotyping"@en .


###  https://w3id.org/enigma#hasPercentEpigeneticsBlood
:hasPercentEpigeneticsBlood rdf:type owl:DatatypeProperty ;
                            rdfs:domain :CohortGroup ;
                            rdfs:range xsd:double ;
                            <http://purl.org/vocab/vann/example> "CohortGroupSZ hasPercentEpigeneticsBlood 23.0"@en ;
                            rdfs:comment "Describes the percent of cohort group biosamples which are from blood epigenetics"@en ;
                            rdfs:label "has percent epigenetics blood"@en .


###  https://w3id.org/enigma#hasPercentEpigeneticsSaliva
:hasPercentEpigeneticsSaliva rdf:type owl:DatatypeProperty ;
                             rdfs:domain :CohortGroup ;
                             rdfs:range xsd:double ;
                             <http://purl.org/vocab/vann/example> "CohortGroupSZ hasPercentEpigeneticsSaliva 23.0"@en ;
                             rdfs:comment "Describes the percent of cohort group biosamples which are from saliva epigenetics"@en ;
                             rdfs:label "has percent epigenetics saliva"@en .


###  https://w3id.org/enigma#hasPercentExomeSequencing
:hasPercentExomeSequencing rdf:type owl:DatatypeProperty ;
                           rdfs:domain :CohortGroup ;
                           rdfs:range xsd:double ;
                           <http://purl.org/vocab/vann/example> "CohortGroupSZ hasPercentExomeSequencing 75.0"@en ;
                           rdfs:comment "Describes the percent of cohort group biosamples which are from exome sequencing"@en ;
                           rdfs:label "has percent exome sequencing"@en .


###  https://w3id.org/enigma#hasPercentGeneExpression
:hasPercentGeneExpression rdf:type owl:DatatypeProperty ;
                          rdfs:domain :CohortGroup ;
                          rdfs:range xsd:double ;
                          <http://purl.org/vocab/vann/example> "CohortGroupSZ hasPercentGeneExpression 22.1"@en ;
                          rdfs:comment "Describes the percent of cohort group biosamples which are from gene expression"@en ;
                          rdfs:label "has percent gene expression"@en .


###  https://w3id.org/enigma#hasPercentGenomewideGenotyping
:hasPercentGenomewideGenotyping rdf:type owl:DatatypeProperty ;
                                rdfs:domain :CohortGroup ;
                                rdfs:range xsd:double ;
                                <http://purl.org/vocab/vann/example> "CohortGroupSZ hasPercentGenomewideGenotyping 55.5"@en ;
                                rdfs:comment "Describes the percent of cohort group biosamples which are from genome-wide genotyping"@en ;
                                rdfs:label "has percent genome-wide genotyping"@en .


###  https://w3id.org/enigma#hasPercentMitochondrialGenotyping
:hasPercentMitochondrialGenotyping rdf:type owl:DatatypeProperty ;
                                   rdfs:domain :CohortGroup ;
                                   rdfs:range xsd:double ;
                                   <http://purl.org/vocab/vann/example> "CohortGroupSZ hasPercentMitochondrialGenotyping 44.5"@en ;
                                   rdfs:comment "Describes the percent of cohort group biosamples which are from mitochondrial genotyping"@en ;
                                   rdfs:label "has percent mitochondrial genotyping"@en .


###  https://w3id.org/enigma#hasPercentPlasma
:hasPercentPlasma rdf:type owl:DatatypeProperty ;
                  rdfs:domain :CohortGroup ;
                  rdfs:range xsd:double ;
                  <http://purl.org/vocab/vann/example> "CohortGroupSZ hasPercentPlasma 11.0"@en ;
                  rdfs:comment "Describes the percent of cohort group biosamples which are from plasma"@en ;
                  rdfs:label "has percent plasma"@en .


###  https://w3id.org/enigma#hasPercentSelectLoci
:hasPercentSelectLoci rdf:type owl:DatatypeProperty ;
                      rdfs:domain :CohortGroup ;
                      rdfs:range xsd:double ;
                      <http://purl.org/vocab/vann/example> "CohortGroupSZ hasPercentSelectLoci 67.0"@en ;
                      rdfs:comment "Describes the percent of cohort group biosamples which are from select loci (some SNPs/CNVs)"@en ;
                      rdfs:label "has percent select loci"@en .


###  https://w3id.org/enigma#hasPercentTranscriptomics
:hasPercentTranscriptomics rdf:type owl:DatatypeProperty ;
                           rdfs:domain :CohortGroup ;
                           rdfs:range xsd:double ;
                           <http://purl.org/vocab/vann/example> "CohortGroupSZ hasPercentTranscriptomics 24.7"@en ;
                           rdfs:comment "Describes the percent of cohort group biosamples which are from transcriptomics"@en ;
                           rdfs:label "has percent transcriptomics"@en .


###  https://w3id.org/enigma#hasPercentWholeGenomeSequencing
:hasPercentWholeGenomeSequencing rdf:type owl:DatatypeProperty ;
                                 rdfs:domain :CohortGroup ;
                                 rdfs:range xsd:double ;
                                 <http://purl.org/vocab/vann/example> "CohortGroupSZ hasPercentWholeGenomeSequencing 60.0"@en ;
                                 rdfs:comment "Describes the percent of cohort group biosamples which are from whole genome sequencing"@en ;
                                 rdfs:label "has percent whole genome sequencing"@en .


###  https://w3id.org/enigma#hasPregnantMembers
:hasPregnantMembers rdf:type owl:DatatypeProperty ;
                    rdfs:domain :CohortGroup ;
                    rdfs:range xsd:boolean ;
                    <http://purl.org/vocab/vann/example> "CohortGroup1 hasPregnantMembers false"@en ;
                    rdfs:comment "Describes if the cohort has pregnant members"@en ;
                    rdfs:label "has pregnant members"@en .


###  https://w3id.org/enigma#hasPsychiatricComorbidity
:hasPsychiatricComorbidity rdf:type owl:DatatypeProperty ;
                           rdfs:subPropertyOf :hasComorbidity ;
                           rdfs:domain :CohortGroup ;
                           rdfs:range xsd:boolean ;
                           <http://purl.org/vocab/vann/example> "CohortGroup1 hasPsychiatricComorbidity true --> CohortGroup1 only includes people who have two or more pyschiatric disorders"@en ;
                           rdfs:comment "Describes if the members of a cohort group have a psychiatric comorbidity"@en ;
                           rdfs:label "has psychiatric comorbidity"@en .


###  https://w3id.org/enigma#hasSexDeterminedGenetically
:hasSexDeterminedGenetically rdf:type owl:DatatypeProperty ;
                             rdfs:domain :CohortGroup ;
                             rdfs:range xsd:boolean ;
                             <http://purl.org/vocab/vann/example> "Cohort1 sexDeterminedGenetically true"@en ;
                             rdfs:comment "Describes whether the genders of cohort group members were determined genetically"@en ;
                             rdfs:label "has sex determined genetically"@en .


###  https://w3id.org/enigma#hasSpecies
:hasSpecies rdf:type owl:DatatypeProperty ;
            rdfs:domain :Cohort ;
            rdfs:range xsd:string ;
            <http://purl.org/vocab/vann/example> "Cohort1 hasSpecies \"humans\""@en ;
            rdfs:comment "Describes the species of the subjects of a cohort (Humans, Chimps, Mice, etc.)"@en ;
            rdfs:label "has species"@en .


###  https://w3id.org/enigma#hasStudyDesign
:hasStudyDesign rdf:type owl:DatatypeProperty ;
                rdfs:domain [ rdf:type owl:Class ;
                              owl:unionOf ( :CohortGroup
                                            :Project
                                          )
                            ] ;
                rdfs:range xsd:string ;
                <http://purl.org/vocab/vann/example> "CohortGroup1 hasStudyDesign \"Population\""@en ;
                rdfs:comment """Describes the study design of the cohort group or project (Case/control; Population; Healthy only; Patients only)

NOTE: study design options are mutually exclusive for Cohort Groups but not Projects"""@en ;
                rdfs:label "has study design"@en .


###  https://w3id.org/enigma#hasStudyFeature
:hasStudyFeature rdf:type owl:DatatypeProperty ;
                 rdfs:domain :CohortGroup ;
                 rdfs:range xsd:string ;
                 <http://purl.org/vocab/vann/example> "CohortGroup1 hasStudyFeatures \"Clinical trial, Twin/Family study\""@en ;
                 rdfs:comment "Describes the study features of a cohort group (Clinical trial; Twin/Family study; Logitudinal; in-vivo; ex-vivo; post-mortem)"@en ;
                 rdfs:label "has study feature"@en .


###  https://w3id.org/enigma#includesFemale
:includesFemale rdf:type owl:DatatypeProperty ;
                rdfs:domain :Cohort ;
                rdfs:range xsd:boolean ;
                <http://purl.org/vocab/vann/example> "Cohort1 includesFemale true"@en ;
                rdfs:comment "Describes whether a cohort includes female participants"@en ;
                rdfs:label "includes female"@en .


###  https://w3id.org/enigma#includesMale
:includesMale rdf:type owl:DatatypeProperty ;
              rdfs:domain :Cohort ;
              rdfs:range xsd:boolean ;
              <http://purl.org/vocab/vann/example> "Cohort1 includesMale true"@en ;
              rdfs:comment "Describes whether a cohort includes male participants"@en ;
              rdfs:label "includes male"@en .


###  https://w3id.org/enigma#isClinicallyStable
:isClinicallyStable rdf:type owl:DatatypeProperty ;
                    rdfs:domain :Cohort ;
                    rdfs:range xsd:boolean ;
                    <http://purl.org/vocab/vann/example> "CohortGroup1 isClinicallyStable yes --> CohortGroup1 only includes people who are clinically stable"@en ;
                    rdfs:comment "Describes if the members of the cohort group are clinically stable (typically indicated by vital signs within 20% of usual readings)"@en ;
                    rdfs:label "is clinically stable"@en .


###  https://w3id.org/enigma#isFamilyBased
:isFamilyBased rdf:type owl:DatatypeProperty ;
               rdfs:domain :Cohort ;
               rdfs:range xsd:boolean ;
               <http://purl.org/vocab/vann/example> "Cohort1 isFamilyBased true"@en ;
               rdfs:comment "Describes if a cohort study was family based"@en ;
               rdfs:label "is family based"@en .


###  https://w3id.org/enigma#isProficientInLocalLanguage
:isProficientInLocalLanguage rdf:type owl:DatatypeProperty ;
                             rdfs:domain :Cohort ;
                             rdfs:range xsd:boolean ;
                             <http://purl.org/vocab/vann/example> "CohortGroup1 isProficientInLocalLanguage true"@en ;
                             rdfs:comment "Describes whether or not the members of the cohort group are proficient in local language"@en ;
                             rdfs:label "is proficient in local language"@en .


###  https://w3id.org/enigma#isPublic
:isPublic rdf:type owl:DatatypeProperty ;
          rdfs:domain :Cohort ;
          rdfs:range xsd:boolean ;
          <http://purl.org/vocab/vann/example> "SZCohort isPublic \"true\""@en ;
          rdfs:comment "Describes if a cohort's data is publicly available"@en ;
          rdfs:label "is public"@en .


###  https://w3id.org/enigma#usesScanner
:usesScanner rdf:type owl:DatatypeProperty ;
             rdfs:domain :Cohort ;
             rdfs:range xsd:string ;
             <http://purl.org/vocab/vann/example> "SZCohort usesScanner \"1.5T-GE-Signa\""@en ;
             rdfs:comment "Describes the scanner used by the cohort"@en ;
             rdfs:label "uses scanner"@en .


###  https://w3id.org/enigma#withDisorderSeverity
:withDisorderSeverity rdf:type owl:DatatypeProperty ;
                      rdfs:domain :SpecificDisorderInfo ;
                      rdfs:range xsd:positiveInteger ;
                      <http://purl.org/vocab/vann/example> """CohortGroup1 hasDisorderDetails Schizophrenia
Schizophrenia withDisorderSeverity 5

--> CohortGroup1 only includes people with schizophrenia with disease severity 5"""@en ;
                      rdfs:comment "Describes the severity of the disease"@en ;
                      rdfs:label "with disorder severity"@en .


###  https://w3id.org/enigma#withMaxAgeOfOnsetOfDisorder
:withMaxAgeOfOnsetOfDisorder rdf:type owl:DatatypeProperty ;
                             rdfs:domain :SpecificDisorderInfo ;
                             rdfs:range xsd:nonNegativeInteger ;
                             <http://purl.org/vocab/vann/example> """CohortGroup1 hasDisorderDetails Schizophrenia
Schizophrenia withMaxAgeOfOnsetOfDisorder 18

--> CohortGroup1 only includes people who had schizophrenia at 18 or younger"""@en ;
                             rdfs:comment "Describes the maximum age of onset of a disease"@en ;
                             rdfs:label "with max age of onset of disorder"@en .


###  https://w3id.org/enigma#withMaxDurationOfDisorder
:withMaxDurationOfDisorder rdf:type owl:DatatypeProperty ;
                           rdfs:domain :SpecificDisorderInfo ;
                           rdfs:range xsd:nonNegativeInteger ;
                           <http://purl.org/vocab/vann/example> """CohortGroup1 hasDisorderDetails Schizophrenia
Schizophrenia withMaxDurationOfDisorder 20

--> CohortGroup1 only includes people who had bipolar disorder for at most 20 years"""@en ;
                           rdfs:comment "Describes the maximum duration (in years) of a disease"@en ;
                           rdfs:label "with max duration of disorder"@en .


###  https://w3id.org/enigma#withMaxNumber
:withMaxNumber rdf:type owl:DatatypeProperty ;
               rdfs:domain :SpecificMedicalRatingInfo ;
               rdfs:range xsd:nonNegativeInteger ;
               <http://purl.org/vocab/vann/example> """CohortGroup1 hasMedicalRatingDetails YoungManiaRatingScale
YoungManiaRatingScale withMaxDurationOfDisorder 10

--> CohortGroup1 only includes people who received a score of at most 10 on the YMRS"""@en ;
               rdfs:comment "Describes the maximum medical rating score of individuals included in a cohort group"@en ;
               rdfs:label "with max number"@en .


###  https://w3id.org/enigma#withMinAgeOfOnsetOfDisorder
:withMinAgeOfOnsetOfDisorder rdf:type owl:DatatypeProperty ;
                             rdfs:domain :SpecificDisorderInfo ;
                             rdfs:range xsd:nonNegativeInteger ;
                             <http://purl.org/vocab/vann/example> """CohortGroup1 hasDisorderDetails Schizophrenia
Schizophrenia withMinAgeOfOnsetOfDisorder 10

--> CohortGroup1 only includes people who had schizophrenia at 10 or older"""@en ;
                             rdfs:comment "Describes the minimum age of onset of a disease"@en ;
                             rdfs:label "with min age of onset of disorder"@en .


###  https://w3id.org/enigma#withMinDurationOfDisorder
:withMinDurationOfDisorder rdf:type owl:DatatypeProperty ;
                           rdfs:domain :SpecificDisorderInfo ;
                           rdfs:range xsd:nonNegativeInteger ;
                           <http://purl.org/vocab/vann/example> """CohortGroup1 hasDisorderDetails Schizophrenia
Schizophrenia withMinDurationOfDisorder 10

--> CohortGroup1 only includes people had bipolar disorder for at least 10 years"""@en ;
                           rdfs:comment "Describes the minimum duration (in years) of a disease"@en ;
                           rdfs:label "with min duration of disorder"@en .


###  https://w3id.org/enigma#withMinNumber
:withMinNumber rdf:type owl:DatatypeProperty ;
               rdfs:domain :SpecificMedicalRatingInfo ;
               rdfs:range xsd:nonNegativeInteger ;
               <http://purl.org/vocab/vann/example> """CohortGroup1 hasMedicalRatingDetails YoungManiaRatingScale
YoungManiaRatingScale withMaxDurationOfDisorder 0

--> CohortGroup1 only includes people who scored at least a 0 on the YMRS"""@en ;
               rdfs:comment "Describes the minimum medical rating score of individuals included in a cohort group"@en ;
               rdfs:label "with min number"@en .


#################################################################
#    Classes
#################################################################

###  https://w3id.org/enigma#AnxietyDisorder
:AnxietyDisorder rdf:type owl:Class ;
                 rdfs:subClassOf :MentalHealthDisorder ;
                 <http://purl.org/vocab/vann/example> "PTSD"@en ;
                 rdfs:comment "A mental health disorder defined by feelings of anxiety, fear, or worry"@en ;
                 rdfs:label "Anxiety Disorder"@en .


###  https://w3id.org/enigma#BrainScanDataType
:BrainScanDataType rdf:type owl:Class ;
                   rdfs:subClassOf :DataType ;
                   <http://purl.org/vocab/vann/example> "EEG"@en ;
                   rdfs:comment "Specifies the kinds of brain scan data collected"@en ;
                   rdfs:label "Brain Scan Data Type"@en .


###  https://w3id.org/enigma#BriefPsychiatricRatingScale
:BriefPsychiatricRatingScale rdf:type owl:Class ;
                             rdfs:subClassOf :MedicalRating ;
                             rdfs:comment "Rating scale used to measure psychiatric symptoms among cohort members"@en ;
                             rdfs:label "Brief Psychiatric Rating Scale"@en .


###  https://w3id.org/enigma#Cancer
:Cancer rdf:type owl:Class ;
        rdfs:subClassOf :Disorder ;
        <http://purl.org/vocab/vann/example> "CNS Cancer"@en ;
        rdfs:comment "A disease characterized by abnormal cell division and growth"@en ;
        rdfs:label "Cancer"@en .


###  https://w3id.org/enigma#CardiovascularDisorder
:CardiovascularDisorder rdf:type owl:Class ;
                        rdfs:subClassOf :VascularDisorder ;
                        <http://purl.org/vocab/vann/example> "Coronary Artery Disease"@en ;
                        rdfs:comment "A subset of vascular disorders affecting the heart"@en ;
                        rdfs:label "Cardiovascular Disorder"@en .


###  https://w3id.org/enigma#CerebrovascularDisorder
:CerebrovascularDisorder rdf:type owl:Class ;
                         rdfs:subClassOf :VascularDisorder ;
                         <http://purl.org/vocab/vann/example> "Stroke"@en ;
                         rdfs:comment "A subset of vascular disorders affecting blood vessels of the brain and cerebral circulation"@en ;
                         rdfs:label "Cerebrovascular Disorder"@en .


###  https://w3id.org/enigma#City
:City rdf:type owl:Class ;
      rdfs:subClassOf :Location ;
      <http://purl.org/vocab/vann/example> "Los Angeles"@en ;
      rdfs:comment "City in which a cohort is located"@en ;
      rdfs:label "City"@en .


###  https://w3id.org/enigma#ClinicalGlobalImpressionsScale
:ClinicalGlobalImpressionsScale rdf:type owl:Class ;
                                rdfs:subClassOf :MedicalRating ;
                                rdfs:comment "Rating scale used to measure mental disorder symptom severity and treaments"@en ;
                                rdfs:label "Clinical Global Impression Scale"@en .


###  https://w3id.org/enigma#Cohort
:Cohort rdf:type owl:Class ;
        <http://purl.org/vocab/vann/example> "ADNI: Alzheimer’s Disease Neuroimaging Initiative"@en ;
        rdfs:comment "A group of individuals studied by a working group, limited by certain inclusion and exclusion criteria"@en ;
        rdfs:label "Cohort"@en .


###  https://w3id.org/enigma#CohortGroup
:CohortGroup rdf:type owl:Class ;
             rdfs:subClassOf :Cohort ;
             <http://purl.org/vocab/vann/example> "AMCControlGroup is a control cohort group of the AMC cohort"@en ;
             rdfs:comment "A subset of Cohort, which either forms the patient group or control group"@en ;
             rdfs:label "Cohort Group"@en .


###  https://w3id.org/enigma#Condition
:Condition rdf:type owl:Class ;
           <http://purl.org/vocab/vann/example> "Euthymia"@en ;
           rdfs:comment "A state or mood experienced by the members of a cohort"@en ;
           rdfs:label "Condition"@en .


###  https://w3id.org/enigma#Country
:Country rdf:type owl:Class ;
         rdfs:subClassOf :Location ;
         <http://purl.org/vocab/vann/example> "United States"@en ;
         rdfs:comment "Country in which a cohort is located"@en ;
         rdfs:label "Country"@en .


###  https://w3id.org/enigma#DataType
:DataType rdf:type owl:Class ;
          rdfs:comment "Specifies the kinds of data collected"@en ;
          rdfs:label "Data Type"@en .


###  https://w3id.org/enigma#DiagnosisInstrument
:DiagnosisInstrument rdf:type owl:Class ;
                     <http://purl.org/vocab/vann/example> "Consensus Consultant Diagnosis"@en ;
                     rdfs:comment "The method used to diagnosis individuals in a Cohort"@en ;
                     rdfs:label "Diagnosis Instrument"@en .


###  https://w3id.org/enigma#DiagnosticCriteria
:DiagnosticCriteria rdf:type owl:Class ;
                    <http://purl.org/vocab/vann/example> "DSM4"@en ;
                    rdfs:comment "The principles and standards used to diagnose a diease or condition"@en ;
                    rdfs:label "Diagnostic Criteria"@en .


###  https://w3id.org/enigma#Disorder
:Disorder rdf:type owl:Class ;
          rdfs:comment "A disorder/disease experienced by members of a cohort"@en ;
          rdfs:label "Disorder"@en .


###  https://w3id.org/enigma#EndocrineDisorder
:EndocrineDisorder rdf:type owl:Class ;
                   rdfs:subClassOf :Disorder ;
                   <http://purl.org/vocab/vann/example> "Hypothyroidism"@en ;
                   rdfs:comment "Disorders which affect the endocrine system"@en ;
                   rdfs:label "Endocrine Disorder"@en .


###  https://w3id.org/enigma#GeneticDataType
:GeneticDataType rdf:type owl:Class ;
                 rdfs:subClassOf :DataType ;
                 <http://purl.org/vocab/vann/example> "Epigenetic"@en ;
                 rdfs:comment "Specifies the kinds of genetic data collected"@en ;
                 rdfs:label "Genetic Data Type"@en .


###  https://w3id.org/enigma#GeneticDisorder
:GeneticDisorder rdf:type owl:Class ;
                 rdfs:subClassOf :Disorder ;
                 <http://purl.org/vocab/vann/example> "Cystic Fibrosis"@en ;
                 rdfs:comment "Disorders which are inherited and caused by abnormalities in the genome"@en ;
                 rdfs:label "Genetic Disorder"@en .


###  https://w3id.org/enigma#GenotypePlatform
:GenotypePlatform rdf:type owl:Class ;
                  <http://purl.org/vocab/vann/example> "IlluminaOmniExpress"@en ;
                  rdfs:comment "Software tools used for genotyping within a cohort"@en ;
                  rdfs:label "Genotype Platform"@en .


###  https://w3id.org/enigma#HamiltonDepressionRatingScale
:HamiltonDepressionRatingScale rdf:type owl:Class ;
                               rdfs:subClassOf :MedicalRating ;
                               rdfs:comment "Questionnaire used to measure the severity of depression"@en ;
                               rdfs:label "Hamilton Depression Rating Scale"@en .


###  https://w3id.org/enigma#ImageAcquisitionProtocol
:ImageAcquisitionProtocol rdf:type owl:Class ;
                          <http://purl.org/vocab/vann/example> "ENIGMA-Sulci"@en ;
                          rdfs:comment "Procedure used to collect image data within the cohort"@en ;
                          rdfs:label "Image Acquisition Protocol"@en .


###  https://w3id.org/enigma#InfectiousDisorder
:InfectiousDisorder rdf:type owl:Class ;
                    rdfs:subClassOf :Disorder ;
                    <http://purl.org/vocab/vann/example> "HIV"@en ;
                    rdfs:comment "A disease or disorder caused by the invasion of microorganisms"@en ;
                    rdfs:label "Infectious Disorder"@en .


###  https://w3id.org/enigma#InformationObtainmentMethod
:InformationObtainmentMethod rdf:type owl:Class ;
                             <http://purl.org/vocab/vann/example> "Hospital Records"@en ;
                             rdfs:comment "Method used to receive information about cohort subjects"@en ;
                             rdfs:label "Information Obtainment Method"@en .


###  https://w3id.org/enigma#Location
:Location rdf:type owl:Class ;
          <http://purl.org/vocab/vann/example> "Los Angeles, California"@en ;
          rdfs:comment "Geographic location of the cohort"@en ;
          rdfs:label "Location"@en .


###  https://w3id.org/enigma#MedicalRating
:MedicalRating rdf:type owl:Class ;
               <http://purl.org/vocab/vann/example> "ClincalGlobalImpressionsScale"@en ;
               rdfs:comment "Systems or scales used to measure the severity of a medical condition"@en ;
               rdfs:label "Medical Rating"@en .


###  https://w3id.org/enigma#MentalHealthDisorder
:MentalHealthDisorder rdf:type owl:Class ;
                      rdfs:subClassOf :Disorder ;
                      <http://purl.org/vocab/vann/example> "OCD"@en ;
                      rdfs:comment "Disorders which can affect mood, behavior, and thinking"@en ;
                      rdfs:label "Mental Health Disorder"@en .


###  https://w3id.org/enigma#MoodDisorder
:MoodDisorder rdf:type owl:Class ;
              rdfs:subClassOf :MentalHealthDisorder ;
              <http://purl.org/vocab/vann/example> "Bipolar Disorder"@en ;
              rdfs:comment "A mental health disorder defined by mood or behavioral swings"@en ;
              rdfs:label "Mood Disorder"@en .


###  https://w3id.org/enigma#NeurologicalDisorder
:NeurologicalDisorder rdf:type owl:Class ;
                      rdfs:subClassOf :Disorder ;
                      <http://purl.org/vocab/vann/example> "Epilepsy"@en ;
                      rdfs:comment "Disorders which affect the nervous system"@en ;
                      rdfs:label "Neurological Disorder"@en .


###  https://w3id.org/enigma#OrganicMedicalDisorder
:OrganicMedicalDisorder rdf:type owl:Class ;
                        rdfs:subClassOf :Disorder ;
                        <http://purl.org/vocab/vann/example> "Delirium"@en ;
                        rdfs:comment "Disorder characterized by decreased mental function due to a medical or physical disease"@en ;
                        rdfs:label "Organic Medical Disorder"@en .


###  https://w3id.org/enigma#Person
:Person rdf:type owl:Class ;
        <http://purl.org/vocab/vann/example> "Theo van Erp"@en ;
        rdfs:comment "Individual involved with the cohort"@en ;
        rdfs:label "Person"@en .


###  https://w3id.org/enigma#Project
:Project rdf:type owl:Class ;
         <http://purl.org/vocab/vann/example> "SZPositiveSymptoms"@en ;
         rdfs:comment "Project associated with the cohort"@en ;
         rdfs:label "Project"@en .


###  https://w3id.org/enigma#ProjectCohort
:ProjectCohort rdf:type owl:Class ;
               rdfs:subClassOf :Cohort ;
               <http://purl.org/vocab/vann/example> "\"Healthy\" individuals from the ASRB Cohort were sampled to form a Project Cohort of SZCorticol"@en ;
               rdfs:comment "The subset of the individuals from a Cohort, which are used as samples for a specific project"@en ;
               rdfs:label "Project Cohort"@en .


###  https://w3id.org/enigma#RespiratoryDisorder
:RespiratoryDisorder rdf:type owl:Class ;
                     rdfs:subClassOf :Disorder ;
                     <http://purl.org/vocab/vann/example> "Asthma"@en ;
                     rdfs:comment "Disorders which affect the respiratory system"@en ;
                     rdfs:label "Respiratory Disorder"@en .


###  https://w3id.org/enigma#SignificantGeneralMedicalCondition
:SignificantGeneralMedicalCondition rdf:type owl:Class ;
                                    rdfs:subClassOf :Disorder ;
                                    <http://purl.org/vocab/vann/example> "Cancer"@en ;
                                    rdfs:comment "Blanket term ecompassing serious medical condtions"@en ;
                                    rdfs:label "Significant General Medical Condition"@en .


###  https://w3id.org/enigma#SpecificConditionInfo
:SpecificConditionInfo rdf:type owl:Class ;
                       <http://purl.org/vocab/vann/example> "Severity of a condition"@en ;
                       rdfs:comment "Details unique to a given condition of the cohort"@en ;
                       rdfs:label "Specific Condition Info"@en .


###  https://w3id.org/enigma#SpecificDisorderInfo
:SpecificDisorderInfo rdf:type owl:Class ;
                      <http://purl.org/vocab/vann/example> "Severity of a disorder"@en ;
                      rdfs:comment "Details unique to a given disorder of the cohort"@en ;
                      rdfs:label "Specific Disorder Info"@en .


###  https://w3id.org/enigma#SpecificMedicalRatingInfo
:SpecificMedicalRatingInfo rdf:type owl:Class ;
                           <http://purl.org/vocab/vann/example> "Specifc scale used for medical rating"@en ;
                           rdfs:comment "Details unique to a given medical rating of the cohort"@en ;
                           rdfs:label "Specific Medical Rating Info"@en .


###  https://w3id.org/enigma#SpecificTreatmentInfo
:SpecificTreatmentInfo rdf:type owl:Class ;
                       <http://purl.org/vocab/vann/example> "The length of the treatment usage period"@en ;
                       rdfs:comment "Details of a specific treatment of the cohort"@en ;
                       rdfs:label "Specific Treatment Info"@en .


###  https://w3id.org/enigma#SubstanceAbuse
:SubstanceAbuse rdf:type owl:Class ;
                rdfs:subClassOf :MentalHealthDisorder ;
                <http://purl.org/vocab/vann/example> "Alcoholism"@en ;
                rdfs:comment "A mental health disorder defined by the overusage or abuse of a substance"@en ;
                rdfs:label "Substance Abuse"@en .


###  https://w3id.org/enigma#SubstanceDependence
:SubstanceDependence rdf:type owl:Class ;
                     rdfs:subClassOf :SubstanceAbuse ;
                     <http://purl.org/vocab/vann/example> "Alcohol Dependence"@en ;
                     rdfs:comment "A subset of substance abuse in which symptoms of withdrawal may appeared after reduction of substance use"@en ;
                     rdfs:label "Substance Dependence"@en .


###  https://w3id.org/enigma#Treatment
:Treatment rdf:type owl:Class ;
           <http://purl.org/vocab/vann/example> "Antidepressants"@en ;
           rdfs:comment "Treatments used on the members of the cohort"@en ;
           rdfs:label "Treatment"@en .


###  https://w3id.org/enigma#VascularDisorder
:VascularDisorder rdf:type owl:Class ;
                  rdfs:subClassOf :Disorder ;
                  <http://purl.org/vocab/vann/example> "Coronary Artery Disease"@en ;
                  rdfs:comment "Disorder which affects the body's network of blood vessels"@en ;
                  rdfs:label "Vascular Disorder"@en .


###  https://w3id.org/enigma#WorkingGroup
:WorkingGroup rdf:type owl:Class ;
              <http://purl.org/vocab/vann/example> "BipolarWG"@en ;
              rdfs:comment "Group of researchers studying a certain topic/disease"@en ;
              rdfs:label "Working Group"@en .


###  https://w3id.org/enigma#YoungManiaRatingScale
:YoungManiaRatingScale rdf:type owl:Class ;
                       rdfs:subClassOf :MedicalRating ;
                       rdfs:comment "Rating scale used to measure the severity of manic episodes in children and young adults"@en ;
                       rdfs:label "Young Mania Rating Scale"@en .


###  Generated by the OWL API (version 5.1.0) https://github.com/owlcs/owlapi/
