@prefix :        <https://w3id.org/enigma#> .
@prefix owl:     <http://www.w3.org/2002/07/owl#> .
@prefix rdf:     <http://www.w3.org/1999/02/22-rdf-syntax-ns#> .
@prefix xml:     <http://www.w3.org/XML/1998/namespace> .
@prefix xsd:     <http://www.w3.org/2001/XMLSchema#> .
@prefix rdfs:    <http://www.w3.org/2000/01/rdf-schema#> .

:isPartOfWorkingGroup
      a       owl:ObjectProperty ;
      rdfs:comment "Property that indicates the cohorts which are a part of a working group"@en ;
      rdfs:domain
              [ a       owl:Class ;
                owl:unionOf (:Cohort :CohortGroup :CohortProject)
              ] ;
      rdfs:domain
              [ a       owl:Class ;
                owl:unionOf (:Cohort :CohortGroup :CohortProject)
              ] ;
      rdfs:domain
              [ a       owl:Class ;
                owl:unionOf (:Cohort :CohortGroup :CohortProject)
              ] ;
      rdfs:domain
              [ a       owl:Class ;
                owl:unionOf (:Cohort :CohortGroup :CohortProject)
              ] ;
      rdfs:domain
              [ a       owl:Class ;
                owl:unionOf (:Cohort :CohortGroup :CohortProject)
              ] ;
      rdfs:label "is part of working group"@en ;
      rdfs:range :WorkingGroup .

:rationale
      a       owl:AnnotationProperty .

:OrthostaticHypertension
      a       owl:DatatypeProperty ;
      rdfs:comment "Orthostatic Hypertension: an increase in blood pressure upon assuming an upright position" ;
      rdfs:domain :Cardiovascular ;
      rdfs:label "Orthostatic Hypertension" ;
      rdfs:range xsd:boolean ;
      rdfs:subPropertyOf owl:topDataProperty .

:SASDQ
      a       owl:DatatypeProperty ;
      rdfs:comment "Sleep Apnea Scale of the Sleep Disorders Questionnaire" ;
      rdfs:domain :Neuropsychiatric ;
      rdfs:label "SASDQ" ;
      rdfs:range xsd:boolean ;
      rdfs:subPropertyOf owl:topDataProperty .

<http://www.linkedmodel.org/schema/vaem#rationale>
      a       owl:AnnotationProperty .

:hasWorkingGroupMember
      a       owl:ObjectProperty ;
      rdfs:comment "Describes who the members of the working group are"@en , "Describes what working group a person is a member of"@en ;
      rdfs:domain :WorkingGroup ;
      rdfs:label "has working group member"@en ;
      rdfs:range :Person ;
      rdfs:subPropertyOf <http://xmlns.com/foaf/0.1/member> ;
      <http://purl.org/vocab/vann/example>
              "BipolarWorkingGroup hasWorkingGroupMember JohnSmith"@en , "BipolarWorkingGroup hasWorkingGroupMember JohnSmith --> The bipolar working group has John Smith as a member"@en .

:MDS-UPDRSTotal
      a       owl:DatatypeProperty ;
      rdfs:comment "Movement Disorders Society Unified Parkinson's Disease Rating Scale - Total Score" ;
      rdfs:domain :PDDemographics ;
      rdfs:label "MDS-UPDRS Total" ;
      rdfs:range xsd:boolean .

:hasExclusionCriteria
      a       owl:DatatypeProperty ;
      rdfs:comment "Criteria used to exclude cohort patients"@en ;
      rdfs:domain
              [ a       owl:Class ;
                owl:unionOf (:Cohort :CohortGroup :CohortProject)
              ] ;
      rdfs:label "has exclusion criteria"@en ;
      rdfs:range xsd:string .

:VerbalOrLexicalFluencyTest
      a       owl:DatatypeProperty ;
      rdfs:comment "Verbal fluency tests assess an individual's ability to generate words from a specified letter of the alphabet (e.g. F, A and S) or a semantic category (e.g. animals and fruits)." ;
      rdfs:domain :Cognitive ;
      rdfs:label "Verbal Or Lexical Fluency Test" ;
      rdfs:range xsd:boolean ;
      rdfs:subPropertyOf owl:topDataProperty .

:RespiratoryDisorder
      a       owl:Class ;
      rdfs:comment "Disorders which affect the respiratory system"@en ;
      rdfs:label "Respiratory Disorder"@en ;
      rdfs:subClassOf :Disorder ;
      <http://purl.org/vocab/vann/example>
              "Asthma"@en .

<http://xmlns.com/foaf/0.1/Person>
      a       owl:Class ;
      rdfs:isDefinedBy "http://xmlns.com/foaf/0.1/"@en ;
      owl:equivalentClass :Person .

:Diabetes
      a       owl:DatatypeProperty ;
      rdfs:domain :Cardiovascular ;
      rdfs:label "Diabetes" ;
      rdfs:range xsd:boolean ;
      rdfs:subPropertyOf owl:topDataProperty .

:PDDemographics
      a       owl:Class ;
      rdfs:comment "PD-specific demographic Covariates measured by each cohort" ;
      rdfs:label "PD Demographics" .

:RBDDiagnosis
      a       owl:DatatypeProperty ;
      rdfs:comment "RBD (REM Sleep Behavior Disorder) Diagnosis" ;
      rdfs:domain :PDDemographics ;
      rdfs:label "RBD Diagnosis" ;
      rdfs:range xsd:boolean .

:cityDwelling
      a       owl:DatatypeProperty ;
      rdfs:comment "If measured subjects in the cohort were city dwelling (pop >100,000)" ;
      rdfs:domain :PDDemographics ;
      rdfs:label "City-Dwelling" ;
      rdfs:range xsd:boolean .

:usesScanner
      a       owl:DatatypeProperty ;
      rdfs:comment "Describes the scanner used by the cohort"@en ;
      rdfs:domain
              [ a       owl:Class ;
                owl:unionOf (:Cohort :CohortGroup :CohortProject)
              ] ;
      rdfs:label "uses scanner"@en ;
      rdfs:range xsd:string ;
      <http://purl.org/vocab/vann/example>
              "SZCohort usesScanner \"1.5T-GE-Signa\""@en .

:UPDRS-1
      a       owl:DatatypeProperty ;
      rdfs:comment "Unified Parkinson's Disease Rating Scale - 1" ;
      rdfs:domain :PDDemographics ;
      rdfs:label "UPDRS-1" ;
      rdfs:range xsd:boolean .

<https://schema.org/name>
      a       owl:DatatypeProperty ;
      rdfs:isDefinedBy <https://schema.org> .

:Other_Depression_Severity_Total_Score
      a       owl:DatatypeProperty ;
      rdfs:comment "Total scores for other depression severity scales" ;
      rdfs:domain :Neuropsychiatric ;
      rdfs:label "Other Depression Severity Total Score" ;
      rdfs:range xsd:boolean .

:hasWorkingGroupChair
      a       owl:ObjectProperty ;
      rdfs:comment "Describes the working groups that someone is a chair of"@en ;
      rdfs:domain :WorkingGroup ;
      rdfs:label "has working group chair"@en ;
      rdfs:range :Person ;
      rdfs:subPropertyOf :hasWorkingGroupMember ;
      <http://purl.org/vocab/vann/example>
              "BipolarWorkingGroup hasWorkingGroupChair JohnSmith"@en .

<https://schema.org/contentUrl>
      a       owl:DatatypeProperty ;
      rdfs:isDefinedBy <https://schema.org/> .

:checksum
      a       owl:DatatypeProperty ;
      rdfs:comment "checksum of data file to check if there are modifications" ;
      rdfs:domain :DataDownload ;
      rdfs:label "checksum" ;
      rdfs:range xsd:string .

:DataDownload
      a       owl:Class ;
      rdfs:comment "Dataset in downloadable form"@en ;
      rdfs:label "Data Download"@en ;
      rdfs:subClassOf <http://schema.org/DataDownload> .

<http://xmlns.com/foaf/0.1/member>
      a       owl:ObjectProperty ;
      rdfs:isDefinedBy <http://xmlns.com/foaf/0.1/member> .

:UPDRS-2
      a       owl:DatatypeProperty ;
      rdfs:comment "Unified Parkinson's Disease Rating Scale - 2" ;
      rdfs:domain :PDDemographics ;
      rdfs:label "UPDRS-2" ;
      rdfs:range xsd:boolean ;
      rdfs:subPropertyOf owl:topDataProperty .

:RBD1Q
      a       owl:DatatypeProperty ;
      rdfs:comment "REM Sleep Behavior Disorder 1 item screener" ;
      rdfs:domain :Neuropsychiatric ;
      rdfs:label "RBD1Q" ;
      rdfs:range xsd:boolean ;
      rdfs:subPropertyOf owl:topDataProperty .

:raceEthnicity
      a       owl:DatatypeProperty ;
      rdfs:comment "race/ethnicity of the subjects" ;
      rdfs:domain :PDDemographics ;
      rdfs:label "Race/Ethnicity" ;
      rdfs:range xsd:boolean .

:PhiladelphiaVerbalLearningTest
      a       owl:DatatypeProperty ;
      rdfs:comment "Assesses learning for a set of 12 words across 5 learning trials" ;
      rdfs:domain :Cognitive ;
      rdfs:label "Philadelphia Verba lLearning Test" ;
      rdfs:range xsd:boolean ;
      rdfs:subPropertyOf owl:topDataProperty .

:CoagulationScreenPerformed
      a       owl:DatatypeProperty ;
      rdfs:domain :Cardiovascular ;
      rdfs:label "Coagulation Screen Performed" ;
      rdfs:range xsd:boolean ;
      rdfs:subPropertyOf owl:topDataProperty .

<http://purl.org/vocab/vann/preferredNamespaceUri>
      a       owl:AnnotationProperty .

:handedness
      a       owl:DatatypeProperty ;
      rdfs:comment "dominant hand (left/right) of the subjects" ;
      rdfs:domain :PDDemographics ;
      rdfs:label "Handedness" ;
      rdfs:range xsd:boolean .

:UPDRS-3
      a       owl:DatatypeProperty ;
      rdfs:comment "Unified Parkinson's Disease Rating Scale - 3" ;
      rdfs:domain :PDDemographics ;
      rdfs:label "UPDRS-3" ;
      rdfs:range xsd:boolean .

:hasStudyDesign
      a       owl:DatatypeProperty ;
      rdfs:comment """Describes the study design of the cohort group or project (Case/control; Population; Healthy only; Patients only)

NOTE: study design options are mutually exclusive for Cohort Groups but not Projects"""@en , """Describes the study design of a project (Case/control; Population; Healthy only; Patients only)
NOTE: study design options are mutually exclusive for Cohort Groups but not Projects"""@en ;
      rdfs:domain :Project ;
      rdfs:domain
              [ a       owl:Class ;
                owl:unionOf (:CohortGroup :Project)
              ] ;
      rdfs:label "has study design"@en ;
      rdfs:range xsd:string ;
      <http://purl.org/vocab/vann/example>
              "Project1 hasStudyDesign \"Case/control, Population\""@en , "CohortGroup1 hasStudyDesign \"Population\""@en .

:hasGeneticDataType
      a       owl:ObjectProperty ;
      rdfs:comment "Describes the genetic data types that were collected for a cohort or project"@en ;
      rdfs:domain
              [ a       owl:Class ;
                owl:unionOf (:Cohort :CohortGroup :CohortProject)
              ] ;
      rdfs:domain
              [ a       owl:Class ;
                owl:unionOf (:Cohort :CohortGroup :CohortProject)
              ] ;
      rdfs:domain
              [ a       owl:Class ;
                owl:unionOf (:Cohort :CohortGroup :CohortProject)
              ] ;
      rdfs:domain
              [ a       owl:Class ;
                owl:unionOf (:Cohort :CohortGroup :CohortProject)
              ] ;
      rdfs:domain
              [ a       owl:Class ;
                owl:unionOf (:Cohort :CohortGroup :CohortProject)
              ] ;
      rdfs:label "has genetic data type"@en ;
      rdfs:range :GeneticDataType ;
      rdfs:subPropertyOf :hasDataType ;
      <http://purl.org/vocab/vann/example>
              "Cohort1 hasGeneticDataType epigenetic"@en .

:MentalHealthDisorder
      a       owl:Class ;
      rdfs:comment "Disorders which can affect mood, behavior, and thinking"@en ;
      rdfs:label "Mental Health Disorder"@en ;
      rdfs:subClassOf :Disorder ;
      <http://purl.org/vocab/vann/example>
              "OCD"@en .

:isPartOfProject
      a       owl:ObjectProperty ;
      rdfs:comment "Property that indicates the cohort groups specific to a project"@en ;
      rdfs:domain
              [ a       owl:Class ;
                owl:unionOf (:CohortGroup :CohortProject)
              ] ;
      rdfs:domain
              [ a       owl:Class ;
                owl:unionOf (:CohortGroup :CohortProject)
              ] ;
      rdfs:domain
              [ a       owl:Class ;
                owl:unionOf (:CohortGroup :CohortProject)
              ] ;
      rdfs:domain
              [ a       owl:Class ;
                owl:unionOf (:CohortGroup :CohortProject)
              ] ;
      rdfs:domain
              [ a       owl:Class ;
                owl:unionOf (:CohortGroup :CohortProject)
              ] ;
      rdfs:label "is part of project"@en ;
      rdfs:range :Project .

:hasContentUrl
      a       owl:DatatypeProperty ;
      rdfs:comment "Points to a media object, like an image or video file" ;
      rdfs:domain :DataDownload ;
      rdfs:label "has content URL" ;
      rdfs:range xsd:anyURI ;
      rdfs:subPropertyOf <https://schema.org/contentUrl> .

:NeurologicalDisorder
      a       owl:Class ;
      rdfs:comment "Disorders which affect the nervous system"@en ;
      rdfs:label "Neurological Disorder"@en ;
      rdfs:subClassOf :Disorder ;
      <http://purl.org/vocab/vann/example>
              "Epilepsy"@en .

:hasCurrentJobTitle
      a       owl:DatatypeProperty ;
      rdfs:comment "Data property that aims to capture the current job title of a person. Examples are student, faculty, staff, postdoc, etc."@en ;
      rdfs:domain :Person ;
      rdfs:label "has current job title"@en ;
      rdfs:range xsd:string ;
      <http://purl.org/vocab/vann/example>
              "JohnSmith hasCurrentJobTitle \"Postdoc\""@en .

:SubstanceAbuse
      a       owl:Class ;
      rdfs:comment "A mental health disorder defined by the overusage or abuse of a substance"@en ;
      rdfs:label "Substance Abuse"@en ;
      rdfs:subClassOf :MentalHealthDisorder ;
      <http://purl.org/vocab/vann/example>
              "Alcoholism"@en .

:hasDate_DataContributionDeadline
      a       owl:DatatypeProperty ;
      rdfs:comment "Describes the deadline date for data contribution of a project"@en ;
      rdfs:domain :Project ;
      rdfs:label "has data contribution deadline date"@en ;
      rdfs:range xsd:date .

:HistoryOfStrokeOrTransientIschaemicAttack
      a       owl:DatatypeProperty ;
      rdfs:comment "Transient Ischaemic Attack: A \"mini stroke\" with minor stroke symptoms" ;
      rdfs:domain :Cardiovascular ;
      rdfs:label "History of Stroke or Transient Ischaemic Attack" ;
      rdfs:range xsd:boolean ;
      rdfs:subPropertyOf owl:topDataProperty .

:Reys15WordTest
      a       owl:DatatypeProperty ;
      rdfs:domain :Cognitive ;
      rdfs:label "Rey's 15-word Test - Immediate Recall (RIR) and Delayed Recall (RDR)" ;
      rdfs:range xsd:boolean ;
      rdfs:subPropertyOf owl:topDataProperty .

:has_longitude
      a       owl:DatatypeProperty ;
      rdfs:comment "The longitude of the cohort" ;
      rdfs:domain :Location ;
      rdfs:label "has longitude" ;
      rdfs:range xsd:float .

:SCOPA-Autonomic
      a       owl:DatatypeProperty ;
      rdfs:comment "Scales for Outcomes in Parkinson's Disease - Autonomic" ;
      rdfs:domain :PDDemographics ;
      rdfs:label "SCOPA-Autonomic" ;
      rdfs:range xsd:boolean .

:isOverallCohort
      a       owl:DatatypeProperty ;
      rdfs:comment "Describes if a cohort is an \"overall\" cohort, or a top-level cohort without having been separated into its component cohort groups/projects" ;
      rdfs:domain :Cohort ;
      rdfs:label "Is Overall Cohort" ;
      rdfs:range xsd:boolean .

:DataType
      a       owl:Class ;
      rdfs:comment "Specifies the kinds of data collected"@en ;
      rdfs:label "Data Type"@en .

:KSS  a       owl:DatatypeProperty ;
      rdfs:comment "Karolinska Sleepiness Scale" ;
      rdfs:domain :Neuropsychiatric ;
      rdfs:label "KSS" ;
      rdfs:range xsd:boolean ;
      rdfs:subPropertyOf owl:topDataProperty .

:RBDSQ
      a       owl:DatatypeProperty ;
      rdfs:comment "REM Sleep Behavior Disorder Screening Questionnaire - full screener" ;
      rdfs:domain :Neuropsychiatric ;
      rdfs:label "RBDSQ" ;
      rdfs:range xsd:boolean ;
      rdfs:subPropertyOf owl:topDataProperty .

:WordListLearningTask
      a       owl:DatatypeProperty ;
      rdfs:comment "Word List Learning Task: Note the version used" ;
      rdfs:domain :Cognitive ;
      rdfs:label "Word List Learning Task" ;
      rdfs:range xsd:string ;
      rdfs:subPropertyOf owl:topDataProperty .

:SCOPA-Motor
      a       owl:DatatypeProperty ;
      rdfs:comment "Scales for Outcomes in Parkinson's Disease - Motor" ;
      rdfs:domain :PDDemographics ;
      rdfs:label "SCOPA-Motor" ;
      rdfs:range xsd:boolean .

:HAMA
      a       owl:DatatypeProperty ;
      rdfs:comment "Hamilton Anxiety Scale" ;
      rdfs:domain :Neuropsychiatric ;
      rdfs:label "HAMA" ;
      rdfs:range xsd:boolean ;
      rdfs:subPropertyOf owl:topDataProperty .

:has_cardiovascular
      a       owl:ObjectProperty ;
      rdfs:comment "Describes cardiovascular covariate properties specific to the PD working group" ;
      rdfs:domain :Cohort ;
      rdfs:label "has cardiovascular" ;
      rdfs:range :Cardiovascular ;
      rdfs:subPropertyOf owl:topObjectProperty .

<http://xmlns.com/foaf/0.1/Organization>
      a       owl:Class ;
      rdfs:comment "An organization contributing to a given ENIGMA project"@en ;
      rdfs:isDefinedBy <http://xmlns.com/foaf/0.1> ;
      owl:equivalentClass :Organization .

:OrganicMedicalDisorder
      a       owl:Class ;
      rdfs:comment "Disorder characterized by decreased mental function due to a medical or physical disease"@en ;
      rdfs:label "Organic Medical Disorder"@en ;
      rdfs:subClassOf :Disorder ;
      <http://purl.org/vocab/vann/example>
              "Delirium"@en .

:hasMiddleInitial
      a       owl:DatatypeProperty ;
      rdfs:comment "Describes middle initial of a person"^^xsd:string ;
      rdfs:domain :Person ;
      rdfs:label "has middle initial"@en ;
      rdfs:range xsd:string ;
      <http://purl.org/vocab/vann/example>
              "John A Smith hasMiddleInitial \"A\""^^xsd:string .

<http://purl.org/vocab/vann/preferredNamespacePrefix>
      a       owl:AnnotationProperty .

<http://purl.org/dc/terms/contributor>
      a       owl:AnnotationProperty .

:hasSpecies
      a       owl:DatatypeProperty ;
      rdfs:comment "Describes the species of the subjects of a cohort (Humans, Chimps, Mice, etc.)"@en ;
      rdfs:domain
              [ a       owl:Class ;
                owl:unionOf (:Cohort :CohortGroup :CohortProject)
              ] ;
      rdfs:label "has species"@en ;
      rdfs:range xsd:string ;
      <http://purl.org/vocab/vann/example>
              "Cohort1 hasSpecies \"humans\""@en .

:STAI
      a       owl:DatatypeProperty ;
      rdfs:comment "State-Trait Anxiety Index" ;
      rdfs:domain :Neuropsychiatric ;
      rdfs:label "STAI" ;
      rdfs:range xsd:boolean ;
      rdfs:subPropertyOf owl:topDataProperty .

:DigitSpanForward
      a       owl:DatatypeProperty ;
      rdfs:domain :Cognitive ;
      rdfs:label "Digit Span Forward" ;
      rdfs:range xsd:boolean ;
      rdfs:subPropertyOf owl:topDataProperty .

:isActive
      a       owl:DatatypeProperty ;
      rdfs:comment "Describes whether a project is active"@en ;
      rdfs:domain :Project ;
      rdfs:label "is Active"@en ;
      rdfs:range xsd:string .

:has_location
      a       owl:ObjectProperty ;
      rdfs:comment "The location of the cohort" ;
      rdfs:domain :Cohort ;
      rdfs:label "has location" ;
      rdfs:range :Location .

:BrainScanDataType
      a       owl:Class ;
      rdfs:comment "Specifies the kinds of brain scan data collected"@en ;
      rdfs:label "Brain Scan Data Type"@en ;
      rdfs:subClassOf :DataType ;
      <http://purl.org/vocab/vann/example>
              "EEG"@en .

:hasDataset
      a       owl:ObjectProperty ;
      rdfs:comment "Property that links a cohort project with the data being described."@en ;
      rdfs:domain
              [ a       owl:Class ;
                owl:unionOf (:Cohort :CohortProject)
              ] ;
      rdfs:domain
              [ a       owl:Class ;
                owl:unionOf (:Cohort :CohortProject)
              ] ;
      rdfs:domain
              [ a       owl:Class ;
                owl:unionOf (:Cohort :CohortProject)
              ] ;
      rdfs:domain
              [ a       owl:Class ;
                owl:unionOf (:Cohort :CohortProject)
              ] ;
      rdfs:domain
              [ a       owl:Class ;
                owl:unionOf (:Cohort :CohortProject)
              ] ;
      rdfs:label "has dataset"@en ;
      rdfs:range :Dataset .

:education
      a       owl:DatatypeProperty ;
      rdfs:domain :PDDemographics ;
      rdfs:label "Education" ;
      rdfs:range xsd:boolean .

:usesProtocol
      a       owl:ObjectProperty ;
      rdfs:comment "Describes which protocol was used in a project"@en ;
      rdfs:domain :Project ;
      rdfs:label "uses protocol"@en ;
      rdfs:range :DataProcessingProtocol ;
      <http://purl.org/vocab/vann/example>
              "BipolarProject usesProtocol ENIGMA-SulciProtocol"@en .

:SupineBloodPressure
      a       owl:DatatypeProperty ;
      rdfs:comment "Supine blood pressure after resting for at least 5 minutes" ;
      rdfs:domain :Cardiovascular ;
      rdfs:label "Supine Blood Pressure" ;
      rdfs:range xsd:boolean ;
      rdfs:subPropertyOf owl:topDataProperty .

:ImageAcquisitionProtocol
      a       owl:Class ;
      rdfs:comment "Procedure used to collect image data within the cohort"@en ;
      rdfs:label "Image Acquisition Protocol"@en ;
      <http://purl.org/vocab/vann/example>
              "ENIGMA-Sulci"@en .

xsd:date
      a       rdfs:Datatype .

:CDSS
      a       owl:DatatypeProperty ;
      rdfs:comment "Calgary Depression Symptom Scale" ;
      rdfs:domain :Neuropsychiatric ;
      rdfs:label "CDSS" ;
      rdfs:range xsd:boolean .

:DigitSpanBackward
      a       owl:DatatypeProperty ;
      rdfs:domain :Cognitive ;
      rdfs:label "Digit Span Backward" ;
      rdfs:range xsd:boolean ;
      rdfs:subPropertyOf owl:topDataProperty .

:Dataset
      a       owl:Class ;
      rdfs:comment "A dataset containing information about an ENIGMA project cohort"@en ;
      rdfs:label "Dataset"@en ;
      rdfs:subClassOf <http://schema.org/Dataset> .

:hasContact
      a       owl:ObjectProperty ;
      rdfs:comment "Property that points to the person that is a contact for the project or cohort"@en ;
      rdfs:domain
              [ a       owl:Class ;
                owl:unionOf (:Cohort :CohortGroup :CohortProject)
              ] ;
      rdfs:domain
              [ a       owl:Class ;
                owl:unionOf (:Cohort :CohortGroup :CohortProject)
              ] ;
      rdfs:domain
              [ a       owl:Class ;
                owl:unionOf (:Cohort :CohortGroup :CohortProject)
              ] ;
      rdfs:domain
              [ a       owl:Class ;
                owl:unionOf (:Cohort :CohortGroup :CohortProject)
              ] ;
      rdfs:domain
              [ a       owl:Class ;
                owl:unionOf (:Cohort :CohortGroup :CohortProject)
              ] ;
      rdfs:label "has contact"@en ;
      rdfs:range :Person ;
      <http://purl.org/vocab/vann/example>
              "BipolarCohort hasContact JohnSmith"@en .

:AcademicArticle
      a       owl:Class ;
      rdfs:comment "An academic article, submitted as a result of the work in an ENIGMA project"@en ;
      rdfs:label "Academic article"@en .

:hasEmail
      a       owl:ObjectProperty ;
      rdfs:comment "Property that indicates which is the email of a person"@en ;
      rdfs:domain :Person ;
      rdfs:label "has email"@en ;
      rdfs:range owl:Thing ;
      rdfs:subPropertyOf <http://xmlns.com/foaf/0.1/mbox> ;
      <http://www.linkedmodel.org/schema/vaem#rationale>
              "Property added to facilitate interaction with domain and ranges in the wiki. It's equivalent to foaf:mbox"@en .

:hasFamilyName
      a       owl:DatatypeProperty ;
      rdfs:comment "The family name of some person."@en ;
      rdfs:domain :Person ;
      rdfs:label "has family name"@en ;
      rdfs:range xsd:string ;
      rdfs:subPropertyOf <http://xmlns.com/foaf/0.1/familyName> ;
      <http://www.linkedmodel.org/schema/vaem#rationale>
              "Property added to restrict the domain to enigma:Person. This is done for facilitating the interaction with the wiki interface"@en .

:SCOPA-Sleep
      a       owl:DatatypeProperty ;
      rdfs:comment "Scales for Outcomes in Parkinson's Disease - Sleep" ;
      rdfs:domain :PDDemographics ;
      rdfs:label "SCOPA-Sleep" ;
      rdfs:range xsd:boolean .

:STAXI
      a       owl:DatatypeProperty ;
      rdfs:comment "State-Trait Anger Expression Inventory" ;
      rdfs:domain :Neuropsychiatric ;
      rdfs:label "STAXI" ;
      rdfs:range xsd:boolean ;
      rdfs:subPropertyOf owl:topDataProperty .

:FamilyHistoryOfCVDisease
      a       owl:DatatypeProperty ;
      rdfs:comment "CV: Cardiovascular Disease" ;
      rdfs:domain :Cardiovascular ;
      rdfs:label "Family History of CV Disease" ;
      rdfs:range xsd:boolean ;
      rdfs:subPropertyOf owl:topDataProperty .

:BostonNamingTest
      a       owl:DatatypeProperty ;
      rdfs:comment "The Boston Naming Test is a widely used assessment tool that evaluates a person's ability to name objects from line drawings." ;
      rdfs:domain :Cognitive ;
      rdfs:label "Boston Naming Test" ;
      rdfs:range xsd:boolean ;
      rdfs:subPropertyOf owl:topDataProperty .

:ConflictOfInterest
      a       owl:Class ;
      rdfs:comment "Concept used to represent a conflict of interest of an author in a paper"@en ;
      rdfs:label "Conflict of interest"@en .

:hasCohortStatus
      a       owl:DatatypeProperty ;
      rdfs:comment "Describes the current status of a cohort, cohort group or cohort project"@en ;
      rdfs:domain
              [ a       owl:Class ;
                owl:unionOf (:Cohort :CohortGroup :CohortProject)
              ] ;
      rdfs:label "has cohort status"@en ;
      rdfs:range
              [ a       rdfs:Datatype ;
                owl:oneOf
                        [ a       rdf:List ;
                          rdf:first "gathering participants" ;
                          rdf:rest
                                  [ a       rdf:List ;
                                    rdf:first "protocol preparation" ;
                                    rdf:rest
                                            [ a       rdf:List ;
                                              rdf:first "published" ;
                                              rdf:rest
                                                      [ a       rdf:List ;
                                                        rdf:first "revision" ;
                                                        rdf:rest ()
                                                      ]
                                            ]
                                  ]
                        ]
              ] ;
      <http://purl.org/vocab/vann/example>
              "CohortGroup1 hasCohortStatus published"@en .

:subjectSES
      a       owl:DatatypeProperty ;
      rdfs:comment "Subjects' Socioeconomic Status" ;
      rdfs:domain :PDDemographics ;
      rdfs:label "Subject SES" ;
      rdfs:range xsd:boolean .

:BAI  a       owl:DatatypeProperty ;
      rdfs:comment "Beck's Anxiety Index" ;
      rdfs:domain :Neuropsychiatric ;
      rdfs:label "BAI" ;
      rdfs:range xsd:boolean ;
      rdfs:subPropertyOf owl:topDataProperty .

:PatientMedicationOnOffDuringUPDRS
      a       owl:DatatypeProperty ;
      rdfs:comment "If the patient was on medication during Unified Parkinson's Disease Rating Scale measurements" ;
      rdfs:domain :PDDemographics ;
      rdfs:label "Patient Medication On/Off During UPDRS" ;
      rdfs:range xsd:boolean .

:OtherNeuropsychiatricCovariates
      a       owl:DatatypeProperty ;
      rdfs:domain :Neuropsychiatric ;
      rdfs:label "Other Neuropsychiatric Covariates" ;
      rdfs:range xsd:string ;
      rdfs:subPropertyOf owl:topDataProperty .

:SHAPS
      a       owl:DatatypeProperty ;
      rdfs:comment "Snaith Hamilton Rating Scale" ;
      rdfs:domain :Neuropsychiatric ;
      rdfs:label "SHAPS" ;
      rdfs:range xsd:boolean ;
      rdfs:subPropertyOf owl:topDataProperty .

:EndocrineDisorder
      a       owl:Class ;
      rdfs:comment "Disorders which affect the endocrine system"@en ;
      rdfs:label "Endocrine Disorder"@en ;
      rdfs:subClassOf :Disorder ;
      <http://purl.org/vocab/vann/example>
              "Hypothyroidism"@en .

:hasAge_StandardDeviation
      a       owl:DatatypeProperty ;
      rdfs:comment "Describes the standard deviation of the age of a cohort"@en ;
      rdfs:domain
              [ a       owl:Class ;
                owl:unionOf (:CohortGroup :CohortProject)
              ] ;
      rdfs:label "has age standard deviation"@en ;
      rdfs:range xsd:double ;
      <http://purl.org/vocab/vann/example>
              "Cohort1 hasAge_StandardDeviation 5.0"@en .

:hasPersonRole_Investigator
      a       owl:ObjectProperty ;
      rdfs:comment "Describe the investigators of a cohort"@en ;
      rdfs:domain :Cohort ;
      rdfs:label "has person role investigator"@en ;
      rdfs:range :Person ;
      <http://purl.org/vocab/vann/example>
              "BipolarCohort hasInvestigator JohnSmith"@en .

:SCOPA-Cognition
      a       owl:DatatypeProperty ;
      rdfs:comment "Scales for Outcomes in Parkinson's Disease - Cognition" ;
      rdfs:domain :PDDemographics ;
      rdfs:label "SCOPA-Cognition" ;
      rdfs:range xsd:boolean .

:hasPersonRole_PrincipalInvestigator
      a       owl:ObjectProperty ;
      rdfs:comment "Describes who the principal investigator of the cohort is"@en , "Describes the principal investigator of the cohort"@en ;
      rdfs:domain :Cohort ;
      rdfs:label "has PersonRole Principal Investigator"@en , "has person role principal investigator"@en ;
      rdfs:range :Person ;
      rdfs:subPropertyOf :hasPersonRole_Investigator ;
      <http://purl.org/vocab/vann/example>
              "Cohort1 hasPrincipalInvestigator JohnSmith"@en , "Cohort1 hasPrincipalInvestigator John --> the principal investigator of Cohort1 is John"@en .

:durill
      a       owl:DatatypeProperty ;
      rdfs:comment "Duration of Illness" ;
      rdfs:domain :PDDemographics ;
      rdfs:label "DURILL" ;
      rdfs:range xsd:boolean .

:otherDemographics
      a       owl:DatatypeProperty ;
      rdfs:comment "Other Demographics info for PD cohorts" ;
      rdfs:domain :PDDemographics ;
      rdfs:label "Other Demographics" ;
      rdfs:range xsd:string .

:hasHomePage
      a       owl:DatatypeProperty , owl:ObjectProperty ;
      rdfs:comment "Property that describes the home page of a cohort or person"@en , "Homepage URL of the Person or Cohort"@en ;
      rdfs:domain
              [ a       owl:Class ;
                owl:unionOf (:Cohort :CohortGroup :CohortProject :Person)
              ] ;
      rdfs:domain
              [ a       owl:Class ;
                owl:unionOf (:Cohort :Person)
              ] ;
      rdfs:domain
              [ a       owl:Class ;
                owl:unionOf (:Cohort :CohortGroup :CohortProject :Person)
              ] ;
      rdfs:domain
              [ a       owl:Class ;
                owl:unionOf (:Cohort :CohortGroup :CohortProject :Person)
              ] ;
      rdfs:domain
              [ a       owl:Class ;
                owl:unionOf (:Cohort :CohortGroup :CohortProject :Person)
              ] ;
      rdfs:domain
              [ a       owl:Class ;
                owl:unionOf (:Cohort :CohortGroup :CohortProject :Person)
              ] ;
      rdfs:label "has home page"@en ;
      rdfs:range owl:Thing , xsd:anyURI ;
      <http://www.linkedmodel.org/schema/vaem#rationale>
              "Property added to facilitate interaction with domain and ranges in the wiki. It's equivalent to foaf:homePage"@en .

:AES  a       owl:DatatypeProperty ;
      rdfs:comment "Apathy Evaluation Scale - 12 item scale or 18 item scale" ;
      rdfs:domain :Neuropsychiatric ;
      rdfs:label "AES" ;
      rdfs:range xsd:string ;
      rdfs:subPropertyOf owl:topDataProperty .

:Covariates
      a       owl:Class ;
      rdfs:comment "A class used to describe covariates information for a cohort or study." ;
      rdfs:label "Covariates" .

:otherMotorEvaluation
      a       owl:DatatypeProperty ;
      rdfs:comment "Other Motor Evaluations" ;
      rdfs:domain :PDDemographics ;
      rdfs:label "Other Motor Evaluations" ;
      rdfs:range xsd:string .

:hasDataCollectionPeriodEnd
      a       owl:DatatypeProperty ;
      rdfs:comment "Describes the end year of the data collection period of the cohort"@en ;
      rdfs:domain
              [ a       owl:Class ;
                owl:unionOf (:Cohort :CohortGroup :CohortProject)
              ] ;
      rdfs:label "has data collection period end"@en ;
      rdfs:range xsd:gYear ;
      <http://purl.org/vocab/vann/example>
              "Cohort1 hasDataCollectionPeriodEnd 2008"@en .

:BDI  a       owl:DatatypeProperty ;
      rdfs:comment "Beck's Depression Inventory" ;
      rdfs:domain :Neuropsychiatric ;
      rdfs:label "BDI" ;
      rdfs:range xsd:boolean ;
      rdfs:subPropertyOf owl:topDataProperty .

:UPDRS-4
      a       owl:DatatypeProperty ;
      rdfs:comment "Unified Parkinson's Disease Rating Scale - 4" ;
      rdfs:domain :PDDemographics ;
      rdfs:label "UPDRS-4" ;
      rdfs:range xsd:boolean .

:hasTransgenderMtoF
      a       owl:DatatypeProperty ;
      rdfs:comment "Describing the number of male to female transgender individuals in a cohort group"@en ;
      rdfs:domain :CohortGroup ;
      rdfs:label "has transgender m to f"@en ;
      rdfs:range xsd:nonNegativeInteger ;
      <http://purl.org/vocab/vann/example>
              "CohortGroup1 hasTransgenderMtoF 20"@en .

:MoCA
      a       owl:DatatypeProperty ;
      rdfs:comment "Montreal Cognitive Assessment" ;
      rdfs:domain :Cognitive ;
      rdfs:label "MoCA" ;
      rdfs:range xsd:boolean ;
      rdfs:subPropertyOf owl:topDataProperty .

:hasPopulationGroup
      a       owl:ObjectProperty ;
      rdfs:comment "Describes the population group of a population-based cohort"@en ;
      rdfs:domain
              [ a       owl:Class ;
                owl:unionOf (:Cohort :CohortGroup :CohortProject)
              ] ;
      rdfs:domain
              [ a       owl:Class ;
                owl:unionOf (:Cohort :CohortGroup :CohortProject)
              ] ;
      rdfs:domain
              [ a       owl:Class ;
                owl:unionOf (:Cohort :CohortGroup :CohortProject)
              ] ;
      rdfs:domain
              [ a       owl:Class ;
                owl:unionOf (:Cohort :CohortGroup :CohortProject)
              ] ;
      rdfs:domain
              [ a       owl:Class ;
                owl:unionOf (:Cohort :CohortGroup :CohortProject)
              ] ;
      rdfs:label "has population group"@en ;
      rdfs:range :CohortGroup ;
      rdfs:subPropertyOf :hasCohortGroup ;
      <http://purl.org/vocab/vann/example>
              "BipolarCohort hasPopulationGroup USCPopulationGroup"@en .

<https://schema.org/description>
      a       owl:DatatypeProperty ;
      rdfs:isDefinedBy <https://schema.org/> .

:hasAge_Group
      a       owl:DatatypeProperty ;
      rdfs:comment "Describes the age groupings of individuals within a cohort group"@en ;
      rdfs:domain :Cohort ;
      rdfs:label "has age group"@en ;
      rdfs:range xsd:string ;
      <http://purl.org/vocab/vann/example>
              "Cohort1 hasAge_Group \"22-45\""@en .

:CerebrovascularDisorder
      a       owl:Class ;
      rdfs:comment "A subset of vascular disorders affecting blood vessels of the brain and cerebral circulation"@en ;
      rdfs:label "Cerebrovascular Disorder"@en ;
      rdfs:subClassOf :VascularDisorder ;
      <http://purl.org/vocab/vann/example>
              "Stroke"@en .

:Neuropsychiatric
      a       owl:Class ;
      rdfs:comment "Neuropsychiatric Covariates measured by each cohort" , "Neuropsychiatric Covariates measured by each PD cohort" ;
      rdfs:label "Neuropsychiatric" .

:WAIS_4_VerbalComprehension
      a       owl:DatatypeProperty ;
      rdfs:comment "This index reflects an individual’s ability to understand, use and think with spoken language on the WAIS 4 (Wechsler Adult Intelligence Scale-IV) scale" ;
      rdfs:domain :Cognitive ;
      rdfs:label "WAIS 4 Verbal Comprehension" ;
      rdfs:range xsd:boolean ;
      rdfs:subPropertyOf owl:topDataProperty .

:hasGroupCriteria
      a       owl:DatatypeProperty ;
      rdfs:comment "Criteria used to define group of cohort patients"@en ;
      rdfs:domain :CohortGroup ;
      rdfs:label "has group criteria"@en ;
      rdfs:range xsd:string .

:BodyMassIndex
      a       owl:DatatypeProperty ;
      rdfs:domain :Cardiovascular ;
      rdfs:label "Body Mass Index" ;
      rdfs:range xsd:boolean ;
      rdfs:subPropertyOf owl:topDataProperty .

:LogicalMemoryTest
      a       owl:DatatypeProperty ;
      rdfs:comment "The Logical Memory (LM) test is a part of the Wechsler Memory Scale, Fourth Edition (WMS-IV) that measures a person's ability to remember narrative stories" ;
      rdfs:domain :Cognitive ;
      rdfs:label "Logical Memory Test" ;
      rdfs:range xsd:boolean ;
      rdfs:subPropertyOf owl:topDataProperty .

:hasBrainScanDataType
      a       owl:ObjectProperty ;
      rdfs:comment "Describes which brain scan data types a cohort or project has"@en , "Describes the brain scan data types that were collected for a cohort or project"@en ;
      rdfs:domain
              [ a       owl:Class ;
                owl:unionOf (:Cohort :CohortGroup :CohortProject :Project)
              ] ;
      rdfs:domain
              [ a       owl:Class ;
                owl:unionOf (:Cohort :CohortGroup :CohortProject :Project)
              ] ;
      rdfs:domain
              [ a       owl:Class ;
                owl:unionOf (:Cohort :CohortGroup :CohortProject :Project)
              ] ;
      rdfs:domain
              [ a       owl:Class ;
                owl:unionOf (:Cohort :CohortGroup :CohortProject :Project)
              ] ;
      rdfs:domain
              [ a       owl:Class ;
                owl:unionOf (:Cohort :Project)
              ] ;
      rdfs:domain
              [ a       owl:Class ;
                owl:unionOf (:Cohort :CohortGroup :CohortProject :Project)
              ] ;
      rdfs:label "has brain scan data type"@en ;
      rdfs:range :BrainScanDataType ;
      rdfs:subPropertyOf :hasDataType ;
      <http://purl.org/vocab/vann/example>
              "Cohort1 hasBrainScanDataType MRI"@en , "BipolarProject hasBrainScanDataType DiffusionMRI"@en .

:GeneticDisorder
      a       owl:Class ;
      rdfs:comment "Disorders which are inherited and caused by abnormalities in the genome"@en ;
      rdfs:label "Genetic Disorder"@en ;
      rdfs:subClassOf :Disorder ;
      <http://purl.org/vocab/vann/example>
              "Cystic Fibrosis"@en .

:Project
      a       owl:Class ;
      rdfs:comment "Project encompassing cohort"@en , "Project associated with the cohort"@en ;
      rdfs:label "Project"@en ;
      <http://purl.org/vocab/vann/example>
              "SZPositiveSymptoms"@en .

:MMSE
      a       owl:DatatypeProperty ;
      rdfs:comment "Mini Mental State Exam" ;
      rdfs:domain :Cognitive ;
      rdfs:label "MMSE" ;
      rdfs:range xsd:boolean ;
      rdfs:subPropertyOf owl:topDataProperty .

<http://purl.org/dc/terms/license>
      a       owl:AnnotationProperty .

<http://purl.org/dc/terms/title>
      a       owl:AnnotationProperty .

:Country
      a       owl:Class ;
      rdfs:comment "Country in which a cohort is located"@en ;
      rdfs:label "Country"@en ;
      rdfs:subClassOf :Location ;
      <http://purl.org/vocab/vann/example>
              "United States"@en .

:OtherCognitiveCovariates
      a       owl:DatatypeProperty ;
      rdfs:domain :Cognitive ;
      rdfs:label "Other Cognitive Covariates" ;
      rdfs:range xsd:string ;
      rdfs:subPropertyOf owl:topDataProperty .

:WCST-SF
      a       owl:DatatypeProperty ;
      rdfs:comment "Wisconsin Card Sorting Test - Short Form" ;
      rdfs:domain :Cognitive ;
      rdfs:label "WCST-SF" ;
      rdfs:range xsd:boolean ;
      rdfs:subPropertyOf owl:topDataProperty .

:iq   a       owl:DatatypeProperty ;
      rdfs:comment "IQ of participants" ;
      rdfs:domain :PDDemographics ;
      rdfs:label "IQ" ;
      rdfs:range xsd:boolean .

:hasTransgenderFtoM
      a       owl:DatatypeProperty ;
      rdfs:comment "Describing the number of female to male transgender individuals in a cohort group"@en ;
      rdfs:domain :CohortGroup ;
      rdfs:label "has transgender F to M"@en ;
      rdfs:range xsd:nonNegativeInteger ;
      <http://purl.org/vocab/vann/example>
              "CohortGroup2 hasTransgenderFtoM 14"@en .

:TowerOfLondon
      a       owl:DatatypeProperty ;
      rdfs:comment "The Tower of London tests executive planning proficiency, incorporating delineation, organization, and integration of behaviors needed to achieve a goal." ;
      rdfs:domain :Cognitive ;
      rdfs:label "Tower Of London" ;
      rdfs:range xsd:boolean ;
      rdfs:subPropertyOf owl:topDataProperty .

:UPDRSTotal
      a       owl:DatatypeProperty ;
      rdfs:comment "Unified Parkinson's Disease Rating Scale - Total Score" ;
      rdfs:domain :PDDemographics ;
      rdfs:label "UPDRS Total" ;
      rdfs:range xsd:boolean .

:Cognitive
      a       owl:Class ;
      rdfs:comment "Cognitive Covariates measured by each PD cohort" ;
      rdfs:label "Cognitive" .

:maritalStatus
      a       owl:DatatypeProperty ;
      rdfs:comment "Subjects' marital status" ;
      rdfs:domain :PDDemographics ;
      rdfs:label "Marital Status" ;
      rdfs:range xsd:boolean .

:hasAge_Maximum
      a       owl:DatatypeProperty ;
      rdfs:comment "Describes inclusion criteria for maximum age of participants in a Cohort, CohortProject or CohortGroup"@en ;
      rdfs:domain
              [ a       owl:Class ;
                owl:unionOf (:Cohort :CohortGroup :CohortProject :Covariates)
              ] ;
      rdfs:label "has maximum age"@en ;
      rdfs:range xsd:positiveInteger ;
      <http://purl.org/vocab/vann/example>
              "CohortGroup1 hasAge_Maximum 60"@en .

<http://schema.org/Dataset>
      a       owl:Class ;
      rdfs:comment "Dataset" ;
      rdfs:isDefinedBy <http://schema.org> ;
      rdfs:label "Dataset" .

:AlcoholConsumption
      a       owl:DatatypeProperty ;
      rdfs:comment "Include info on how this was measured" ;
      rdfs:domain :Cardiovascular ;
      rdfs:label "Alcohol Consumption" ;
      rdfs:range xsd:string ;
      rdfs:subPropertyOf owl:topDataProperty .

:hasBriefDescription
      a       owl:DatatypeProperty ;
      rdfs:comment "Provides a brief description of the working group or project or cohort or image acquisition protocol"@en , "Provides a brief description of the working group or project or cohort"@en ;
      rdfs:domain
              [ a       owl:Class ;
                owl:unionOf (:Cohort :Project :WorkingGroup)
              ] ;
      rdfs:domain
              [ a       owl:Class ;
                owl:unionOf (:Cohort :CohortGroup :CohortProject :ImageAcquisitionProtocol :Project :WorkingGroup)
              ] ;
      rdfs:label "has brief description"@en ;
      rdfs:range xsd:string ;
      rdfs:subPropertyOf <http://purl.org/dc/terms/description> ;
      <http://purl.org/vocab/vann/example>
              "SZCohort hasBriefDescription \"finds correlations between schizophrenia and other conditions\""@en , "ProjectSZ hasBriefDescription \"reports effect size for corticol thickness\""@en .

:PSQI
      a       owl:DatatypeProperty ;
      rdfs:comment "Pittsburgh Sleep Quality Index - Note whether you have the 7 component scores" ;
      rdfs:domain :Neuropsychiatric ;
      rdfs:label "PSQI" ;
      rdfs:range xsd:string ;
      rdfs:subPropertyOf owl:topDataProperty .

:hasCohort
      a       owl:ObjectProperty ;
      rdfs:comment "Describes what cohorts are part of a project or working group"@en , "Describes what cohorts are part of the project"@en ;
      rdfs:domain
              [ a       owl:Class ;
                owl:unionOf (:Project :WorkingGroup)
              ] ;
      rdfs:domain
              [ a       owl:Class ;
                owl:unionOf (:Project :WorkingGroup)
              ] ;
      rdfs:label "has cohort"@en ;
      rdfs:range :Cohort ;
      <http://purl.org/vocab/vann/example>
              "BipolarProject hasCohort AmsterdamBipolarCohort --> Bipolar Project includes the Amsterdam Bipolar Cohort"@en , "BipolarProject hasCohort AmsterdamBipolarCohort"@en .

:hasFundingSource
      a       owl:DatatypeProperty ;
      rdfs:comment "Describes the funding source of the cohort"@en ;
      rdfs:domain
              [ a       owl:Class ;
                owl:unionOf (:Cohort :CohortProject)
              ] ;
      rdfs:label "has funding source"@en ;
      rdfs:range xsd:string ;
      <http://purl.org/vocab/vann/example>
              "Cohort1 hasFundingSource \"NIMH, 5P50MH080272\""@en .

:FivePointTest
      a       owl:DatatypeProperty ;
      rdfs:comment "Five Point Test (5TT) is a neuropsychological test that assesses figural fluency. A participant is asked to generate as many unique designs as possible in a certain time limit." ;
      rdfs:domain :Cognitive ;
      rdfs:label "Five Point Test" ;
      rdfs:range xsd:boolean ;
      rdfs:subPropertyOf owl:topDataProperty .

:GeneticDataType
      a       owl:Class ;
      rdfs:comment "Specifies the kinds of genetic data collected"@en ;
      rdfs:label "Genetic Data Type"@en ;
      rdfs:subClassOf :DataType ;
      <http://purl.org/vocab/vann/example>
              "Epigenetic"@en .

:hasResearchInterest
      a       owl:DatatypeProperty ;
      rdfs:comment "Describes a research interest of a person"@en ;
      rdfs:domain :Person ;
      rdfs:label "has research interest"@en ;
      rdfs:range xsd:string ;
      <http://purl.org/vocab/vann/example>
              "JohnSmith hasReasearchInterest \"bipolar disorder\", \"schizophrenia\""@en .

:Organization
      a       owl:Class ;
      rdfs:comment "An organization belonging to the ENIGMA consortium. Organization can be hospitals, universities, departments, etc." , "An organization belonging to the ENIGMA consortium. Organization can be hospitals, universities, departments, etc."@en ;
      rdfs:label "Organization"@en .

:hasDiagnosticGroup
      a       owl:ObjectProperty ;
      rdfs:comment "Describes the patient group of a cohort"@en ;
      rdfs:domain
              [ a       owl:Class ;
                owl:unionOf (:Cohort :CohortProject)
              ] ;
      rdfs:domain
              [ a       owl:Class ;
                owl:unionOf (:Cohort :CohortProject)
              ] ;
      rdfs:domain
              [ a       owl:Class ;
                owl:unionOf (:Cohort :CohortProject)
              ] ;
      rdfs:domain
              [ a       owl:Class ;
                owl:unionOf (:Cohort :CohortProject)
              ] ;
      rdfs:domain
              [ a       owl:Class ;
                owl:unionOf (:Cohort :CohortProject)
              ] ;
      rdfs:label "has diagnostic group"@en ;
      rdfs:range :CohortGroup ;
      rdfs:subPropertyOf :hasCohortGroup ;
      <http://purl.org/vocab/vann/example>
              "BipolarCohort hasPatientGroup BipolarPatientGroup"@en .

:TAS-20
      a       owl:DatatypeProperty ;
      rdfs:comment "Toronto Alexithymia Scale" ;
      rdfs:domain :Neuropsychiatric ;
      rdfs:label "TAS-20" ;
      rdfs:range xsd:boolean ;
      rdfs:subPropertyOf owl:topDataProperty .

:sex  a       owl:DatatypeProperty ;
      rdfs:comment "sex of participants" ;
      rdfs:domain :PDDemographics ;
      rdfs:label "Sex" ;
      rdfs:range xsd:boolean .

:isPublic
      a       owl:DatatypeProperty ;
      rdfs:comment "Describes if a cohort's data is publicly available"@en ;
      rdfs:domain
              [ a       owl:Class ;
                owl:unionOf (:Cohort :CohortGroup :CohortProject)
              ] ;
      rdfs:label "is public"@en ;
      rdfs:range xsd:boolean ;
      <http://purl.org/vocab/vann/example>
              "SZCohort isPublic \"true\""@en .

:hasPersonRole_MainPrincipalInvestigator
      a       owl:ObjectProperty ;
      rdfs:comment "Describes which cohorts somone is a main PI of"@en ;
      rdfs:domain
              [ a       owl:Class ;
                owl:unionOf (:Cohort :CohortGroup :CohortProject)
              ] ;
      rdfs:domain
              [ a       owl:Class ;
                owl:unionOf (:Cohort :CohortGroup :CohortProject)
              ] ;
      rdfs:domain
              [ a       owl:Class ;
                owl:unionOf (:Cohort :CohortGroup :CohortProject)
              ] ;
      rdfs:domain
              [ a       owl:Class ;
                owl:unionOf (:Cohort :CohortGroup :CohortProject)
              ] ;
      rdfs:domain
              [ a       owl:Class ;
                owl:unionOf (:Cohort :CohortGroup :CohortProject)
              ] ;
      rdfs:label "has main person role principal investigator"@en ;
      rdfs:range :Person ;
      rdfs:subPropertyOf :hasPersonRole_PrincipalInvestigator ;
      <http://purl.org/vocab/vann/example>
              "Cohort1 hasMainPrincipalInvestigatorof JohnSmith"@en .

:PANSS
      a       owl:DatatypeProperty ;
      rdfs:comment "Positive and Negative Syndrome Scale" ;
      rdfs:domain :Neuropsychiatric ;
      rdfs:label "PANSS" ;
      rdfs:range xsd:boolean ;
      rdfs:subPropertyOf owl:topDataProperty .

:SideOfOnset
      a       owl:DatatypeProperty ;
      rdfs:comment "The side of PD symptoms during PD onset" ;
      rdfs:domain :PDDemographics ;
      rdfs:label "Side of Onset" ;
      rdfs:range xsd:boolean .

:BriefVisuospatialMemoryTest
      a       owl:DatatypeProperty ;
      rdfs:comment "Assessment tool to measure visuospatial learning and memory abilities across research and clinical settings" ;
      rdfs:domain :Cognitive ;
      rdfs:label "Brief Visuospatial Memory Test" ;
      rdfs:range xsd:boolean ;
      rdfs:subPropertyOf owl:topDataProperty .

<https://w3id.org/enigma>
      a       owl:Ontology ;
      <http://purl.org/dc/terms/contributor>
              "Haripriya Dharmala"^^xsd:string , "Michael Bornstein" , "Ryan Espiritu" , "Aarya M Vakharia" , "Yolanda Gil"^^xsd:string , "MiHyun Jang" , "Aarya Vakharia" , "Agnes McMahon" ;
      <http://purl.org/dc/terms/creator>
              "Kevin Low" , "Haripriya Dharmala" , "Joanna Bright" , "Josh Boyd" , "Wesley Surento" , "Ryan Espiritu"^^xsd:string , "Yolanda Gil" , "MiHyun Jang"^^xsd:string , "Hernan Vargas" , "Daniel Garijo" , "Neda Jahanshad" , "Neda Jahanshad"^^xsd:string ;
      <http://purl.org/dc/terms/description>
              "An ontology to describe cohorts of patients participating in ENIGMA projects."@en , "An ontology that describes ENIGMA projects and their properties."@en , "A core ontology representing the main concepts of ENIGMA. This ontology includes general concepts and properties applicable to all ENIGMA working groups."@en , "A cohort ontology that describes persons participating in ENIGMA and their properties."@en ;
      <http://purl.org/dc/terms/license>
              <http://creativecommons.org/licenses/by/2.0/> ;
      <http://purl.org/dc/terms/title>
              "The Enigma Core Ontology"@en , "The PD Cognitive Ontology"@en , "The Neuropsychiatric Ontology"@en , "The Project Ontology"@en , "The Cohort Ontology"@en , "The PD Cardiovascular Ontology"@en , "The Person Ontology"^^xsd:string , "The PD Demographics Ontology"@en ;
      <http://purl.org/vocab/vann/preferredNamespacePrefix>
              "enigma" , "enigma"^^xsd:string ;
      <http://purl.org/vocab/vann/preferredNamespaceUri>
              : ;
      owl:priorVersion "https://w3id.org/enigma/cohort/1.0.0" , <https://w3id.org/enigma/core/1.0.0> , <https://w3id.org/enigma/person/1.0.0> ;
      owl:versionIRI <https://w3id.org/enigma/cohort/1.1.0> , <https://w3id.org/enigma/pd-cognitive/1.1.0> , <https://w3id.org/enigma/core/1.1.0> , <https://w3id.org/enigma/project/1.1.0> , <https://w3id.org/enigma/person/1.1.0> , <https://w3id.org/enigma/pd-cardiovascular/1.1.0> , <https://w3id.org/enigma/pd-demographics/1.1.0> , <https://w3id.org/enigma/neuropsychiatric/1.1.0> ;
      owl:versionInfo "v1.1.0" , "v1.1.0"^^xsd:string .

:HeartRate
      a       owl:DatatypeProperty ;
      rdfs:domain :Cardiovascular ;
      rdfs:label "Heart Rate" ;
      rdfs:range xsd:boolean ;
      rdfs:subPropertyOf owl:topDataProperty .

:Rey_OsterriethComplexFigureTest
      a       owl:DatatypeProperty ;
      rdfs:domain :Cognitive ;
      rdfs:label "Rey-Osterrieth Complex Figure Test" ;
      rdfs:range xsd:boolean ;
      rdfs:subPropertyOf owl:topDataProperty .

:IDS  a       owl:DatatypeProperty ;
      rdfs:comment "Inventory of Depressive Symptomology" ;
      rdfs:domain :Neuropsychiatric ;
      rdfs:label "IDS" ;
      rdfs:range xsd:boolean ;
      rdfs:subPropertyOf owl:topDataProperty .

:MADRS
      a       owl:DatatypeProperty ;
      rdfs:comment "Montgomery-Asberg Depression Rating Scale" ;
      rdfs:domain :Neuropsychiatric ;
      rdfs:label "MADRS" ;
      rdfs:range xsd:boolean ;
      rdfs:subPropertyOf owl:topDataProperty .

:MoodDisorder
      a       owl:Class ;
      rdfs:comment "A mental health disorder defined by mood or behavioral swings"@en ;
      rdfs:label "Mood Disorder"@en ;
      rdfs:subClassOf :MentalHealthDisorder ;
      <http://purl.org/vocab/vann/example>
              "Bipolar Disorder"@en .

:PictureArrangementTest
      a       owl:DatatypeProperty ;
      rdfs:comment "A psychological test that presents a series of pictures in a random order and asks the subject to arrange them to form a logical story." ;
      rdfs:domain :Cognitive ;
      rdfs:label "Picture Arrangement Test" ;
      rdfs:range xsd:boolean ;
      rdfs:subPropertyOf owl:topDataProperty .

<http://schema.org/DataDownload>
      a       owl:Class ;
      rdfs:isDefinedBy <http://schema.org> ;
      rdfs:label "Data Download" .

:hasPublication
      a       owl:ObjectProperty ;
      rdfs:comment "Property that links a project to a publication that resulted from it."@en ;
      rdfs:domain :Project ;
      rdfs:label "has publication"@en ;
      rdfs:range :AcademicArticle .

:hasCohortGroup
      a       owl:ObjectProperty ;
      rdfs:comment "Property that indicates the cohort groups part of a cohort"@en ;
      rdfs:domain
              [ a       owl:Class ;
                owl:unionOf (:Cohort :CohortProject)
              ] ;
      rdfs:domain
              [ a       owl:Class ;
                owl:unionOf (:Cohort :CohortProject)
              ] ;
      rdfs:domain
              [ a       owl:Class ;
                owl:unionOf (:Cohort :CohortProject)
              ] ;
      rdfs:domain
              [ a       owl:Class ;
                owl:unionOf (:Cohort :CohortProject)
              ] ;
      rdfs:domain
              [ a       owl:Class ;
                owl:unionOf (:Cohort :CohortProject)
              ] ;
      rdfs:label "has cohort group"@en ;
      rdfs:range :CohortGroup ;
      <http://purl.org/vocab/vann/example>
              "QTIM has cohort group QTIM_control"@en .

<http://vivoweb.org/ontology/core#orcidId>
      a       owl:ObjectProperty ;
      rdfs:comment "This is now an object property where the object value is a resource of the form <http://orcid.org/NNNN-NNNN-NNNN-NNNN>.  This is to support connecting VIVO and ORCID in the linked data web.   Note: a person can have multiple ORCID iDs."^^xsd:string ;
      rdfs:isDefinedBy "http://vivoweb.org/ontology/core#"@en .

<http://xmlns.com/foaf/0.1/familyName>
      a       owl:DatatypeProperty ;
      rdfs:comment "The family name of some person."^^xsd:string ;
      rdfs:domain <http://xmlns.com/foaf/0.1/Person> ;
      rdfs:isDefinedBy "http://xmlns.com/foaf/0.1/"@en .

:Location
      a       owl:Class ;
      rdfs:comment "Geographic location of the cohort"@en ;
      rdfs:label "Location"@en ;
      <http://purl.org/vocab/vann/example>
              "Los Angeles, California"@en .

:CohortProject
      a       owl:Class ;
      rdfs:comment "The subset of the individuals from a Cohort, which are used as samples for a specific project"@en ;
      rdfs:label "Cohort Project"@en ;
      rdfs:subClassOf :Cohort ;
      <http://purl.org/vocab/vann/example>
              "\"Healthy\" individuals from the ASRB Cohort were sampled to form a Cohort Project of SZCorticol"@en .

:hasCohortProject
      a       owl:ObjectProperty ;
      rdfs:comment "Describes the subcohorts, specific to a given project, that are part of that cohort"@en ;
      rdfs:domain
              [ a       owl:Class ;
                owl:unionOf (:Cohort :CohortGroup :ImageAcquisitionProtocol)
              ] ;
      rdfs:domain
              [ a       owl:Class ;
                owl:unionOf (:Cohort :CohortGroup :ImageAcquisitionProtocol)
              ] ;
      rdfs:domain
              [ a       owl:Class ;
                owl:unionOf (:Cohort :CohortGroup :ImageAcquisitionProtocol)
              ] ;
      rdfs:domain
              [ a       owl:Class ;
                owl:unionOf (:Cohort :CohortGroup :ImageAcquisitionProtocol)
              ] ;
      rdfs:domain
              [ a       owl:Class ;
                owl:unionOf (:Cohort :CohortGroup :ImageAcquisitionProtocol)
              ] ;
      rdfs:label "has cohort project"@en ;
      rdfs:range :CohortProject ;
      <http://purl.org/vocab/vann/example>
              "BipolarCohort hasCohortProject BipolarBarcelonaCohort"@en .

:PDMotorSubtype
      a       owl:DatatypeProperty ;
      rdfs:comment "PD Motor Subtypes (mild-motor predominant, intermediate, or diffuse malignant)" ;
      rdfs:domain :PDDemographics ;
      rdfs:label "PD Motor Subtype" ;
      rdfs:range xsd:boolean .

:hasGrant
      a       owl:DatatypeProperty ;
      rdfs:comment "Data property that aims to capture the grants that have been obtained by a person, in order to properly list them in the acknowledgements of the corresponding publication"@en ;
      rdfs:domain :Person ;
      rdfs:label "has grant"@en ;
      rdfs:range xsd:string ;
      <http://purl.org/vocab/vann/example>
              "John Smith hasGrant \"U54EB020403 (NIH)\""@en .

<http://xmlns.com/foaf/0.1/mbox>
      a       owl:ObjectProperty ;
      rdfs:comment "A  personal mailbox, ie. an Internet mailbox associated with exactly one owner, the first owner of this mailbox. This is a 'static inverse functional property', in that  there is (across time and change) at most one individual that ever has any particular value for foaf:mbox."^^xsd:string ;
      rdfs:domain <http://xmlns.com/foaf/0.1/Person> ;
      rdfs:isDefinedBy "http://xmlns.com/foaf/0.1/"@en ;
      rdfs:range owl:Thing .

:City
      a       owl:Class ;
      rdfs:comment "City in which a cohort is located"@en ;
      rdfs:label "City"@en ;
      rdfs:subClassOf :Location ;
      <http://purl.org/vocab/vann/example>
              "Los Angeles"@en .

:SubstanceDependence
      a       owl:Class ;
      rdfs:comment "A subset of substance abuse in which symptoms of withdrawal may appeared after reduction of substance use"@en ;
      rdfs:label "Substance Dependence"@en ;
      rdfs:subClassOf :SubstanceAbuse ;
      <http://purl.org/vocab/vann/example>
              "Alcohol Dependence"@en .

:hasNumberOfFemaleSex
      a       owl:DatatypeProperty ;
      rdfs:comment "Describing the number of females in a cohort project"@en ;
      rdfs:domain :CohortProject ;
      rdfs:label "has number of females"@en ;
      rdfs:range xsd:nonNegativeInteger ;
      <http://purl.org/vocab/vann/example>
              "CohortGroup2 hasNumberOfFemaleSex 16"@en .

:OtherRelevantDiagnoses
      a       owl:DatatypeProperty ;
      rdfs:comment "e.g. chronic kidney disease and stage, migraines, arthritis, lupus" ;
      rdfs:domain :Cardiovascular ;
      rdfs:label "Other Relevant Diagnoses" ;
      rdfs:range xsd:string ;
      rdfs:subPropertyOf owl:topDataProperty .

:hasAdditionalDemographic
      a       owl:DatatypeProperty ;
      rdfs:comment "Describes the additional demographics defining a given cohort"@en ;
      rdfs:domain :Cohort ;
      rdfs:label "has additional demographic"@en ;
      rdfs:range xsd:string ;
      <http://purl.org/vocab/vann/example>
              "CohortGroup1 hasAdditionalDemographic \"handedness, IQ\""@en .

:NART
      a       owl:DatatypeProperty ;
      rdfs:comment "The National Adult Reading test in any language" ;
      rdfs:domain :Cognitive ;
      rdfs:label "NART (National Adult Reading Test)" ;
      rdfs:range xsd:boolean ;
      rdfs:subPropertyOf owl:topDataProperty .

:subjID
      a       owl:DatatypeProperty ;
      rdfs:comment "Subject ID" ;
      rdfs:domain :PDDemographics ;
      rdfs:label "subj ID" ;
      rdfs:range xsd:boolean .

:hasCollectionSite
      a       owl:DatatypeProperty ;
      rdfs:comment "Describes where the data of the cohort was collected"@en ;
      rdfs:domain :Cohort ;
      rdfs:label "has collection site"@en ;
      rdfs:range xsd:string ;
      <http://purl.org/vocab/vann/example>
              "Cohort1 hasCollectionSite Toronto"@en .

:ISI  a       owl:DatatypeProperty ;
      rdfs:comment "Insomnia Severity Index" ;
      rdfs:domain :Neuropsychiatric ;
      rdfs:label "ISI" ;
      rdfs:range xsd:boolean ;
      rdfs:subPropertyOf owl:topDataProperty .

:WorkingGroup
      a       owl:Class ;
      rdfs:comment "Group of researchers studying a certain topic/disease"@en ;
      rdfs:label "Working Group"@en ;
      <http://purl.org/vocab/vann/example>
              "BipolarWG"@en .

:AnxietyDisorder
      a       owl:Class ;
      rdfs:comment "A mental health disorder defined by feelings of anxiety, fear, or worry"@en ;
      rdfs:label "Anxiety Disorder"@en ;
      rdfs:subClassOf :MentalHealthDisorder ;
      <http://purl.org/vocab/vann/example>
              "PTSD"@en .

xsd:gYear
      a       rdfs:Datatype .

:AtrialFibrillation
      a       owl:DatatypeProperty ;
      rdfs:comment "Atrial Fibrillation: irregular (and often rapid) heart rate caused by poor blood flow that can cause blood clots, strokes, etc." ;
      rdfs:domain :Cardiovascular ;
      rdfs:label "Atrial Fibrillation" ;
      rdfs:range xsd:boolean ;
      rdfs:subPropertyOf owl:topDataProperty .

:hasNumberOfParticipants
      a       owl:DatatypeProperty ;
      rdfs:comment "Describes the number of participants in a cohort group or cohort project"@en ;
      rdfs:domain
              [ a       owl:Class ;
                owl:unionOf (:CohortGroup :CohortProject)
              ] ;
      rdfs:label "has number of participants"@en ;
      rdfs:range xsd:int ;
      <http://purl.org/vocab/vann/example>
              "CohortGroup2 hasNumberOfParticipants 200"@en .

:OtherMedUseLifetime
      a       owl:DatatypeProperty ;
      rdfs:comment "Other Medication used during their lifetime" ;
      rdfs:domain :PDDemographics ;
      rdfs:label "Other Medication Use Lifetime" ;
      rdfs:range xsd:boolean .

<http://xmlns.com/foaf/0.1/givenName>
      a       owl:DatatypeProperty ;
      rdfs:comment "The given name of some person."@en ;
      rdfs:domain <http://xmlns.com/foaf/0.1/Person> ;
      rdfs:isDefinedBy <http://xmlns.com/foaf/0.1/> .

:hasDegree
      a       owl:DatatypeProperty ;
      rdfs:comment "Describes what degree a person has (e.g., BsC, PhD, etc.)"@en ;
      rdfs:domain :Person ;
      rdfs:label "has degree"@en ;
      rdfs:range xsd:string ;
      <http://purl.org/vocab/vann/example>
              "JohnSmith hasDegree PhD"@en .

:diagnosisConfirmed
      a       owl:DatatypeProperty ;
      rdfs:comment "If PD diagnosis was confirmed in the subject(s)" ;
      rdfs:domain :PDDemographics ;
      rdfs:label "Diagnosis Confirmed" ;
      rdfs:range xsd:boolean .

:hasDate_ProposalApproval
      a       owl:DatatypeProperty ;
      rdfs:comment "Describes the date the proposal for a project was approved"@en ;
      rdfs:domain :Project ;
      rdfs:label "has proposal approval date"@en ;
      rdfs:range xsd:date .

:hasNumberOfMaleSex
      a       owl:DatatypeProperty ;
      rdfs:comment "Describing the number of males in a cohort project"@en ;
      rdfs:domain :CohortProject ;
      rdfs:label "has number of males"@en ;
      rdfs:range xsd:nonNegativeInteger ;
      <http://purl.org/vocab/vann/example>
              "CohortGroup2 hasNumberOfMaleSex 12"@en .

<http://xmlns.com/foaf/0.1/homepage>
      a       owl:ObjectProperty ;
      rdfs:comment "A homepage for some thing." ;
      rdfs:isDefinedBy <http://xmlns.com/foaf/0.1/> ;
      rdfs:label "homepage" .

:requiresDataType
      a       owl:ObjectProperty ;
      rdfs:comment "Describes which data type is required by a project"@en ;
      rdfs:domain :Project ;
      rdfs:label "requires data type"@en ;
      rdfs:range :DataType .

:hasConflictOfInterest
      a       owl:ObjectProperty ;
      rdfs:comment "Property linking an author with a conflict of interest that the author has on a paper"@en ;
      rdfs:domain :Person ;
      rdfs:label "has conflict of interest"@en ;
      rdfs:range :ConflictOfInterest .

:DiagnosticInstrument
      a       owl:Class ;
      rdfs:comment "The method used to diagnose individuals in a Cohort"@en ;
      rdfs:label "Diagnostic Instrument"@en ;
      <http://purl.org/vocab/vann/example>
              "Consensus Consultant Diagnosis"@en .

:PAS  a       owl:DatatypeProperty ;
      rdfs:comment "Parkinson's Anxiety Scale" ;
      rdfs:domain :Neuropsychiatric ;
      rdfs:label "PAS" ;
      rdfs:range xsd:boolean ;
      rdfs:subPropertyOf owl:topDataProperty .

:hasPersonRole_ProjectContact
      a       owl:ObjectProperty ;
      rdfs:comment "Property that points to the person that is a contact for the project or cohort"@en ;
      rdfs:domain
              [ a       owl:Class ;
                owl:unionOf (:Cohort :Project)
              ] ;
      rdfs:label "has contact"@en ;
      rdfs:range :Person ;
      rdfs:subPropertyOf owl:topObjectProperty ;
      <http://purl.org/vocab/vann/example>
              "BipolarCohort hasPersonRole_ProjectContact JohnSmith"@en .

:SWCT
      a       owl:DatatypeProperty ;
      rdfs:comment "Stroop Word-Color Test" ;
      rdfs:domain :Cognitive ;
      rdfs:label "SWCT" ;
      rdfs:range xsd:boolean ;
      rdfs:subPropertyOf owl:topDataProperty .

:studiesDisorder
      a       owl:ObjectProperty ;
      rdfs:comment "Property that indicates which project/working group studies which disorder"@en ;
      rdfs:domain
              [ a       owl:Class ;
                owl:unionOf (:Project :WorkingGroup)
              ] ;
      rdfs:domain
              [ a       owl:Class ;
                owl:unionOf (:Project :WorkingGroup)
              ] ;
      rdfs:domain
              [ a       owl:Class ;
                owl:unionOf (:Project :WorkingGroup)
              ] ;
      rdfs:domain
              [ a       owl:Class ;
                owl:unionOf (:Project :WorkingGroup)
              ] ;
      rdfs:domain
              [ a       owl:Class ;
                owl:unionOf (:Project :WorkingGroup)
              ] ;
      rdfs:label "studies disorder"@en ;
      rdfs:range :Disorder .

:has_city
      a       owl:DatatypeProperty ;
      rdfs:comment "City in which cohort is located" ;
      rdfs:domain :Location ;
      rdfs:label "has city" ;
      rdfs:range xsd:string .

:hasName
      a       owl:DatatypeProperty ;
      rdfs:comment "Name of an item" ;
      rdfs:domain :Dataset ;
      rdfs:label "has name" ;
      rdfs:range xsd:string ;
      rdfs:subPropertyOf <https://schema.org/name> .

:SE-ADLS
      a       owl:DatatypeProperty ;
      rdfs:comment "Schwab and England: Activities of Daily Living Scale" ;
      rdfs:domain :PDDemographics ;
      rdfs:label "SE-ADLS" ;
      rdfs:range xsd:boolean .

:hasDate_TargetStart
      a       owl:DatatypeProperty ;
      rdfs:comment "Describes the start date of the target period of the project"@en ;
      rdfs:domain :Project ;
      rdfs:label "has target start date"@en ;
      rdfs:range xsd:date .

:MDS-UPDRS-3
      a       owl:DatatypeProperty ;
      rdfs:comment "Movement Disorders Society Unified Parkinson's Disease Rating Scale - 3" ;
      rdfs:domain :PDDemographics ;
      rdfs:label "MDS-UPDRS-3" ;
      rdfs:range xsd:boolean .

:CohortGroup
      a       owl:Class ;
      rdfs:comment "A subset of Cohort, which either forms the patient group or control group"@en ;
      rdfs:label "Cohort Group"@en ;
      rdfs:subClassOf :Cohort ;
      <http://purl.org/vocab/vann/example>
              "AMCControlGroup is a control cohort group of the AMC cohort"@en .

:otherPDDiagnosisData
      a       owl:DatatypeProperty ;
      rdfs:comment "Other Parkinson's Diagnosis Data" ;
      rdfs:domain :PDDemographics ;
      rdfs:label "Other PD Diagnosis Data" ;
      rdfs:range xsd:string .

:DataProcessingProtocol
      a       owl:Class ;
      rdfs:comment "An image processing or genetic analysis protocol used to extract brain feature data"@en ;
      rdfs:label "Data Processing Protocol"@en ;
      <http://purl.org/vocab/vann/example>
              "ENIGMA-Sulci Protocol"@en .

:Disorder
      a       owl:Class ;
      rdfs:comment "A disorder/disease experienced by members of a cohort"@en ;
      rdfs:label "Disorder"@en .

:hasProject
      a       owl:ObjectProperty ;
      rdfs:comment "Describes what projects are worked on by a specific working group"@en ;
      rdfs:domain :WorkingGroup ;
      rdfs:label "has project"@en ;
      rdfs:range :Project ;
      <http://purl.org/vocab/vann/example>
              "BipolarWorkingGroup hasProject BipolarCorticolProject --> The Bipolar Working Group is working on the Bipolar Corticol Project"@en .

:CardiovascularDisorder
      a       owl:Class ;
      rdfs:comment "A subset of vascular disorders affecting the heart"@en ;
      rdfs:label "Cardiovascular Disorder"@en ;
      rdfs:subClassOf :VascularDisorder ;
      <http://purl.org/vocab/vann/example>
              "Coronary Artery Disease"@en .

:has_PD_Demographics
      a       owl:ObjectProperty ;
      rdfs:comment "Describes demographics properties specific to the PD working group" ;
      rdfs:domain :Cohort ;
      rdfs:label "has PD demographics" ;
      rdfs:range :PDDemographics ;
      rdfs:subPropertyOf owl:topObjectProperty .

:hasAncestry
      a       owl:DatatypeProperty ;
      rdfs:comment "Describes the ancestry of the participants of the cohort"@en ;
      rdfs:domain
              [ a       owl:Class ;
                owl:unionOf (:Cohort :CohortProject)
              ] ;
      rdfs:label "has ancestry"@en ;
      rdfs:range
              [ a       rdfs:Datatype ;
                owl:oneOf
                        [ a       rdf:List ;
                          rdf:first "African American" ;
                          rdf:rest
                                  [ a       rdf:List ;
                                    rdf:first "Asian" ;
                                    rdf:rest
                                            [ a       rdf:List ;
                                              rdf:first "European" ;
                                              rdf:rest
                                                      [ a       rdf:List ;
                                                        rdf:first "Latino" ;
                                                        rdf:rest
                                                                [ a       rdf:List ;
                                                                  rdf:first "Two or More Races" ;
                                                                  rdf:rest ()
                                                                ]
                                                      ]
                                            ]
                                  ]
                        ]
              ] ;
      <http://purl.org/vocab/vann/example>
              "Cohort1 hasAncestry \"European\""@en .

:MDS-UPDRS-2
      a       owl:DatatypeProperty ;
      rdfs:comment "Movement Disorders Society Unified Parkinson's Disease Rating Scale - 2" ;
      rdfs:domain :PDDemographics ;
      rdfs:label "MDS-UPDRS-2" ;
      rdfs:range xsd:boolean .

:DigitNumberSequencing
      a       owl:DatatypeProperty ;
      rdfs:comment "A verbal task, with stimuli presented auditorily, and responses spoken by the participant." ;
      rdfs:domain :Cognitive ;
      rdfs:label "Digit Number Sequencing" ;
      rdfs:range xsd:boolean ;
      rdfs:subPropertyOf owl:topDataProperty .

:hasInclusionCriteria
      a       owl:DatatypeProperty ;
      rdfs:comment "criteria used to include cohort patients" ;
      rdfs:domain :CohortProject , :CohortGroup , :Cohort ;
      rdfs:label "has inclusion criteria" ;
      rdfs:range xsd:string .

<http://purl.org/dc/terms/description>
      a       owl:DatatypeProperty , owl:AnnotationProperty .

:SmokingPackYears
      a       owl:DatatypeProperty ;
      rdfs:comment "A \"pack year\" is defined as twenty cigarettes smoked everyday for one year" ;
      rdfs:domain :Cardiovascular ;
      rdfs:label "Smoking Pack Years" ;
      rdfs:range xsd:string ;
      rdfs:subPropertyOf owl:topDataProperty .

:Hyperlipidaemia
      a       owl:DatatypeProperty ;
      rdfs:comment "Hyperlipidaemia: High levels of lipids/cholesterol/fats in the blood" ;
      rdfs:domain :Cardiovascular ;
      rdfs:label "Hyperlipidaemia" ;
      rdfs:range xsd:boolean ;
      rdfs:subPropertyOf owl:topDataProperty .

<http://purl.org/vocab/vann/example>
      a       owl:AnnotationProperty .

:PDSS
      a       owl:DatatypeProperty ;
      rdfs:comment "Parkinson's Disease Sleep Scale" ;
      rdfs:domain :Neuropsychiatric ;
      rdfs:label "PDSS" ;
      rdfs:range xsd:boolean ;
      rdfs:subPropertyOf owl:topDataProperty .

:PD_DementiaDiagnosis
      a       owl:DatatypeProperty ;
      rdfs:domain :Cognitive ;
      rdfs:label "PD Dementia Diagnosis" ;
      rdfs:range xsd:boolean ;
      rdfs:subPropertyOf owl:topDataProperty .

:hasProjectResults
      a       owl:ObjectProperty ;
      rdfs:comment "Property to link project results to a Cohort Project" ;
      rdfs:domain :CohortProject ;
      rdfs:label "has project results" ;
      rdfs:range :DataDownload .

:InfectiousDisorder
      a       owl:Class ;
      rdfs:comment "A disease or disorder caused by the invasion of microorganisms"@en ;
      rdfs:label "Infectious Disorder"@en ;
      rdfs:subClassOf :Disorder ;
      <http://purl.org/vocab/vann/example>
              "HIV"@en .

:hasStatistics
      a       owl:ObjectProperty ;
      rdfs:comment "Property used to link a cohort with the summary statistics that may have been  produced after applying a given protocol"@en ;
      rdfs:domain :CohortProject ;
      rdfs:label "has statistics"@en ;
      rdfs:range :Dataset .

:occupation
      a       owl:DatatypeProperty ;
      rdfs:comment "Occupation of the subjects" ;
      rdfs:domain :PDDemographics ;
      rdfs:label "Occupation" ;
      rdfs:range xsd:boolean .

:hasImageAcquisitionProtocol
      a       owl:ObjectProperty ;
      rdfs:comment "Describes the acquisition protocol that was used to scan the data of a cohort"@en , "Describes the acquisition protocol that was used to scan a cohort"@en ;
      rdfs:domain :Cohort ;
      rdfs:domain
              [ a       owl:Class ;
                owl:unionOf (:Cohort :CohortGroup :CohortProject)
              ] ;
      rdfs:domain
              [ a       owl:Class ;
                owl:unionOf (:Cohort :CohortGroup :CohortProject)
              ] ;
      rdfs:domain
              [ a       owl:Class ;
                owl:unionOf (:Cohort :CohortGroup :CohortProject)
              ] ;
      rdfs:domain
              [ a       owl:Class ;
                owl:unionOf (:Cohort :CohortGroup :CohortProject)
              ] ;
      rdfs:domain
              [ a       owl:Class ;
                owl:unionOf (:Cohort :CohortGroup :CohortProject)
              ] ;
      rdfs:label "has image acquisition protocol"@en , "has acquisition protocol"@en ;
      rdfs:range :ImageAcquisitionProtocol ;
      <http://purl.org/vocab/vann/example>
              "Cohort1 hasImageAcquisitionProtocol AcquisitionProtocol1"@en , "Cohort1 hasAcquisitionProtocol AcquiPro3"@en .

:hasAffiliate
      a       owl:ObjectProperty ;
      rdfs:comment "Describes the organization's affiliates"@en , "Points to the person who is an affiliate of an organization"@en ;
      rdfs:domain :Organization ;
      rdfs:label "has affiliate"@en ;
      rdfs:range :Person ;
      rdfs:subPropertyOf <http://xmlns.com/foaf/0.1/member> ;
      <http://purl.org/vocab/vann/example>
              "Harvard hasAffiliate JohnSmith"@en , "HarvardU hasAffiliate JohnSmith"@en .

:MDS-UPDRS-1
      a       owl:DatatypeProperty ;
      rdfs:comment "Movement Disorders Society Unified Parkinson's Disease Rating Scale - 1" ;
      rdfs:domain :PDDemographics ;
      rdfs:label "MDS-UPDRS-1" ;
      rdfs:range xsd:boolean .

:mildCognitiveImpairmentDiagnosis
      a       owl:DatatypeProperty ;
      rdfs:domain :Cognitive ;
      rdfs:label "Mild Cognitive Impairment Diagnosis" ;
      rdfs:range xsd:boolean ;
      rdfs:subPropertyOf owl:topDataProperty .

:hasDescription
      a       owl:DatatypeProperty ;
      rdfs:comment "Description of an item" ;
      rdfs:domain :Dataset ;
      rdfs:label "has description" ;
      rdfs:range xsd:string ;
      rdfs:subPropertyOf <https://schema.org/description> .

:hasTotalNumberOfParticipants
      a       owl:DatatypeProperty ;
      rdfs:comment "Describes the total number of participants in the cohort"@en ;
      rdfs:domain :Cohort ;
      rdfs:label "has total number of participants"@en ;
      rdfs:range xsd:positiveInteger ;
      <http://purl.org/vocab/vann/example>
              "Cohort1 hasTotalNumberOfParticipants 500 --> Cohort1 is made up of approximately 500 patients"@en .

:hasGivenName
      a       owl:DatatypeProperty ;
      rdfs:comment "The given name of some person."@en ;
      rdfs:domain :Person ;
      rdfs:label "has given name"@en ;
      rdfs:range xsd:string ;
      rdfs:subPropertyOf <http://xmlns.com/foaf/0.1/givenName> ;
      <http://www.linkedmodel.org/schema/vaem#rationale>
              "Property added to restrict the domain to enigma:Person. This is done for facilitating the interaction with the wiki interface"@en .

:SignificantGeneralMedicalCondition
      a       owl:Class ;
      rdfs:comment "Blanket term ecompassing serious medical condtions"@en ;
      rdfs:label "Significant General Medical Condition"@en ;
      rdfs:subClassOf :Disorder ;
      <http://purl.org/vocab/vann/example>
              "Cancer"@en .

:VascularDisorder
      a       owl:Class ;
      rdfs:comment "Disorder which affects the body's network of blood vessels"@en ;
      rdfs:label "Vascular Disorder"@en ;
      rdfs:subClassOf :Disorder ;
      <http://purl.org/vocab/vann/example>
              "Coronary Artery Disease"@en .

:otherEnvironmentalFactors
      a       owl:DatatypeProperty ;
      rdfs:comment "Any other environmental factors relating to a PD cohort" ;
      rdfs:domain :PDDemographics ;
      rdfs:label "Other Environmental Factors" ;
      rdfs:range xsd:string .

:ReyAuditoryVerbalLearningTest
      a       owl:DatatypeProperty ;
      rdfs:comment "Assessment designed to evaluate verbal memory in patients, 16 years of age and older" ;
      rdfs:domain :Cognitive ;
      rdfs:label "Rey Auditory Verbal Learning Test" ;
      rdfs:range xsd:boolean ;
      rdfs:subPropertyOf owl:topDataProperty .

:comorbidities
      a       owl:DatatypeProperty ;
      rdfs:comment "If other comorbidities were measured in subjects" ;
      rdfs:domain :PDDemographics ;
      rdfs:label "comorbidities" ;
      rdfs:range xsd:boolean .

:ESS  a       owl:DatatypeProperty ;
      rdfs:comment "Epworth Sleepiness Scale" ;
      rdfs:domain :Neuropsychiatric ;
      rdfs:label "ESS" ;
      rdfs:range xsd:boolean ;
      rdfs:subPropertyOf owl:topDataProperty .

:BentonJudgmentOfLineOrientation
      a       owl:DatatypeProperty ;
      rdfs:comment "The Benton Judgment of Line Orientation (JLO) test is a standardized neuropsychological test that measures visuospatial judgment and perception." ;
      rdfs:domain :Cognitive ;
      rdfs:label "Benton Judgment Of Line Orientation" ;
      rdfs:range xsd:boolean ;
      rdfs:subPropertyOf owl:topDataProperty .

:WAIS_4_PerceptualReasoning
      a       owl:DatatypeProperty ;
      rdfs:comment "This index reflects an individual’s ability to accurately interpret, organize and think with visual information on the WAIS 4 (Wechsler Adult Intelligence Scale-IV) scale" ;
      rdfs:domain :Cognitive ;
      rdfs:label "WAIS 4 Perceptual Reasoning Index" ;
      rdfs:range xsd:boolean ;
      rdfs:subPropertyOf owl:topDataProperty .

:has_cognitive
      a       owl:ObjectProperty ;
      rdfs:comment "Describes cogitive covariate properties specific to the PD working group" ;
      rdfs:domain :Cohort ;
      rdfs:label "has cognitive" ;
      rdfs:range :Cognitive ;
      rdfs:subPropertyOf owl:topObjectProperty .

:SAPS-PD
      a       owl:DatatypeProperty ;
      rdfs:comment "Schedule for Assessment of Positive Symptoms - PD" ;
      rdfs:domain :Neuropsychiatric ;
      rdfs:label "SAPS-PD" ;
      rdfs:range xsd:boolean ;
      rdfs:subPropertyOf owl:topDataProperty .

:hasDataProcessingProtocol
      a       owl:ObjectProperty ;
      rdfs:comment "Describes which data processing protocol was used in a project"@en ;
      rdfs:domain :Project ;
      rdfs:label "uses data processing protocol"@en ;
      rdfs:range :DataProcessingProtocol .

:SentencesConstruction
      a       owl:DatatypeProperty ;
      rdfs:domain :Cognitive ;
      rdfs:label "Sentences Construction" ;
      rdfs:range xsd:boolean ;
      rdfs:subPropertyOf owl:topDataProperty .

:PhonologicalAndSemanticVerbalFluencyTest
      a       owl:DatatypeProperty ;
      rdfs:domain :Cognitive ;
      rdfs:label "Phonological (PVF) and Semantic (SVF) Verbal Fluency Test" ;
      rdfs:range xsd:boolean ;
      rdfs:subPropertyOf owl:topDataProperty .

:hasDataCollectionPeriodStart
      a       owl:DatatypeProperty ;
      rdfs:comment "Describes the start year of the data collection period of the cohort"@en ;
      rdfs:domain
              [ a       owl:Class ;
                owl:unionOf (:Cohort :CohortGroup :CohortProject)
              ] ;
      rdfs:label "has data collection period start"@en ;
      rdfs:range xsd:gYear ;
      <http://purl.org/vocab/vann/example>
              "Cohort1 hasDataCollectionPeriodStart 2005"@en .

:Cohort
      a       owl:Class ;
      rdfs:comment """A group of individuals studied by a working group, limited by certain inclusion and exclusion criteria.

Cohort Groups: COHORT_grp_NAME
Example: STELLENBOCH_grp_CN for the control group

Cohort Projects: COHORT_proj_NAME
Example: STELLENBOCH_proj_FS for the Freesurfer project"""@en , "A group of individuals studied by a working group, limited by certain inclusion and exclusion criteria"@en ;
      rdfs:label "Cohort"@en ;
      <http://purl.org/vocab/vann/example>
              "ADNI: Alzheimer’s Disease Neuroimaging Initiative"@en .

:Cardiovascular
      a       owl:Class ;
      rdfs:comment "Cardiovascular Covariates measured by each PD cohort" ;
      rdfs:label "Cardiovascular" .

:QUIP-rs
      a       owl:DatatypeProperty ;
      rdfs:comment "Questionnaire for Impulsive-Compulsive Disorders in Parkinson's Disease–Rating Scale" ;
      rdfs:domain :Neuropsychiatric ;
      rdfs:label "QUIP-rs" ;
      rdfs:range xsd:boolean ;
      rdfs:subPropertyOf owl:topDataProperty .

:isPartOfCohort
      a       owl:ObjectProperty ;
      rdfs:comment "Property that indicates the cohort groups and cohort projects which are part of a cohort"@en ;
      rdfs:domain
              [ a       owl:Class ;
                owl:unionOf (:Cohort :CohortGroup :CohortProject)
              ] ;
      rdfs:domain
              [ a       owl:Class ;
                owl:unionOf (:Cohort :CohortGroup :CohortProject)
              ] ;
      rdfs:domain
              [ a       owl:Class ;
                owl:unionOf (:Cohort :CohortGroup :CohortProject)
              ] ;
      rdfs:domain
              [ a       owl:Class ;
                owl:unionOf (:Cohort :CohortGroup :CohortProject)
              ] ;
      rdfs:domain
              [ a       owl:Class ;
                owl:unionOf (:Cohort :CohortGroup :CohortProject)
              ] ;
      rdfs:label "is part of cohort"@en ;
      rdfs:range :Cohort .

:WOQ  a       owl:DatatypeProperty ;
      rdfs:comment "Wearing-Off Questionnaires WOQ-9, WOQ-19, WOQ-32" ;
      rdfs:domain :Neuropsychiatric ;
      rdfs:label "WOQ" ;
      rdfs:range xsd:string ;
      rdfs:subPropertyOf owl:topDataProperty .

<http://purl.org/ontology/bibo/AcademicArticle>
      a       owl:Class ;
      rdfs:isDefinedBy <http://purl.org/ontology/bibo/AcademicArticle> ;
      owl:equivalentClass :AcademicArticle .

:HistoryOfIschamicHeartDisease
      a       owl:DatatypeProperty ;
      rdfs:comment "Ischamic Heart Disease: aka Coronary Heart Disease, heart problems caused by narrowed arteries that supply blood to the heart" ;
      rdfs:domain :Cardiovascular ;
      rdfs:label "History of Ischamic Heart Disease" ;
      rdfs:range xsd:boolean ;
      rdfs:subPropertyOf owl:topDataProperty .

:TrialMakingTestA-B
      a       owl:DatatypeProperty ;
      rdfs:domain :Cognitive ;
      rdfs:label "Trial Making Test A-B" ;
      rdfs:range xsd:boolean ;
      rdfs:subPropertyOf owl:topDataProperty .

:hasCovariates
      a       owl:ObjectProperty ;
      rdfs:domain :Cohort ;
      rdfs:label "has covariates" ;
      rdfs:range :Covariates .

:hasOrcidId
      a       owl:ObjectProperty ;
      rdfs:comment "ORCID Id of a Person"@en ;
      rdfs:domain :Person ;
      rdfs:label "has ORCID Id"@en ;
      rdfs:subPropertyOf <http://vivoweb.org/ontology/core#orcidId> ;
      <http://www.linkedmodel.org/schema/vaem#rationale>
              "Property added to facilitate interaction with the wiki, making domains and ranges explicit"@en .

:OtherRelevantCardiovascularMedications
      a       owl:DatatypeProperty ;
      rdfs:comment "e.g. antihypertensives, cholesterol lowering drugs, aspirin, steriods" ;
      rdfs:domain :Cardiovascular ;
      rdfs:label "Other Relevant Cardiovascular Medications" ;
      rdfs:range xsd:string ;
      rdfs:subPropertyOf owl:topDataProperty .

:has_neuropsychiatric
      a       owl:ObjectProperty ;
      rdfs:comment "Describes the neuropsychiatric covariates of the PD working group" ;
      rdfs:domain :Cohort ;
      rdfs:label "has neuropsychiatric" ;
      rdfs:range :Neuropsychiatric ;
      rdfs:subPropertyOf owl:topObjectProperty .

:hasDataType
      a       owl:ObjectProperty ;
      rdfs:comment "Describes the data types that a cohort or project collected"@en ;
      rdfs:domain
              [ a       owl:Class ;
                owl:unionOf (:Cohort :Project)
              ] ;
      rdfs:domain
              [ a       owl:Class ;
                owl:unionOf (:Cohort :Project)
              ] ;
      rdfs:domain
              [ a       owl:Class ;
                owl:unionOf (:Cohort :Project)
              ] ;
      rdfs:domain
              [ a       owl:Class ;
                owl:unionOf (:Cohort :Project)
              ] ;
      rdfs:domain
              [ a       owl:Class ;
                owl:unionOf (:Cohort :Project)
              ] ;
      rdfs:domain
              [ a       owl:Class ;
                owl:unionOf (:Cohort :Project)
              ] ;
      rdfs:label "has data type"@en ;
      rdfs:range :DataType ;
      <http://purl.org/vocab/vann/example>
              "BipolarProject hasDataType MRIImage"@en , "Cohort1 hasDataType dataType1"@en .

:Other_Depression_Severity_Tests
      a       owl:DatatypeProperty ;
      rdfs:comment "Test names for other depression severity scales/measures" ;
      rdfs:domain :Neuropsychiatric ;
      rdfs:label "Other Depression Severity Tests" ;
      rdfs:range xsd:boolean .

:SCOPA-Psychiatric
      a       owl:DatatypeProperty ;
      rdfs:comment "Scales for Outcomes in Parkinson's Disease - Psychiatric" ;
      rdfs:domain :PDDemographics ;
      rdfs:label "SCOPA-Psychiatric" ;
      rdfs:range xsd:boolean .

:hasControlGroup
      a       owl:ObjectProperty ;
      rdfs:comment "Describes the control group of a cohort"@en ;
      rdfs:domain
              [ a       owl:Class ;
                owl:unionOf (:Cohort :CohortProject)
              ] ;
      rdfs:domain
              [ a       owl:Class ;
                owl:unionOf (:Cohort :CohortProject)
              ] ;
      rdfs:domain
              [ a       owl:Class ;
                owl:unionOf (:Cohort :CohortProject)
              ] ;
      rdfs:domain
              [ a       owl:Class ;
                owl:unionOf (:Cohort :CohortProject)
              ] ;
      rdfs:domain
              [ a       owl:Class ;
                owl:unionOf (:Cohort :CohortProject)
              ] ;
      rdfs:label "has control group"@en ;
      rdfs:range :CohortGroup ;
      rdfs:subPropertyOf :hasCohortGroup ;
      <http://purl.org/vocab/vann/example>
              "BipolarCohort hasControlGroup BipolarControlGroup"@en .

:has_latitude
      a       owl:DatatypeProperty ;
      rdfs:comment "The latitude of the cohort" ;
      rdfs:domain :Location ;
      rdfs:label "has latitude" ;
      rdfs:range xsd:float .

:AS   a       owl:DatatypeProperty ;
      rdfs:comment "Starkstein's Apathy Scale" ;
      rdfs:domain :Neuropsychiatric ;
      rdfs:label "AS" ;
      rdfs:range xsd:boolean ;
      rdfs:subPropertyOf owl:topDataProperty .

:author
      a       owl:ObjectProperty ;
      rdfs:comment "Property to describe the author of a publication in the context of an ENIGMA project"@en ;
      rdfs:domain :AcademicArticle ;
      rdfs:label "author"@en ;
      rdfs:range :Person ;
      rdfs:subPropertyOf <http://purl.org/dc/terms/creator> .

:isPartOfCohortGroup
      a       owl:ObjectProperty ;
      rdfs:comment "Property that indicates the projects which are part of a cohort group"@en ;
      rdfs:domain :CohortProject ;
      rdfs:label "is part of cohort group"@en ;
      rdfs:range :CohortGroup .

:Person
      a       owl:Class ;
      rdfs:comment "Individual involved with the cohort"@en ;
      rdfs:label "Person"@en ;
      <http://purl.org/vocab/vann/example>
              "Theo van Erp"@en .

:hasProposalForm
      a       owl:DatatypeProperty ;
      rdfs:comment "Describes the approved proposal form link of a project"@en ;
      rdfs:domain :Project ;
      rdfs:label "has approved proposal form"@en ;
      rdfs:range xsd:anyURI ;
      <http://purl.org/vocab/vann/example>
              "Project1 hasProposalForm www.proposalformexample.com"@en .

:usesEncodingFormat
      a       owl:DatatypeProperty ;
      rdfs:comment "Encoding format of an item"@en ;
      rdfs:domain :DataDownload ;
      rdfs:label "uses encoding format"@en ;
      rdfs:range xsd:string ;
      rdfs:subPropertyOf <https://schema.org/encodingFormat> .

:HRDS
      a       owl:DatatypeProperty ;
      rdfs:comment "Hamilton Rating Scale for Depression (or HAM-D)" ;
      rdfs:domain :Neuropsychiatric ;
      rdfs:label "HRDS" ;
      rdfs:range xsd:boolean ;
      rdfs:subPropertyOf owl:topDataProperty .

:RSGE-PD
      a       owl:DatatypeProperty ;
      rdfs:domain :PDDemographics ;
      rdfs:label "RSGE-PD" ;
      rdfs:range xsd:boolean .

:AgeOfPDOnset
      a       owl:DatatypeProperty ;
      rdfs:comment "Age of Onset of Parkinson's Disease" ;
      rdfs:domain :PDDemographics ;
      rdfs:label "Age of Onset PD" ;
      rdfs:range xsd:boolean .

<https://schema.org/encodingFormat>
      a       owl:DatatypeProperty ;
      rdfs:isDefinedBy <https://schema.org/> .

<https://schema.org/distribution>
      a       owl:ObjectProperty ;
      rdfs:isDefinedBy <https://schema.org/> .

:GDI  a       owl:DatatypeProperty ;
      rdfs:comment "Geriatric Depression Index" ;
      rdfs:domain :Neuropsychiatric ;
      rdfs:label "GDI" ;
      rdfs:range xsd:boolean ;
      rdfs:subPropertyOf owl:topDataProperty .

:hasAge_Mean
      a       owl:DatatypeProperty ;
      rdfs:comment "Describes the mean age of the cohort"@en ;
      rdfs:domain
              [ a       owl:Class ;
                owl:unionOf (:CohortGroup :CohortProject :Covariates)
              ] ;
      rdfs:label "has mean age"@en ;
      rdfs:range xsd:double ;
      <http://purl.org/vocab/vann/example>
              "Cohort1 hasAge_Mean 21.0"@en .

:Cancer
      a       owl:Class ;
      rdfs:comment "A disease characterized by abnormal cell division and growth"@en ;
      rdfs:label "Cancer"@en ;
      rdfs:subClassOf :Disorder ;
      <http://purl.org/vocab/vann/example>
              "CNS Cancer"@en .

:UPSIT
      a       owl:DatatypeProperty ;
      rdfs:comment "University of Pennsylvania Smell Identification Test for Parkinson's Disease" ;
      rdfs:domain :PDDemographics ;
      rdfs:label "UPSIT" ;
      rdfs:range xsd:boolean .

:hasAge_Minimum
      a       owl:DatatypeProperty ;
      rdfs:comment "Describes inclusion criteria for minimum age of participants in a Cohort, CohortProject or CohortGroup"@en ;
      rdfs:domain
              [ a       owl:Class ;
                owl:unionOf (:Cohort :CohortGroup :CohortProject :Covariates)
              ] ;
      rdfs:label "has minimum age"@en ;
      rdfs:range xsd:positiveInteger ;
      <http://purl.org/vocab/vann/example>
              "CohortGroup1 hasAge_Minimum 12"@en .

:hasDiagnosticInstrument
      a       owl:ObjectProperty ;
      rdfs:comment "Describes what instrument is used to diagnose the members of the cohort"@en ;
      rdfs:domain
              [ a       owl:Class ;
                owl:unionOf (:CohortGroup :CohortProject)
              ] ;
      rdfs:domain
              [ a       owl:Class ;
                owl:unionOf (:CohortGroup :CohortProject)
              ] ;
      rdfs:domain
              [ a       owl:Class ;
                owl:unionOf (:CohortGroup :CohortProject)
              ] ;
      rdfs:domain
              [ a       owl:Class ;
                owl:unionOf (:CohortGroup :CohortProject)
              ] ;
      rdfs:domain
              [ a       owl:Class ;
                owl:unionOf (:CohortGroup :CohortProject)
              ] ;
      rdfs:label "has diagnostic instrument"@en ;
      rdfs:range :DiagnosticInstrument ;
      <http://purl.org/vocab/vann/example>
              "Cohort1 hasDiagnosticInstrument miniInternationalNeuropychiatricInterview --> The members of Cohort1 are diagnosed with Mini International Neuropychiatric Interview"@en .

:dx   a       owl:DatatypeProperty ;
      rdfs:comment "Diagnosis Group" ;
      rdfs:domain :PDDemographics ;
      rdfs:range xsd:boolean .

:age  a       owl:DatatypeProperty ;
      rdfs:comment "age of participants" ;
      rdfs:domain :PDDemographics ;
      rdfs:label "age" ;
      rdfs:range xsd:boolean .

:UM-PDHQ
      a       owl:DatatypeProperty ;
      rdfs:comment "University of Miami Parkinson's Disease Hallucinations Questionnaire" ;
      rdfs:domain :Neuropsychiatric ;
      rdfs:label "UM-PDHQ" ;
      rdfs:range xsd:boolean ;
      rdfs:subPropertyOf owl:topDataProperty .

:hasDate_TargetEnd
      a       owl:DatatypeProperty ;
      rdfs:comment "Describes the end date of the target period of the project"@en ;
      rdfs:domain :Project ;
      rdfs:label "has target end date"@en ;
      rdfs:range xsd:date ;
      <http://purl.org/vocab/vann/example>
              "BipolarProject hasDate_TargetEnd 2020-03-12"@en .

:has_country
      a       owl:DatatypeProperty ;
      rdfs:comment "Country in which cohort is located" ;
      rdfs:domain :Location ;
      rdfs:label "has country" ;
      rdfs:range xsd:string .

:hasDistribution
      a       owl:ObjectProperty ;
      rdfs:comment "Indicates a downloadable form of a dataset at a specific location" ;
      rdfs:domain :Dataset ;
      rdfs:label "has distribution" ;
      rdfs:range :DataDownload ;
      rdfs:subPropertyOf <https://schema.org/distribution> .

:TowerOfHanoi
      a       owl:DatatypeProperty ;
      rdfs:comment "This task seeks to measure high-order cognitive problem solving and learning of complex cognitive procedures, providing information about the cognitive abilities mainly related to executive functions such as planning, visual imagery, abstract thinking, working memory and self-monitoring." ;
      rdfs:domain :Cognitive ;
      rdfs:label "Tower Of Hanoi" ;
      rdfs:range xsd:boolean ;
      rdfs:subPropertyOf owl:topDataProperty .

<http://purl.org/dc/terms/creator>
      a       owl:AnnotationProperty , owl:ObjectProperty ;
      rdfs:isDefinedBy <http://purl.org/dc/terms/creator> .

:PDMedicationUseLifetime
      a       owl:DatatypeProperty ;
      rdfs:comment "Describes if the patient used PD medication during their lifetime" ;
      rdfs:domain :PDDemographics ;
      rdfs:label "PD Medication Use Lifetime" ;
      rdfs:range xsd:boolean .

:WAIS_4_WorkingMemory
      a       owl:DatatypeProperty ;
      rdfs:comment "This index reflects an individual’s ability to take in and hold information in immediate awareness and then perform a mental operation on that information on the WAIS 4 (Wechsler Adult Intelligence Scale-IV) scale" ;
      rdfs:domain :Cognitive ;
      rdfs:label "WAIS 4 Working Memory Index" ;
      rdfs:range xsd:boolean ;
      rdfs:subPropertyOf owl:topDataProperty .

:StandingBloodPressure
      a       owl:DatatypeProperty ;
      rdfs:comment "Standing blood pressure after standing for 3 minutes" ;
      rdfs:domain :Cardiovascular ;
      rdfs:label "Standing Blood Pressure" ;
      rdfs:range xsd:boolean ;
      rdfs:subPropertyOf owl:topDataProperty .

:LEDDScore
      a       owl:DatatypeProperty ;
      rdfs:comment "Levodopa Equivalent Doses used to treat Parkinson's Disease" ;
      rdfs:domain :PDDemographics ;
      rdfs:label "LEDD Score" ;
      rdfs:range xsd:boolean .

:MDS-UPDRS-4
      a       owl:DatatypeProperty ;
      rdfs:comment "Movement Disorders Society Unified Parkinson's Disease Rating Scale - 4" ;
      rdfs:domain :PDDemographics ;
      rdfs:label "MDS-UPDRS-4" ;
      rdfs:range xsd:boolean .

:isPartOfCohortProject
      a       owl:ObjectProperty ;
      rdfs:comment "Property that indicates the cohort groups which are part of a cohort project"@en ;
      rdfs:domain :CohortGroup ;
      rdfs:label "is part of cohort project"@en ;
      rdfs:range :CohortProject .

:HoehnAndYahrStage
      a       owl:DatatypeProperty ;
      rdfs:comment "The Stage for Hoehn and Yahr scales used for PD cohorts" ;
      rdfs:domain :PDDemographics ;
      rdfs:label "Hoehn and Yahr Stage" ;
      rdfs:range xsd:boolean .

:PDMedicationUseCurrent
      a       owl:DatatypeProperty ;
      rdfs:comment "Describes if the patient is currently using PD medication" ;
      rdfs:domain :PDDemographics ;
      rdfs:label "PD Medication Use Current" ;
      rdfs:range xsd:boolean .

:DigitSpan
      a       owl:DatatypeProperty ;
      rdfs:comment "Digit Span is a test of verbal short-term memory." ;
      rdfs:domain :Cognitive ;
      rdfs:label "Digit Span" ;
      rdfs:range xsd:boolean ;
      rdfs:subPropertyOf owl:topDataProperty .

:Smoking
      a       owl:DatatypeProperty ;
      rdfs:domain :Cardiovascular ;
      rdfs:label "Smoking" ;
      rdfs:range xsd:boolean ;
      rdfs:subPropertyOf owl:topDataProperty .

:OtherMedUseCurrent
      a       owl:DatatypeProperty ;
      rdfs:comment "Other medication currently used" ;
      rdfs:domain :PDDemographics ;
      rdfs:label "Other Medication Use Current" ;
      rdfs:range xsd:boolean .

:Hypertension
      a       owl:DatatypeProperty ;
      rdfs:comment "Hypertension: high blood pressure" ;
      rdfs:domain :Cardiovascular ;
      rdfs:label "Hypertension" ;
      rdfs:range xsd:boolean ;
      rdfs:subPropertyOf owl:topDataProperty .

:PPRS
      a       owl:DatatypeProperty ;
      rdfs:comment "Parkinson's Psychosis Rating Scale" ;
      rdfs:domain :Neuropsychiatric ;
      rdfs:label "PPRS" ;
      rdfs:range xsd:boolean ;
      rdfs:subPropertyOf owl:topDataProperty .

:QPE  a       owl:DatatypeProperty ;
      rdfs:comment "Questionnaire for Psychotic Experiences" ;
      rdfs:domain :Neuropsychiatric ;
      rdfs:label "QPE" ;
      rdfs:range xsd:boolean ;
      rdfs:subPropertyOf owl:topDataProperty .

:WAIS_4_ProcessingSpeed
      a       owl:DatatypeProperty ;
      rdfs:comment "This index reflects an individual’s ability to process simple or routine visual information quickly and efficiently on the WAIS 4 (Wechsler Adult Intelligence Scale-IV) scale." ;
      rdfs:domain :Cognitive ;
      rdfs:label "WAIS 4 Processing Speed" ;
      rdfs:range xsd:boolean ;
      rdfs:subPropertyOf owl:topDataProperty .
