@prefix :        <https://w3id.org/enigma#> .
@prefix owl:     <http://www.w3.org/2002/07/owl#> .
@prefix rdf:     <http://www.w3.org/1999/02/22-rdf-syntax-ns#> .
@prefix xml:     <http://www.w3.org/XML/1998/namespace> .
@prefix xsd:     <http://www.w3.org/2001/XMLSchema#> .
@prefix rdfs:    <http://www.w3.org/2000/01/rdf-schema#> .

:hasName_Short
      a       owl:DatatypeProperty ;
      rdfs:comment "A short name for the working group, in case the working group name is too long"@en ;
      rdfs:domain :WorkingGroup ;
      rdfs:label "has short name"@en ;
      rdfs:range xsd:string ;
      rdfs:subPropertyOf <http://purl.org/dc/terms/title> ;
      <http://purl.org/vocab/vann/example>
              "SchizophreniaWG hasName_Short SZWG"@en .

:isPartOfWorkingGroup
      a       owl:ObjectProperty ;
      rdfs:comment "Property that indicates the cohorts which are a part of a working group"@en ;
      rdfs:domain
              [ a       owl:Class ;
                owl:unionOf (:Cohort :CohortGroup :CohortProject)
              ] ;
      rdfs:label "is part of working group"@en ;
      rdfs:range :WorkingGroup .

:rationale
      a       owl:AnnotationProperty .

<http://www.w3.org/2006/vcard/ns#locality>
      a       owl:DatatypeProperty ;
      rdfs:comment "The locality (e.g. city or town) associated with the address of the object"@en ;
      rdfs:domain :Address ;
      rdfs:isDefinedBy <http://www.w3.org/2006/vcard/ns> ;
      rdfs:label "locality"@en ;
      rdfs:range xsd:string .

:antiepilepticUse_Lifetime
      a       owl:DatatypeProperty ;
      rdfs:comment "Describes whether the subject's use of antiepileptics during their lifetime is specified." ;
      rdfs:domain :Covariates ;
      rdfs:label "antiepileptic use lifetime" ;
      rdfs:range xsd:boolean ;
      rdfs:subPropertyOf :medicationSomaticProperty .

:hasWorkingGroupMember
      a       owl:ObjectProperty ;
      rdfs:comment "Describes who the members of the working group are"@en , "Describes what working group a person is a member of"@en ;
      rdfs:domain :WorkingGroup ;
      rdfs:label "has working group member"@en ;
      rdfs:range :Person ;
      rdfs:subPropertyOf <http://xmlns.com/foaf/0.1/member> ;
      <http://purl.org/vocab/vann/example>
              "BipolarWorkingGroup hasWorkingGroupMember JohnSmith"@en , "BipolarWorkingGroup hasWorkingGroupMember JohnSmith --> The bipolar working group has John Smith as a member"@en .

<http://www.linkedmodel.org/schema/vaem#rationale>
      a       owl:AnnotationProperty .

<http://www.w3.org/2006/vcard/ns#Address>
      a       owl:Class ;
      rdfs:isDefinedBy <http://www.w3.org/2006/vcard/ns> ;
      rdfs:label "Address"@en .

:atypicalAntipsychoticUse_Lifetime
      a       owl:DatatypeProperty ;
      rdfs:comment "Describes if the subject's use of 2nd generation (atypical) antipsychotics during their lifetime is specified." ;
      rdfs:domain :Covariates ;
      rdfs:label "atypical antipsychotic use lifetime" ;
      rdfs:range xsd:boolean ;
      rdfs:subPropertyOf :medicationSomaticProperty .

<http://www.w3.org/2006/vcard/ns#street-address>
      a       owl:DatatypeProperty .

:hasExclusionCriteria
      a       owl:DatatypeProperty ;
      rdfs:comment "Criteria used to exclude cohort patients"@en ;
      rdfs:domain
              [ a       owl:Class ;
                owl:unionOf (:Cohort :CohortGroup :CohortProject)
              ] ;
      rdfs:label "has exclusion criteria"@en ;
      rdfs:range xsd:string .

:contributor
      a       owl:ObjectProperty ;
      rdfs:comment "Property that indicates who is a contributor to a project or cohort"@en ;
      rdfs:domain
              [ a       owl:Class ;
                owl:unionOf (:AcademicArticle :Cohort :Project)
              ] ;
      rdfs:label "contributor"@en ;
      rdfs:range :Person ;
      rdfs:subPropertyOf <http://purl.org/dc/terms/contributor> ;
      <http://www.linkedmodel.org/schema/vaem#rationale>
              "Property added to restrict the domain to projects, cohorts and academic articles. This is done for facilitating the interaction with the wiki interface"@en .

:BIS_TotalScore
      a       owl:DatatypeProperty ;
      rdfs:comment "Describes whether the Behavioral Inhibition System subscale score on the BIS/BAS is specified." ;
      rdfs:domain :Covariates ;
      rdfs:label "BIS total score" ;
      rdfs:range xsd:boolean ;
      rdfs:subPropertyOf :scoreProperty .

:RespiratoryDisorder
      a       owl:Class ;
      rdfs:comment "Disorders which affect the respiratory system"@en ;
      rdfs:label "Respiratory Disorder"@en ;
      rdfs:subClassOf :Disorder ;
      <http://purl.org/vocab/vann/example>
              "Asthma"@en .

<http://xmlns.com/foaf/0.1/Person>
      a       owl:Class ;
      rdfs:isDefinedBy "http://xmlns.com/foaf/0.1/"@en ;
      owl:equivalentClass :Person .

:somaticIllness_type
      a       owl:DatatypeProperty ;
      rdfs:comment "Describes the subject's somatic illness type." ;
      rdfs:domain :Covariates ;
      rdfs:label "somatic illness type" ;
      rdfs:range xsd:string ;
      rdfs:subPropertyOf :medicationSomaticProperty .

:Protocol
      a       owl:Class ;
      rdfs:comment "An image processing or genetic analysis protocol used to extract brain feature data"@en ;
      rdfs:label "Protocol"@en ;
      <http://purl.org/vocab/vann/example>
              "ENIGMA-Sulci Protocol"@en .

:panicDisorder_Lifetime
      a       owl:DatatypeProperty ;
      rdfs:comment "Describes if the subject had Panic Disorder during their lifetime." ;
      rdfs:domain :Covariates ;
      rdfs:label "panic disorder lifetime" ;
      rdfs:range xsd:boolean ;
      rdfs:subPropertyOf :psychopathologicalProperty .

:GAD_Current
      a       owl:DatatypeProperty ;
      rdfs:comment "Describes if the subject currently has Generalized Anxiety Disorder." ;
      rdfs:domain :Covariates ;
      rdfs:label "GAD current" ;
      rdfs:range xsd:boolean ;
      rdfs:subPropertyOf :psychopathologicalProperty .

:usesScanner
      a       owl:DatatypeProperty ;
      rdfs:comment "Describes the scanner used by the cohort"@en ;
      rdfs:domain
              [ a       owl:Class ;
                owl:unionOf (:Cohort :CohortGroup :CohortProject)
              ] ;
      rdfs:label "uses scanner"@en ;
      rdfs:range xsd:string ;
      <http://purl.org/vocab/vann/example>
              "SZCohort usesScanner \"1.5T-GE-Signa\""@en .

:typicalAntipsychoticUse_Current
      a       owl:DatatypeProperty ;
      rdfs:comment "Describes whether the subject's use of 1st generation (typical) antipsychotics at time of scan is specified." ;
      rdfs:domain :Covariates ;
      rdfs:label "typical antipsychotic use current" ;
      rdfs:range xsd:boolean ;
      rdfs:subPropertyOf :medicationSomaticProperty .

<https://schema.org/name>
      a       owl:DatatypeProperty ;
      rdfs:isDefinedBy <https://schema.org> .

:BD_Stage
      a       owl:DatatypeProperty ;
      rdfs:comment "Describes whether the subject's current Bipolar Disorder stage (first episode, recurrent episodes, no BD, and NA = no information available) is specified." ;
      rdfs:domain :Covariates ;
      rdfs:label "BD stage" ;
      rdfs:range xsd:boolean ;
      rdfs:subPropertyOf :psychopathologicalProperty .

:hasWorkingGroupChair
      a       owl:ObjectProperty ;
      rdfs:comment "Describes the working groups that someone is a chair of"@en , "Describes who the chairs of a working group are"@en ;
      rdfs:domain :WorkingGroup ;
      rdfs:label "has working group chair"@en ;
      rdfs:range :Person ;
      rdfs:subPropertyOf :hasWorkingGroupMember ;
      <http://purl.org/vocab/vann/example>
              "BipolarWorkingGroup hasWorkingGroupChair JohnSmith"@en , "SZWorkingGroup hasWorkingGroupChair JohnSmith"@en .

<https://schema.org/contentUrl>
      a       owl:DatatypeProperty ;
      rdfs:isDefinedBy <https://schema.org/> .

:OCD_AgeofOnset
      a       owl:DatatypeProperty ;
      rdfs:comment "Describes whether the age of onset of the subject's Obsessive Compulsive Disorder is specified." ;
      rdfs:domain :Covariates ;
      rdfs:label "OCD age of onset" ;
      rdfs:range xsd:boolean ;
      rdfs:subPropertyOf :psychopathologicalProperty .

:parent_SocioeconomicStatusScale
      a       owl:DatatypeProperty ;
      rdfs:comment "The scale used in measuring a parent(s) socioeconomic status." ;
      rdfs:domain :Covariates ;
      rdfs:label "parent socioeconomic status scale" ;
      rdfs:range xsd:string ;
      rdfs:subPropertyOf :demographicProperty .

:checksum
      a       owl:DatatypeProperty ;
      rdfs:comment "checksum of data file to check if there are modifications"^^xsd:string ;
      rdfs:domain :DataDownload ;
      rdfs:label "checksum"^^xsd:string ;
      rdfs:range xsd:string .

:DataDownload
      a       owl:Class ;
      rdfs:comment "Dataset in downloadable form"@en ;
      rdfs:label "Data Download"@en ;
      rdfs:subClassOf <http://schema.org/DataDownload> .

<http://xmlns.com/foaf/0.1/member>
      a       owl:ObjectProperty ;
      rdfs:comment "Indicates member of a group"^^xsd:string ;
      rdfs:isDefinedBy <http://xmlns.com/foaf/0.1/member> , <http://xmlns.com/foaf/0.1/> ;
      rdfs:label "member"^^xsd:string .

:socialAnxietyDisorder_Current
      a       owl:DatatypeProperty ;
      rdfs:comment "Describes if the subject currently has Social Anxiety Disorder." ;
      rdfs:domain :Covariates ;
      rdfs:label "social anxiety disorder current" ;
      rdfs:range xsd:boolean ;
      rdfs:subPropertyOf :psychopathologicalProperty .

:hasPersonRole_DataAnalyst
      a       owl:ObjectProperty ;
      rdfs:comment "Describes what project someone is a data analyst of"@en ;
      rdfs:domain :Project ;
      rdfs:label "has data analyst"@en ;
      rdfs:range :Person ;
      rdfs:subPropertyOf :contributor ;
      <http://purl.org/vocab/vann/example>
              "BipolarProject hasPersonRole_DataAnalyst JohnSmith"@en .

:demographicProperty
      a       owl:DatatypeProperty ;
      rdfs:comment "any demographic property" ;
      rdfs:label "demographic property" .

:education_Method
      a       owl:DatatypeProperty ;
      rdfs:comment "The method used for coding the Education Category (ie: 1 = some high school, 2 = some college, 3 = some professional degree)" ;
      rdfs:domain :Covariates ;
      rdfs:label "education method" ;
      rdfs:range xsd:string ;
      rdfs:subPropertyOf :demographicProperty .

:hasPublishedPaper
      a       owl:DatatypeProperty ;
      rdfs:comment "Describes the links to published papers or the paper title (if link does not exist) for the working group"@en ;
      rdfs:domain :WorkingGroup ;
      rdfs:label "has published paper"@en ;
      rdfs:range xsd:string ;
      rdfs:subPropertyOf owl:topDataProperty ;
      <http://purl.org/vocab/vann/example>
              "WorkingGroup2 hasPublishedPaper \"Article Title\""@en , "WorkingGroup1 hasPublishedPaper www.publishedpaperexample.com"@en .

<http://purl.org/vocab/vann/preferredNamespaceUri>
      a       owl:AnnotationProperty .

:negLifeEvents
      a       owl:DatatypeProperty ;
      rdfs:comment "Describes if the number of negative life events the subject experienced in the past 6 months is specified." ;
      rdfs:domain :Covariates ;
      rdfs:label "negative life events" ;
      rdfs:range xsd:boolean ;
      rdfs:subPropertyOf :psychopathologicalProperty .

:hasStudyDesign
      a       owl:DatatypeProperty ;
      rdfs:comment """Describes the study design of the cohort group or project (Case/control; Population; Healthy only; Patients only)

NOTE: study design options are mutually exclusive for Cohort Groups but not Projects"""@en , """Describes the study design of a project (Case/control; Population; Healthy only; Patients only)
NOTE: study design options are mutually exclusive for Cohort Groups but not Projects"""@en ;
      rdfs:domain :Project ;
      rdfs:domain
              [ a       owl:Class ;
                owl:unionOf (:CohortGroup :Project)
              ] ;
      rdfs:label "has study design"@en ;
      rdfs:range xsd:string ;
      <http://purl.org/vocab/vann/example>
              "Project1 hasStudyDesign \"Case/control, Population\""@en , "CohortGroup1 hasStudyDesign \"Population\""@en .

:hasGeneticDataType
      a       owl:ObjectProperty ;
      rdfs:comment "Describes the genetic data types that were collected for a cohort or project"@en ;
      rdfs:domain
              [ a       owl:Class ;
                owl:unionOf (:Cohort :CohortGroup :CohortProject)
              ] ;
      rdfs:label "has genetic data type"@en ;
      rdfs:range :GeneticDataType ;
      rdfs:subPropertyOf :hasDataType ;
      <http://purl.org/vocab/vann/example>
              "Cohort1 hasGeneticDataType epigenetic"@en .

:isPartOfProject
      a       owl:ObjectProperty ;
      rdfs:comment "Property that indicates the cohort groups specific to a project"@en ;
      rdfs:domain
              [ a       owl:Class ;
                owl:unionOf (:CohortGroup :CohortProject)
              ] ;
      rdfs:label "is part of project"@en ;
      rdfs:range :Project .

:MentalHealthDisorder
      a       owl:Class ;
      rdfs:comment "Disorders which can affect mood, behavior, and thinking"@en ;
      rdfs:label "Mental Health Disorder"@en ;
      rdfs:subClassOf :Disorder ;
      <http://purl.org/vocab/vann/example>
              "OCD"@en .

:hasContentUrl
      a       owl:DatatypeProperty ;
      rdfs:comment "Points to a media object, like an image or video file"^^xsd:string ;
      rdfs:domain :DataDownload ;
      rdfs:label "has content URL"^^xsd:string ;
      rdfs:range xsd:anyURI ;
      rdfs:subPropertyOf <https://schema.org/contentUrl> .

:NeurologicalDisorder
      a       owl:Class ;
      rdfs:comment "Disorders which affect the nervous system"@en ;
      rdfs:label "Neurological Disorder"@en ;
      rdfs:subClassOf :Disorder ;
      <http://purl.org/vocab/vann/example>
              "Epilepsy"@en .

:hasCurrentJobTitle
      a       owl:DatatypeProperty ;
      rdfs:comment "Data property that aims to capture the current job title of a person. Examples are student, faculty, staff, postdoc, etc."@en ;
      rdfs:domain :Person ;
      rdfs:label "has current job title"@en ;
      rdfs:range xsd:string ;
      <http://purl.org/vocab/vann/example>
              "JohnSmith hasCurrentJobTitle \"Postdoc\""@en .

:SubstanceAbuse
      a       owl:Class ;
      rdfs:comment "A mental health disorder defined by the overusage or abuse of a substance"@en ;
      rdfs:label "Substance Abuse"@en ;
      rdfs:subClassOf :MentalHealthDisorder ;
      <http://purl.org/vocab/vann/example>
              "Alcoholism"@en .

:otherSubstanceUseDisorder_Current
      a       owl:DatatypeProperty ;
      rdfs:comment "Describes subject's current drug use that meets criteria for substance abuse disorder at the time of scan (e.g. cocaine, opiods etc.)" ;
      rdfs:domain :Covariates ;
      rdfs:label "other substance use disorder current" ;
      rdfs:range xsd:string ;
      rdfs:subPropertyOf :useDisorderProperty .

:hasDate_DataContributionDeadline
      a       owl:DatatypeProperty ;
      rdfs:comment "Describes the deadline date for data contribution of a project"@en ;
      rdfs:domain :Project ;
      rdfs:label "has data contribution deadline date"@en ;
      rdfs:range xsd:date .

:psychoticDisorder_Lifetime
      a       owl:DatatypeProperty ;
      rdfs:comment "Describes if the subject had the Psychotic Disorder during their lifetime." ;
      rdfs:domain :Covariates ;
      rdfs:label "pyschotic disorder lifetime" ;
      rdfs:range xsd:boolean ;
      rdfs:subPropertyOf :psychopathologicalProperty .

<http://vivoweb.org/ontology/core#College>
      a       owl:Class ;
      rdfs:comment "A college contributing to a given ENIGMA project"@en ;
      rdfs:isDefinedBy <http://vivoweb.org/ontology/core> ;
      rdfs:label "College"@en ;
      rdfs:subClassOf <http://xmlns.com/foaf/0.1/Organization> ;
      <http://purl.org/vocab/vann/example>
              "Los Angeles City College"@en .

:otherDx_AgeofOnset
      a       owl:DatatypeProperty ;
      rdfs:comment "Describes if age of onset of subject's other psychiatric disorders is specified." ;
      rdfs:domain :Covariates ;
      rdfs:label "other Dx age of onset" ;
      rdfs:range xsd:boolean ;
      rdfs:subPropertyOf :psychopathologicalProperty .

:hasCountry
      a       owl:DatatypeProperty ;
      rdfs:comment "The country name associated with the address of the object"@en ;
      rdfs:domain :Address ;
      rdfs:label "has country"@en ;
      rdfs:range xsd:string ;
      rdfs:subPropertyOf <http://www.w3.org/2006/vcard/ns#country-name> .

:Address
      a       owl:Class ;
      rdfs:comment "To specify the components of the delivery address for the object"@en ;
      rdfs:label "Address"@en ;
      rdfs:subClassOf <http://www.w3.org/2006/vcard/ns#Address> .

:Marital_status
      a       owl:DatatypeProperty ;
      rdfs:comment "Property which states whether subject's marital status (ie: single, married) is specified." ;
      rdfs:domain :Covariates ;
      rdfs:label "marital status" ;
      rdfs:range xsd:boolean ;
      rdfs:subPropertyOf :demographicProperty .

:smokingStatus_Current
      a       owl:DatatypeProperty ;
      rdfs:comment "Describes if the subject is currently smoking." ;
      rdfs:domain :Covariates ;
      rdfs:label "smoking status current" ;
      rdfs:range xsd:boolean ;
      rdfs:subPropertyOf :useDisorderProperty .

:DataType
      a       owl:Class ;
      rdfs:comment "Specifies the kinds of data collected"@en ;
      rdfs:label "Data Type"@en .

<http://xmlns.com/foaf/0.1/Organization>
      a       owl:Class ;
      rdfs:comment "An organization contributing to a given ENIGMA project"@en ;
      rdfs:isDefinedBy <http://xmlns.com/foaf/0.1> ;
      owl:equivalentClass :Organization .

:SOFAS_Total
      a       owl:DatatypeProperty ;
      rdfs:comment "Describes whether the subject's Social and Occupational Functioning Assessment Scale total score is specified." ;
      rdfs:domain :Covariates ;
      rdfs:label "SOFAS total" ;
      rdfs:range xsd:boolean ;
      rdfs:subPropertyOf :scoreProperty .

:socialAnxietyDisorder_AgeofOnset
      a       owl:DatatypeProperty ;
      rdfs:comment "Describes whether age of onset of subject's Social Anxiety Disorder is specified." ;
      rdfs:domain :Covariates ;
      rdfs:label "social anxiety disorder age of onset" ;
      rdfs:range xsd:boolean ;
      rdfs:subPropertyOf :psychopathologicalProperty .

:OrganicMedicalDisorder
      a       owl:Class ;
      rdfs:comment "Disorder characterized by decreased mental function due to a medical or physical disease"@en ;
      rdfs:label "Organic Medical Disorder"@en ;
      rdfs:subClassOf :Disorder ;
      <http://purl.org/vocab/vann/example>
              "Delirium"@en .

:hasMiddleInitial
      a       owl:DatatypeProperty ;
      rdfs:comment "Describes middle initial of a person"^^xsd:string ;
      rdfs:domain :Person ;
      rdfs:label "has middle initial"@en ;
      rdfs:range xsd:string ;
      <http://purl.org/vocab/vann/example>
              "John A Smith hasMiddleInitial \"A\""^^xsd:string .

<http://purl.org/vocab/vann/preferredNamespacePrefix>
      a       owl:AnnotationProperty .

<http://purl.org/dc/terms/contributor>
      a       owl:AnnotationProperty , owl:ObjectProperty ;
      rdfs:isDefinedBy <http://purl.org/dc/terms/contributor> .

:hasSpecies
      a       owl:DatatypeProperty ;
      rdfs:comment "Describes the species of the subjects of a cohort (Humans, Chimps, Mice, etc.)"@en ;
      rdfs:domain
              [ a       owl:Class ;
                owl:unionOf (:Cohort :CohortGroup :CohortProject)
              ] ;
      rdfs:label "has species"@en ;
      rdfs:range xsd:string ;
      <http://purl.org/vocab/vann/example>
              "Cohort1 hasSpecies \"humans\""@en .

:hasPersonRole_ProtocolRunner
      a       owl:ObjectProperty ;
      rdfs:comment "Describes who ran a protocol for a given cohort"@en ;
      rdfs:domain :Project ;
      rdfs:label "has protocol runner"@en ;
      rdfs:range :Person ;
      rdfs:subPropertyOf :contributor ;
      <http://purl.org/vocab/vann/example>
              "BipolarProject hasPersonRole_ProtocolRunner JohnSmith"@en .

:isActive
      a       owl:DatatypeProperty ;
      rdfs:comment "Describes whether a project is active"@en ;
      rdfs:domain :Project ;
      rdfs:label "is Active"@en ;
      rdfs:range xsd:string .

:BrainScanDataType
      a       owl:Class ;
      rdfs:comment "Specifies the kinds of brain scan data collected"@en ;
      rdfs:label "Brain Scan Data Type"@en ;
      rdfs:subClassOf :DataType ;
      <http://purl.org/vocab/vann/example>
              "EEG"@en .

:hasDataset
      a       owl:ObjectProperty ;
      rdfs:comment "Property that links a cohort project with the data being described."@en ;
      rdfs:domain
              [ a       owl:Class ;
                owl:unionOf (:Cohort :CohortProject)
              ] ;
      rdfs:label "has dataset"@en ;
      rdfs:range :Dataset .

:usesProtocol
      a       owl:ObjectProperty ;
      rdfs:comment "Describes which protocol was used in a project"@en ;
      rdfs:domain :Project ;
      rdfs:label "uses protocol"@en ;
      rdfs:range :Protocol ;
      <http://purl.org/vocab/vann/example>
              "BipolarProject usesProtocol ENIGMA-SulciProtocol"@en .

:ImageAcquisitionProtocol
      a       owl:Class ;
      rdfs:comment "Procedure used to collect image data within the cohort"@en ;
      rdfs:label "Image Acquisition Protocol"@en ;
      <http://purl.org/vocab/vann/example>
              "ENIGMA-Sulci"@en .

xsd:date
      a       rdfs:Datatype .

<http://vivoweb.org/ontology/core#University>
      a       owl:Class ;
      rdfs:comment "A university contributing to a given ENIGMA project"@en ;
      rdfs:isDefinedBy <http://vivoweb.org/ontology/core> ;
      rdfs:label "University"@en ;
      rdfs:subClassOf <http://xmlns.com/foaf/0.1/Organization> ;
      <http://purl.org/vocab/vann/example>
              "USC"@en .

:Dataset
      a       owl:Class ;
      rdfs:comment "A dataset containing information about an ENIGMA project cohort"@en ;
      rdfs:label "Dataset"@en ;
      rdfs:subClassOf <http://schema.org/Dataset> .

:AcademicArticle
      a       owl:Class ;
      rdfs:comment "An academic article, submitted as a result of the work in an ENIGMA project"@en ;
      rdfs:label "Academic article"@en .

:hasContact
      a       owl:ObjectProperty ;
      rdfs:comment "Property that points to the person that is a contact for the project or cohort"@en ;
      rdfs:domain
              [ a       owl:Class ;
                owl:unionOf (:Cohort :CohortGroup :CohortProject)
              ] ;
      rdfs:label "has contact"@en ;
      rdfs:range :Person ;
      <http://purl.org/vocab/vann/example>
              "BipolarCohort hasContact JohnSmith"@en .

:hasEmail
      a       owl:ObjectProperty ;
      rdfs:comment "Property that indicates which is the email of a person"@en ;
      rdfs:domain :Person ;
      rdfs:label "has email"@en ;
      rdfs:range owl:Thing ;
      rdfs:subPropertyOf <http://xmlns.com/foaf/0.1/mbox> ;
      <http://www.linkedmodel.org/schema/vaem#rationale>
              "Property added to facilitate interaction with domain and ranges in the wiki. It's equivalent to foaf:mbox"@en .

:psychoticDisorder_DiagnosisType
      a       owl:DatatypeProperty ;
      rdfs:comment "Describes whether the subject's Psychotic Disorder type (ie: schizophrenia, schizoaffective disorder, delusional disorder, psychosis NOS, schizophreniform disorder, brief psychotic disorder, shared psychotic disorder, substance-induced psychosis) is specified." ;
      rdfs:domain :Covariates ;
      rdfs:label "psychotic disorder diagnosis type" ;
      rdfs:range xsd:boolean ;
      rdfs:subPropertyOf :psychopathologicalProperty .

:hasFamilyName
      a       owl:DatatypeProperty ;
      rdfs:comment "The family name of some person."@en ;
      rdfs:domain :Person ;
      rdfs:label "has family name"@en ;
      rdfs:range xsd:string ;
      rdfs:subPropertyOf <http://xmlns.com/foaf/0.1/familyName> ;
      <http://www.linkedmodel.org/schema/vaem#rationale>
              "Property added to restrict the domain to enigma:Person. This is done for facilitating the interaction with the wiki interface"@en .

:atypicalAntipsychoticUse_Current
      a       owl:DatatypeProperty ;
      rdfs:comment "Describes if the subject's use of 2nd generation (atypical) antipsychotics at time of scan is speciied." ;
      rdfs:domain :Covariates ;
      rdfs:label "atypical antipsychotic use current" ;
      rdfs:range xsd:boolean ;
      rdfs:subPropertyOf :medicationSomaticProperty .

:BD_Current
      a       owl:DatatypeProperty ;
      rdfs:comment "Describes if the subject currently has Bipolar Disorder." ;
      rdfs:domain :Covariates ;
      rdfs:label "BD current" ;
      rdfs:range xsd:boolean ;
      rdfs:subPropertyOf :psychopathologicalProperty .

:somaticIllness_current
      a       owl:DatatypeProperty ;
      rdfs:comment "Describes if the subject has a type of somatic illness." ;
      rdfs:domain :Covariates ;
      rdfs:label "somatic illness current" ;
      rdfs:range xsd:string ;
      rdfs:subPropertyOf :medicationSomaticProperty .

:lithiumUse_Lifetime
      a       owl:DatatypeProperty ;
      rdfs:comment "Describes if the subject's use of lithium during their lifetime is specified." ;
      rdfs:domain :Covariates ;
      rdfs:label "lithium use lifetime" ;
      rdfs:range xsd:boolean ;
      rdfs:subPropertyOf :medicationSomaticProperty .

:ConflictOfInterest
      a       owl:Class ;
      rdfs:comment "Concept used to represent a conflict of interest of an author in a paper"@en ;
      rdfs:label "Conflict of interest"@en .

:MDD_Lifetime
      a       owl:DatatypeProperty ;
      rdfs:comment "Describes if the subject had Major Depressive Disorder during their lifetime." ;
      rdfs:domain :Covariates ;
      rdfs:label "MDD lifetime" ;
      rdfs:range xsd:boolean ;
      rdfs:subPropertyOf :psychopathologicalProperty .

:hasCohortStatus
      a       owl:DatatypeProperty ;
      rdfs:comment "Describes the current status of a cohort, cohort group or cohort project"@en ;
      rdfs:domain
              [ a       owl:Class ;
                owl:unionOf (:Cohort :CohortGroup :CohortProject)
              ] ;
      rdfs:label "has cohort status"@en ;
      rdfs:range
              [ a       rdfs:Datatype ;
                owl:oneOf
                        [ a       rdf:List ;
                          rdf:first "gathering participants"^^xsd:string ;
                          rdf:rest
                                  [ a       rdf:List ;
                                    rdf:first "protocol preparation"^^xsd:string ;
                                    rdf:rest
                                            [ a       rdf:List ;
                                              rdf:first "published"^^xsd:string ;
                                              rdf:rest
                                                      [ a       rdf:List ;
                                                        rdf:first "revision"^^xsd:string ;
                                                        rdf:rest ()
                                                      ]
                                            ]
                                  ]
                        ]
              ] ;
      <http://purl.org/vocab/vann/example>
              "CohortGroup1 hasCohortStatus published"@en .

:BD_Lifetime
      a       owl:DatatypeProperty ;
      rdfs:comment "Describes if the subject had Bipolar Disorder during their lifetime." ;
      rdfs:domain :Covariates ;
      rdfs:label "BD lifetime" ;
      rdfs:range xsd:boolean ;
      rdfs:subPropertyOf :psychopathologicalProperty .

:psychoticDisorder_AgeofOnset
      a       owl:DatatypeProperty ;
      rdfs:comment "Describes whether the age of onset of the subject's psychotic disorder is specified." ;
      rdfs:domain :Covariates ;
      rdfs:label "psychotic disorder age of onset" ;
      rdfs:range xsd:boolean ;
      rdfs:subPropertyOf :psychopathologicalProperty .

:OCD_Lifetime
      a       owl:DatatypeProperty ;
      rdfs:comment "Describes if the subject had Obsessive Compulsive Disorder during their lifetime." ;
      rdfs:domain :Covariates ;
      rdfs:label "OCD lifetime" ;
      rdfs:range xsd:boolean ;
      rdfs:subPropertyOf :psychopathologicalProperty .

:socialAnxietyDisorder_Lifetime
      a       owl:DatatypeProperty ;
      rdfs:comment "Describes if the subject had Social Anxiety Disorder during their lifetime." ;
      rdfs:domain :Covariates ;
      rdfs:label "social anxiety disorder lifetime" ;
      rdfs:range xsd:boolean ;
      rdfs:subPropertyOf :psychopathologicalProperty .

<http://vivoweb.org/ontology/core#Institute>
      a       owl:Class ;
      rdfs:comment "An institute contributing to a given ENIGMA project"@en ;
      rdfs:isDefinedBy <http://vivoweb.org/ontology/core> ;
      rdfs:label "Institute"@en ;
      rdfs:subClassOf <http://xmlns.com/foaf/0.1/Organization> ;
      <http://purl.org/vocab/vann/example>
              "Information Sciences Institute"@en .

:subject_SocioeconomicStatus
      a       owl:DatatypeProperty ;
      rdfs:comment "The scale used in measuring a subject’s socioeconomic status." ;
      rdfs:domain :Covariates ;
      rdfs:label "subject socioeconomic status" ;
      rdfs:range xsd:string ;
      rdfs:subPropertyOf :demographicProperty .

:MDD_AgeofOnset
      a       owl:DatatypeProperty ;
      rdfs:comment "Describes whether the age of onset of the subject's first depressive episode is specified." ;
      rdfs:domain :Covariates ;
      rdfs:label "MDD age of onset" ;
      rdfs:range xsd:boolean ;
      rdfs:subPropertyOf :psychopathologicalProperty .

:GAF_Total
      a       owl:DatatypeProperty ;
      rdfs:comment "Describes if the subject's Global Assessment of Functioning scale total score is specified." ;
      rdfs:domain :Covariates ;
      rdfs:label "GAF total" ;
      rdfs:range xsd:boolean ;
      rdfs:subPropertyOf :scoreProperty .

:EndocrineDisorder
      a       owl:Class ;
      rdfs:comment "Disorders which affect the endocrine system"@en ;
      rdfs:label "Endocrine Disorder"@en ;
      rdfs:subClassOf :Disorder ;
      <http://purl.org/vocab/vann/example>
              "Hypothyroidism"@en .

:hasAge_StandardDeviation
      a       owl:DatatypeProperty ;
      rdfs:comment "Describes the standard deviation of the age of a cohort"@en ;
      rdfs:domain
              [ a       owl:Class ;
                owl:unionOf (:CohortGroup :CohortProject)
              ] ;
      rdfs:label "has age standard deviation"@en ;
      rdfs:range xsd:double ;
      <http://purl.org/vocab/vann/example>
              "Cohort1 hasAge_StandardDeviation 5.0"@en .

:hasPersonRole_Investigator
      a       owl:ObjectProperty ;
      rdfs:comment "Describe the investigators of a cohort"@en ;
      rdfs:domain :Cohort ;
      rdfs:label "has person role investigator"@en ;
      rdfs:range :Person ;
      <http://purl.org/vocab/vann/example>
              "BipolarCohort hasInvestigator JohnSmith"@en .

:hasPersonRole_DataCollector
      a       owl:ObjectProperty ;
      rdfs:comment "Describes what project someone collected data for"@en ;
      rdfs:domain :Project ;
      rdfs:label "has data collector"@en ;
      rdfs:range :Person ;
      rdfs:subPropertyOf :contributor ;
      <http://purl.org/vocab/vann/example>
              "BipolarProject hasPersonRole_DataCollector JohnSmith"@en .

:hasSubmittedPaper
      a       owl:DatatypeProperty ;
      rdfs:comment "Describes the titles of the submitted papers of a working group"@en ;
      rdfs:domain :WorkingGroup ;
      rdfs:label "has submitted paper"@en ;
      rdfs:range xsd:string ;
      <http://purl.org/vocab/vann/example>
              "WorkingGroup1 hasSubmittedPaper \"Paper title\""@en .

:CGITotal
      a       owl:DatatypeProperty ;
      rdfs:comment "Describes the subject's Global Clinical Impression Scale's total score." ;
      rdfs:domain :Covariates ;
      rdfs:label "CGI total" ;
      rdfs:range xsd:boolean ;
      rdfs:subPropertyOf :scoreProperty .

:hasStreetAddress
      a       owl:DatatypeProperty ;
      rdfs:comment "The street address associated with the address of the object"@en ;
      rdfs:domain :Address ;
      rdfs:label "has street address"@en ;
      rdfs:range xsd:string ;
      rdfs:subPropertyOf <http://www.w3.org/2006/vcard/ns#street-address> .

:otherDx_Current
      a       owl:DatatypeProperty ;
      rdfs:comment "Describes the subject's other psychiatric diagnoses at the time of scan (e.g. borderline personality disorder, ADHD, etc.)." ;
      rdfs:domain :Covariates ;
      rdfs:label "other dx current" ;
      rdfs:range xsd:string ;
      rdfs:subPropertyOf :psychopathologicalProperty .

:hasPersonRole_PrincipalInvestigator
      a       owl:ObjectProperty ;
      rdfs:comment "Describes who the principal investigator of the cohort is"@en , "Describes the principal investigator of the cohort"@en ;
      rdfs:domain :Cohort ;
      rdfs:label "has PersonRole Principal Investigator"@en , "has person role principal investigator"@en ;
      rdfs:range :Person ;
      rdfs:subPropertyOf :hasPersonRole_Investigator ;
      <http://purl.org/vocab/vann/example>
              "Cohort1 hasPrincipalInvestigator JohnSmith"@en , "Cohort1 hasPrincipalInvestigator John --> the principal investigator of Cohort1 is John"@en .

:hasHomePage
      a       owl:DatatypeProperty , owl:ObjectProperty ;
      rdfs:comment "Property that describes the home page of a cohort or person"@en , "Homepage URL of the Person or Cohort"@en ;
      rdfs:domain
              [ a       owl:Class ;
                owl:unionOf (:Cohort :Person)
              ] ;
      rdfs:domain
              [ a       owl:Class ;
                owl:unionOf (:Cohort :CohortGroup :CohortProject :Person)
              ] ;
      rdfs:label "has home page"@en ;
      rdfs:range owl:Thing , xsd:anyURI ;
      <http://www.linkedmodel.org/schema/vaem#rationale>
              "Property added to facilitate interaction with domain and ranges in the wiki. It's equivalent to foaf:homePage"@en .

:panicDisorder_AgeofOnset
      a       owl:DatatypeProperty ;
      rdfs:comment "Describes whether age of onset of subject's Panic Disorder is specified." ;
      rdfs:domain :Covariates ;
      rdfs:label "panic disorder age of onset" ;
      rdfs:range xsd:boolean ;
      rdfs:subPropertyOf :psychopathologicalProperty .

:Covariates
      a       owl:Class ;
      rdfs:comment "A class used to describe covariates information for a cohort or study." ;
      rdfs:label "Covariates" .

:hasName_Full
      a       owl:DatatypeProperty ;
      rdfs:comment "Describes the full name of the working group"@en ;
      rdfs:domain :WorkingGroup ;
      rdfs:label "has full name"@en ;
      rdfs:range xsd:string ;
      rdfs:subPropertyOf <http://purl.org/dc/terms/title> ;
      <http://purl.org/vocab/vann/example>
              "SchizophreniaWG hasName_Full SchizophreniaWorkingGroup"@en .

:hasDataCollectionPeriodEnd
      a       owl:DatatypeProperty ;
      rdfs:comment "Describes the end year of the data collection period of the cohort"@en ;
      rdfs:domain
              [ a       owl:Class ;
                owl:unionOf (:Cohort :CohortGroup :CohortProject)
              ] ;
      rdfs:label "has data collection period end"@en ;
      rdfs:range xsd:gYear ;
      <http://purl.org/vocab/vann/example>
              "Cohort1 hasDataCollectionPeriodEnd 2008"@en .

:useDisorderProperty
      a       owl:DatatypeProperty ;
      rdfs:comment "Any use disorder property" ;
      rdfs:label "use disorder property" .

:hasTransgenderMtoF
      a       owl:DatatypeProperty ;
      rdfs:comment "Describing the number of male to female transgender individuals in a cohort group"@en ;
      rdfs:domain :CohortGroup ;
      rdfs:label "has transgender m to f"@en ;
      rdfs:range xsd:nonNegativeInteger ;
      <http://purl.org/vocab/vann/example>
              "CohortGroup1 hasTransgenderMtoF 20"@en .

:hasPopulationGroup
      a       owl:ObjectProperty ;
      rdfs:comment "Describes the population group of a population-based cohort"@en ;
      rdfs:domain
              [ a       owl:Class ;
                owl:unionOf (:Cohort :CohortGroup :CohortProject)
              ] ;
      rdfs:label "has population group"@en ;
      rdfs:range :CohortGroup ;
      rdfs:subPropertyOf :hasCohortGroup ;
      <http://purl.org/vocab/vann/example>
              "BipolarCohort hasPopulationGroup USCPopulationGroup"@en .

<https://schema.org/description>
      a       owl:DatatypeProperty ;
      rdfs:isDefinedBy <https://schema.org/> .

:barratt_TotalScore
      a       owl:DatatypeProperty ;
      rdfs:comment "Describes if the subject's Barratt Impulsiveness Scale total score is specified." ;
      rdfs:domain :Covariates ;
      rdfs:label "barratt total score" ;
      rdfs:range xsd:boolean ;
      rdfs:subPropertyOf :scoreProperty .

:hasAge_Group
      a       owl:DatatypeProperty ;
      rdfs:comment "Describes the age groupings of individuals within a cohort group"@en ;
      rdfs:domain :Cohort ;
      rdfs:label "has age group"@en ;
      rdfs:range xsd:string ;
      <http://purl.org/vocab/vann/example>
              "Cohort1 hasAge_Group \"22-45\""@en .

:HealthyVariation
      a       owl:Class ;
      rdfs:comment "Working groups that are not disease focused"@en ;
      rdfs:label "Healthy Variation"@en ;
      rdfs:subClassOf :WorkingGroup .

:CerebrovascularDisorder
      a       owl:Class ;
      rdfs:comment "A subset of vascular disorders affecting blood vessels of the brain and cerebral circulation"@en ;
      rdfs:label "Cerebrovascular Disorder"@en ;
      rdfs:subClassOf :VascularDisorder ;
      <http://purl.org/vocab/vann/example>
              "Stroke"@en .

:hasPersonRole_FirstDraftContributor
      a       owl:ObjectProperty ;
      rdfs:comment "Property designed to distinguish who collaborated in the creation of the first draft of a publication"@en ;
      rdfs:domain
              [ a       owl:Class ;
                owl:unionOf (:AcademicArticle :Project)
              ] ;
      rdfs:label "first draft contributor"@en ;
      rdfs:range :Person ;
      rdfs:subPropertyOf :contributor ;
      <http://purl.org/vocab/vann/example>
              "BipolarProject hasPersonRole_FirstDraftContributor JohnSmith"@en .

:hasGroupCriteria
      a       owl:DatatypeProperty ;
      rdfs:comment "Criteria used to define group of cohort patients"@en ;
      rdfs:domain :CohortGroup ;
      rdfs:label "has group criteria"@en ;
      rdfs:range xsd:string .

:hasPostalCode
      a       owl:DatatypeProperty ;
      rdfs:comment "The postal code associated with the address of the object"@en ;
      rdfs:domain :Address ;
      rdfs:label "has postal code"@en ;
      rdfs:range xsd:string ;
      rdfs:subPropertyOf <http://www.w3.org/2006/vcard/ns#postal-code> .

:hasBrainScanDataType
      a       owl:ObjectProperty ;
      rdfs:comment "Describes which brain scan data types a cohort or project has"@en , "Describes the brain scan data types that were collected for a cohort or project"@en ;
      rdfs:domain
              [ a       owl:Class ;
                owl:unionOf (:Cohort :Project)
              ] ;
      rdfs:domain
              [ a       owl:Class ;
                owl:unionOf (:Cohort :CohortGroup :CohortProject :Project)
              ] ;
      rdfs:label "has brain scan data type"@en ;
      rdfs:range :BrainScanDataType ;
      rdfs:subPropertyOf :hasDataType ;
      <http://purl.org/vocab/vann/example>
              "Cohort1 hasBrainScanDataType MRI"@en , "BipolarProject hasBrainScanDataType DiffusionMRI"@en .

:GeneticDisorder
      a       owl:Class ;
      rdfs:comment "Disorders which are inherited and caused by abnormalities in the genome"@en ;
      rdfs:label "Genetic Disorder"@en ;
      rdfs:subClassOf :Disorder ;
      <http://purl.org/vocab/vann/example>
              "Cystic Fibrosis"@en .

:Sex  a       owl:DatatypeProperty ;
      rdfs:comment "Property to state whether subject's sex (male, female, other) is specified or not." ;
      rdfs:domain :Covariates ;
      rdfs:label "sex" ;
      rdfs:range xsd:boolean ;
      rdfs:subPropertyOf :demographicProperty .

:Project
      a       owl:Class ;
      rdfs:comment "Project encompassing cohort"@en , "Project associated with the cohort"@en ;
      rdfs:label "Project"@en ;
      <http://purl.org/vocab/vann/example>
              "SZPositiveSymptoms"@en .

<http://purl.org/dc/terms/license>
      a       owl:AnnotationProperty .

<http://purl.org/dc/terms/title>
      a       owl:DatatypeProperty , owl:AnnotationProperty ;
      rdfs:isDefinedBy <http://purl.org/dc/terms/title> ;
      rdfs:range rdfs:Literal .

:Country
      a       owl:Class ;
      rdfs:comment "Country in which a cohort is located"@en ;
      rdfs:label "Country"@en ;
      rdfs:subClassOf :Location ;
      <http://purl.org/vocab/vann/example>
              "United States"@en .

:alcoholUseDisorder_AgeofOnset
      a       owl:DatatypeProperty ;
      rdfs:comment "Describes the age of onset of the subject's alcohol use disorder." ;
      rdfs:domain :Covariates ;
      rdfs:label "alcohol use disorder age of onset" ;
      rdfs:range xsd:boolean ;
      rdfs:subPropertyOf :useDisorderProperty .

<http://www.w3.org/2006/vcard/ns#hasAddress>
      a       owl:ObjectProperty ;
      rdfs:isDefinedBy <http://www.w3.org/2006/vcard/ns> ;
      rdfs:label "has Address"^^xsd:string .

:IQ   a       owl:DatatypeProperty ;
      rdfs:subPropertyOf :demographicProperty .

:hasTransgenderFtoM
      a       owl:DatatypeProperty ;
      rdfs:comment "Describing the number of female to male transgender individuals in a cohort group"@en ;
      rdfs:domain :CohortGroup ;
      rdfs:label "has transgender F to M"@en ;
      rdfs:range xsd:nonNegativeInteger ;
      <http://purl.org/vocab/vann/example>
              "CohortGroup2 hasTransgenderFtoM 14"@en .

:psychoticDisorder_Current
      a       owl:DatatypeProperty ;
      rdfs:comment "Describes if the subject currently has a Psychotic Disorder." ;
      rdfs:domain :Covariates ;
      rdfs:label "pyschotic disorder current" ;
      rdfs:range xsd:boolean ;
      rdfs:subPropertyOf :psychopathologicalProperty .

:parent_SocioeconomicStatus
      a       owl:DatatypeProperty ;
      rdfs:comment "Highest level of parental socioeconomic status either based on education, occupation or both." ;
      rdfs:domain :Covariates ;
      rdfs:label "parent socioeconomic status" ;
      rdfs:range xsd:string ;
      rdfs:subPropertyOf :demographicProperty .

:otherMedUse_Current
      a       owl:DatatypeProperty ;
      rdfs:comment "Describes the subject's other medication use at time of scan." ;
      rdfs:domain :Covariates ;
      rdfs:label "other medication use current" ;
      rdfs:range xsd:string ;
      rdfs:subPropertyOf :medicationSomaticProperty .

:IQ_method
      a       owl:DatatypeProperty ;
      rdfs:comment "The IQ scale used for each subject/group (ie: WISC-IV, WAIS-IV, WASI-II)." ;
      rdfs:domain :Covariates ;
      rdfs:label "IQ method" ;
      rdfs:range xsd:string ;
      rdfs:subPropertyOf :demographicProperty .

:MDD_Current
      a       owl:DatatypeProperty ;
      rdfs:comment "Describes if the subject currently has Major Depressive Disorder." ;
      rdfs:domain :Covariates ;
      rdfs:label "MDD current" ;
      rdfs:range xsd:boolean ;
      rdfs:subPropertyOf :psychopathologicalProperty .

:hasAge_Maximum
      a       owl:DatatypeProperty ;
      rdfs:comment "Describes inclusion criteria for maximum age of participants in a Cohort, CohortProject or CohortGroup"@en ;
      rdfs:domain
              [ a       owl:Class ;
                owl:unionOf (:Cohort :CohortGroup :CohortProject)
              ] ;
      rdfs:label "has maximum age"@en ;
      rdfs:range xsd:positiveInteger ;
      <http://purl.org/vocab/vann/example>
              "CohortGroup1 hasAge_Maximum 60"@en .

:SubjID
      a       owl:DatatypeProperty ;
      rdfs:comment "Property which states whether the identification code/number of unique subjects is specified." ;
      rdfs:domain :Covariates ;
      rdfs:label "subject ID" ;
      rdfs:range xsd:boolean ;
      rdfs:subPropertyOf :demographicProperty .

<http://schema.org/Dataset>
      a       owl:Class ;
      rdfs:comment "Dataset"^^xsd:string ;
      rdfs:isDefinedBy <http://schema.org> ;
      rdfs:label "Dataset"^^xsd:string .

:education_Category
      a       owl:DatatypeProperty ;
      rdfs:comment "Subject's education coded as categories (ie: a range from 1-5)" ;
      rdfs:domain :Covariates ;
      rdfs:label "education category" ;
      rdfs:range xsd:string ;
      rdfs:subPropertyOf :demographicProperty .

:hasKindOfInstitute
      a       owl:DatatypeProperty ;
      rdfs:comment "Describes the specific kind/type of an organization"@en ;
      rdfs:domain :Organization ;
      rdfs:label "kind of institute"@en ;
      rdfs:range xsd:string ;
      <http://purl.org/vocab/vann/example>
              "Organization kind \"University\""@en .

:hasBriefDescription
      a       owl:DatatypeProperty ;
      rdfs:comment "Provides a brief description of the working group or project or cohort or image acquisition protocol"@en , "Provides a brief description of the working group or project or cohort"@en ;
      rdfs:domain
              [ a       owl:Class ;
                owl:unionOf (:Cohort :Project :WorkingGroup)
              ] ;
      rdfs:domain
              [ a       owl:Class ;
                owl:unionOf (:Cohort :Project :WorkingGroup)
              ] ;
      rdfs:domain
              [ a       owl:Class ;
                owl:unionOf (:Cohort :CohortGroup :CohortProject :ImageAcquisitionProtocol :Project :WorkingGroup)
              ] ;
      rdfs:label "has brief description"@en ;
      rdfs:range xsd:string ;
      rdfs:subPropertyOf <http://purl.org/dc/terms/description> ;
      <http://purl.org/vocab/vann/example>
              "SZWG hasBriefDescription \"finds correlations between schizophrenia and other conditions\""@en , "SZCohort hasBriefDescription \"finds correlations between schizophrenia and other conditions\""@en , "ProjectSZ hasBriefDescription \"reports effect size for corticol thickness\""@en .

:hasCohort
      a       owl:ObjectProperty ;
      rdfs:comment "Describes what cohorts are part of a project or working group"@en , "Describes what cohorts are part of the project"@en ;
      rdfs:domain
              [ a       owl:Class ;
                owl:unionOf (:Project :WorkingGroup)
              ] ;
      rdfs:domain
              [ a       owl:Class ;
                owl:unionOf (:Project :WorkingGroup)
              ] ;
      rdfs:domain
              [ a       owl:Class ;
                owl:unionOf (:Project :WorkingGroup)
              ] ;
      rdfs:label "has cohort"@en ;
      rdfs:range :Cohort ;
      <http://purl.org/vocab/vann/example>
              "BipolarProject hasCohort AmsterdamBipolarCohort --> Bipolar Project includes the Amsterdam Bipolar Cohort"@en , "BipolarWorkingGroup hasCohort AmsterdamBipolarCohort --> Bipolar Working Group includes the Amsterdam Bipolar Cohort"@en , "BipolarProject hasCohort AmsterdamBipolarCohort"@en .

:panicDisorder_Current
      a       owl:DatatypeProperty ;
      rdfs:comment "Describes if the subject currently has Panic Disorder." ;
      rdfs:domain :Covariates ;
      rdfs:label "panic disorder current" ;
      rdfs:range xsd:boolean ;
      rdfs:subPropertyOf :psychopathologicalProperty .

:hasFundingSource
      a       owl:DatatypeProperty ;
      rdfs:comment "Describes the funding source of the cohort"@en ;
      rdfs:domain
              [ a       owl:Class ;
                owl:unionOf (:Cohort :CohortProject)
              ] ;
      rdfs:label "has funding source"@en ;
      rdfs:range xsd:string ;
      <http://purl.org/vocab/vann/example>
              "Cohort1 hasFundingSource \"NIMH, 5P50MH080272\""@en .

:BAS_TotalScore
      a       owl:DatatypeProperty ;
      rdfs:comment "Describes if the Behavioral Activation System subscale score on the BIS/BAS is specified." ;
      rdfs:domain :Covariates ;
      rdfs:label "BAS total score" ;
      rdfs:range xsd:boolean ;
      rdfs:subPropertyOf :scoreProperty .

:GeneticDataType
      a       owl:Class ;
      rdfs:comment "Specifies the kinds of genetic data collected"@en ;
      rdfs:label "Genetic Data Type"@en ;
      rdfs:subClassOf :DataType ;
      <http://purl.org/vocab/vann/example>
              "Epigenetic"@en .

:hasResearchInterest
      a       owl:DatatypeProperty ;
      rdfs:comment "Describes a research interest of a person"@en ;
      rdfs:domain :Person ;
      rdfs:label "has research interest"@en ;
      rdfs:range xsd:string ;
      <http://purl.org/vocab/vann/example>
              "JohnSmith hasReasearchInterest \"bipolar disorder\", \"schizophrenia\""@en .

:Organization
      a       owl:Class ;
      rdfs:comment "An organization belonging to the ENIGMA consortium. Organization can be hospitals, universities, departments, etc."^^xsd:string , "An organization belonging to the ENIGMA consortium. Organization can be hospitals, universities, departments, etc."@en , "An organization contributing to a given ENIGMA project"@en ;
      rdfs:isDefinedBy <http://xmlns.com/foaf/0.1> ;
      rdfs:label "Organization"@en ;
      <http://purl.org/vocab/vann/example>
              "Information Sciences Institute"@en ;
      :example "Information Sciences Institute"^^xsd:string .

:hasDiagnosticGroup
      a       owl:ObjectProperty ;
      rdfs:comment "Describes the patient group of a cohort"@en ;
      rdfs:domain
              [ a       owl:Class ;
                owl:unionOf (:Cohort :CohortProject)
              ] ;
      rdfs:label "has diagnostic group"@en ;
      rdfs:range :CohortGroup ;
      rdfs:subPropertyOf :hasCohortGroup ;
      <http://purl.org/vocab/vann/example>
              "BipolarCohort hasPatientGroup BipolarPatientGroup"@en .

:isPublic
      a       owl:DatatypeProperty ;
      rdfs:comment "Describes if a cohort's data is publicly available"@en ;
      rdfs:domain
              [ a       owl:Class ;
                owl:unionOf (:Cohort :CohortGroup :CohortProject)
              ] ;
      rdfs:label "is public"@en ;
      rdfs:range xsd:boolean ;
      <http://purl.org/vocab/vann/example>
              "SZCohort isPublic \"true\""@en .

:hasPersonRole_MainPrincipalInvestigator
      a       owl:ObjectProperty ;
      rdfs:comment "Describes which cohorts somone is a main PI of"@en ;
      rdfs:domain
              [ a       owl:Class ;
                owl:unionOf (:Cohort :CohortGroup :CohortProject)
              ] ;
      rdfs:label "has main person role principal investigator"@en ;
      rdfs:range :Person ;
      rdfs:subPropertyOf :hasPersonRole_PrincipalInvestigator ;
      <http://purl.org/vocab/vann/example>
              "Cohort1 hasMainPrincipalInvestigatorof JohnSmith"@en .

:subject_SocioeconomicStatusScale
      a       owl:DatatypeProperty ;
      rdfs:comment "The highest level of subject's socioeconomic status based on education, occupation or both." ;
      rdfs:domain :Covariates ;
      rdfs:label "subject socioeconomic status" ;
      rdfs:range xsd:string ;
      rdfs:subPropertyOf :demographicProperty .

:psychopathologicalProperty
      a       owl:DatatypeProperty ;
      rdfs:comment "Any psychopathological property" ;
      rdfs:label "psychopathological property" .

<https://w3id.org/enigma>
      a       owl:Ontology , owl:NamedIndividual ;
      rdfs:comment "An ontology for describing people's roles in ENIGMA projects."^^xsd:string ;
      <http://purl.org/dc/terms/contributor>
              "Kevin Low" , "Haripriya Dharmala"^^xsd:string , "Michael Bornstein" , "Ryan Espiritu" , "Yolanda Gil"^^xsd:string , "MiHyun Jang" , "Hernan Vargas" , "Agnes McMahon" , "Agnes McMahon"^^xsd:string , "Daniel Garijo"^^xsd:string ;
      <http://purl.org/dc/terms/creator>
              "Michael Bornstein"^^xsd:string , "Josh Boyd" , "Ryan Espiritu"^^xsd:string , "Yolanda Gil" , "Daniel Garijo" , "Daniel Garijo"^^xsd:string , "Haripriya Dharmala" , "Haripriya Dharmala"^^xsd:string , "Joanna Bright" , "Wesley Surento" , "MiHyun Jang"^^xsd:string , "Neda Jahanshad" , "Neda Jahanshad"^^xsd:string ;
      <http://purl.org/dc/terms/description>
              "An ontology to describe cohorts of patients participating in ENIGMA projects."@en , "An ontology representing roles different persons play in ENIGMA projects, organizations, papers, or working groups."@en , "A core ontology representing the main concepts of ENIGMA."@en , "An ontology representing covariates for the ENIGMA Suicidal Thoughts and Behaviors working group" , "An ontology that describes ENIGMA projects and their properties."@en , "An ontology representing organizations that participate in the ENIGMA consortium."@en , "An ontology representing Working Groups that participate in the ENIGMA consortium."@en , "A cohort ontology that describes persons participating in ENIGMA and their properties."@en ;
      <http://purl.org/dc/terms/license>
              <http://creativecommons.org/licenses/by/2.0/> ;
      <http://purl.org/dc/terms/title>
              "The Core Ontology"@en , "The Project Ontology"@en , "The Roles Ontology"@en , "The STB Ontology" , "The Cohort Ontology"@en , "The Person Ontology"^^xsd:string , "The Organization Ontology"^^xsd:string , "The Working Group Ontology"@en ;
      <http://purl.org/vocab/vann/preferredNamespacePrefix>
              "enigma" , "enigma"^^xsd:string , <https://w3id.org/enigma> ;
      <http://purl.org/vocab/vann/preferredNamespaceUri>
              : ;
      owl:priorVersion <https://w3id.org/enigma/roles/1.0.0> , <https://w3id.org/enigma/organization/1.1.0> , "https://w3id.org/enigma/cohort/1.0.0"^^xsd:string , <https://w3id.org/enigma/core/1.0.0> , <https://w3id.org/enigma/wg/1.0.0> , <https://w3id.org/enigma/person/1.0.0> ;
      owl:versionIRI <https://w3id.org/enigma/cohort/1.1.0> , <https://w3id.org/enigma/roles/1.1.0> , <https://w3id.org/enigma/core/1.1.0> , <https://w3id.org/enigma/stb/1.1.0> , <https://w3id.org/enigma/organization/1.1.0> , <https://w3id.org/enigma/project/1.1.0> , <https://w3id.org/enigma/person/1.1.0> , <https://w3id.org/enigma/wg/1.1.0> ;
      owl:versionInfo "v1.1.0" , "v1.1.0"^^xsd:string .

:hasPersonRole_ProjectLead
      a       owl:ObjectProperty ;
      rdfs:comment "Describes what project someone is a project lead of"@en ;
      rdfs:domain :Project ;
      rdfs:label "has project lead"@en ;
      rdfs:range :Person ;
      rdfs:subPropertyOf owl:topObjectProperty ;
      <http://purl.org/vocab/vann/example>
              "BipolarProject hasPersonRole_ProjectLead JohnSmith"@en .

:MoodDisorder
      a       owl:Class ;
      rdfs:comment "A mental health disorder defined by mood or behavioral swings"@en ;
      rdfs:label "Mood Disorder"@en ;
      rdfs:subClassOf :MentalHealthDisorder ;
      <http://purl.org/vocab/vann/example>
              "Bipolar Disorder"@en .

:Methodology
      a       owl:Class ;
      rdfs:comment "Working groups that develop protocols (imaging or genetics)"@en ;
      rdfs:label "Methodology"@en ;
      rdfs:subClassOf :WorkingGroup .

<http://purl.org/dc/terms/isPartOf>
      a       owl:ObjectProperty ;
      rdfs:comment "A related resource in which the described resource is included."^^xsd:string ;
      rdfs:isDefinedBy <http://purl.org/dc/terms/> ;
      rdfs:label "is Part of"^^xsd:string .

<http://schema.org/DataDownload>
      a       owl:Class ;
      rdfs:isDefinedBy <http://schema.org> ;
      rdfs:label "Data Download"^^xsd:string .

:hasPublication
      a       owl:ObjectProperty ;
      rdfs:comment "Property that links a project to a publication that resulted from it."@en ;
      rdfs:domain :Project ;
      rdfs:label "has publication"@en ;
      rdfs:range :AcademicArticle .

:ClinicalPopulation
      a       owl:Class ;
      rdfs:comment "Working groups that study clinical populations"@en ;
      rdfs:label "Clinical Population"@en ;
      rdfs:subClassOf :WorkingGroup .

:hasCohortGroup
      a       owl:ObjectProperty ;
      rdfs:comment "Property that indicates the cohort groups part of a cohort"@en ;
      rdfs:domain
              [ a       owl:Class ;
                owl:unionOf (:Cohort :CohortProject)
              ] ;
      rdfs:label "has cohort group"@en ;
      rdfs:range :CohortGroup ;
      <http://purl.org/vocab/vann/example>
              "QTIM has cohort group QTIM_control"@en .

:GAD_AgeofOnset
      a       owl:DatatypeProperty ;
      rdfs:comment "Describes if age of onset of subject's Generalized Anxiety Disorder is specified." ;
      rdfs:domain :Covariates ;
      rdfs:label "GAD age of onset" ;
      rdfs:range xsd:boolean ;
      rdfs:subPropertyOf :psychopathologicalProperty .

<http://vivoweb.org/ontology/core#orcidId>
      a       owl:ObjectProperty ;
      rdfs:comment "This is now an object property where the object value is a resource of the form <http://orcid.org/NNNN-NNNN-NNNN-NNNN>.  This is to support connecting VIVO and ORCID in the linked data web.   Note: a person can have multiple ORCID iDs."^^xsd:string ;
      rdfs:isDefinedBy "http://vivoweb.org/ontology/core#"@en .

<http://xmlns.com/foaf/0.1/familyName>
      a       owl:DatatypeProperty ;
      rdfs:comment "The family name of some person."^^xsd:string ;
      rdfs:domain <http://xmlns.com/foaf/0.1/Person> ;
      rdfs:isDefinedBy "http://xmlns.com/foaf/0.1/"@en .

:Location
      a       owl:Class ;
      rdfs:comment "Geographic location of the cohort"@en ;
      rdfs:label "Location"@en ;
      <http://purl.org/vocab/vann/example>
              "Los Angeles, California"@en .

:GeneticStudy
      a       owl:Class ;
      rdfs:comment "Working groups dedicated to genetic analysis"@en ;
      rdfs:label "Genetic study"@en ;
      rdfs:subClassOf :WorkingGroup .

:CohortProject
      a       owl:Class ;
      rdfs:comment "The subset of the individuals from a Cohort, which are used as samples for a specific project"@en ;
      rdfs:label "Cohort Project"@en ;
      rdfs:subClassOf :Cohort ;
      <http://purl.org/vocab/vann/example>
              "\"Healthy\" individuals from the ASRB Cohort were sampled to form a Cohort Project of SZCorticol"@en .

:hasCohortProject
      a       owl:ObjectProperty ;
      rdfs:comment "Describes the subcohorts, specific to a given project, that are part of that cohort"@en ;
      rdfs:domain
              [ a       owl:Class ;
                owl:unionOf (:Cohort :CohortGroup :ImageAcquisitionProtocol)
              ] ;
      rdfs:label "has cohort project"@en ;
      rdfs:range :CohortProject ;
      <http://purl.org/vocab/vann/example>
              "BipolarCohort hasCohortProject BipolarBarcelonaCohort"@en .

:diagnosisGroup
      a       owl:DatatypeProperty ;
      rdfs:comment "Property which states whether the diagnostic group each subject is associated with (control vs. experimental) is specified." ;
      rdfs:domain :Covariates ;
      rdfs:label "diagnosis group" ;
      rdfs:range xsd:boolean ;
      rdfs:subPropertyOf :demographicProperty .

:hasGrant
      a       owl:DatatypeProperty ;
      rdfs:comment "Data property that aims to capture the grants that have been obtained by a person, in order to properly list them in the acknowledgements of the corresponding publication"@en ;
      rdfs:domain :Person ;
      rdfs:label "has grant"@en ;
      rdfs:range xsd:string ;
      <http://purl.org/vocab/vann/example>
              "John Smith hasGrant \"U54EB020403 (NIH)\""@en .

:alcoholUseDisorderScale
      a       owl:DatatypeProperty ;
      rdfs:comment "Describes whether the scale used to determine the diagnosis of alcohol use disorder (ie: SCID, ASSIST, AUDIT) is specified." ;
      rdfs:domain :Covariates ;
      rdfs:label "alcohol use disorder scale" ;
      rdfs:range xsd:boolean ;
      rdfs:subPropertyOf :useDisorderProperty .

<http://xmlns.com/foaf/0.1/mbox>
      a       owl:ObjectProperty ;
      rdfs:comment "A  personal mailbox, ie. an Internet mailbox associated with exactly one owner, the first owner of this mailbox. This is a 'static inverse functional property', in that  there is (across time and change) at most one individual that ever has any particular value for foaf:mbox."^^xsd:string ;
      rdfs:domain <http://xmlns.com/foaf/0.1/Person> ;
      rdfs:isDefinedBy "http://xmlns.com/foaf/0.1/"@en ;
      rdfs:range owl:Thing .

<http://www.w3.org/2006/vcard/ns#country-name>
      a       owl:DatatypeProperty .

:City
      a       owl:Class ;
      rdfs:comment "City in which a cohort is located"@en ;
      rdfs:label "City"@en ;
      rdfs:subClassOf :Location ;
      <http://purl.org/vocab/vann/example>
              "Los Angeles"@en .

:SubstanceDependence
      a       owl:Class ;
      rdfs:comment "A subset of substance abuse in which symptoms of withdrawal may appeared after reduction of substance use"@en ;
      rdfs:label "Substance Dependence"@en ;
      rdfs:subClassOf :SubstanceAbuse ;
      <http://purl.org/vocab/vann/example>
              "Alcohol Dependence"@en .

:BD_DiagnosisType
      a       owl:DatatypeProperty ;
      rdfs:comment "Describes whether the subject's Bipolar Disorder type (ie: type I, type II, NOS, no BD, NA) is specified." ;
      rdfs:domain :Covariates ;
      rdfs:label "BD diagnosis type" ;
      rdfs:range xsd:boolean ;
      rdfs:subPropertyOf :psychopathologicalProperty .

:hasNumberOfFemaleSex
      a       owl:DatatypeProperty ;
      rdfs:comment "Describing the number of females in a cohort project"@en ;
      rdfs:domain :CohortProject ;
      rdfs:label "has number of females"@en ;
      rdfs:range xsd:nonNegativeInteger ;
      <http://purl.org/vocab/vann/example>
              "CohortGroup2 hasNumberOfFemaleSex 16"@en .

<http://www.w3.org/2006/vcard/ns#region>
      a       owl:DatatypeProperty .

:hasAdditionalDemographic
      a       owl:DatatypeProperty ;
      rdfs:comment "Describes the additional demographics defining a given cohort"@en ;
      rdfs:domain :Cohort ;
      rdfs:label "has additional demographic"@en ;
      rdfs:range xsd:string ;
      <http://purl.org/vocab/vann/example>
              "CohortGroup1 hasAdditionalDemographic \"handedness, IQ\""@en .

:hasCollectionSite
      a       owl:DatatypeProperty ;
      rdfs:comment "Describes where the data of the cohort was collected"@en ;
      rdfs:domain :Cohort ;
      rdfs:label "has collection site"@en ;
      rdfs:range xsd:string ;
      <http://purl.org/vocab/vann/example>
              "Cohort1 hasCollectionSite Toronto"@en .

:WorkingGroup
      a       owl:Class ;
      rdfs:comment "Group of researchers studying a certain topic/disease"@en ;
      rdfs:label "Working Group"@en ;
      <http://purl.org/vocab/vann/example>
              "BipolarWG"@en .

:AnxietyDisorder
      a       owl:Class ;
      rdfs:comment "A mental health disorder defined by feelings of anxiety, fear, or worry"@en ;
      rdfs:label "Anxiety Disorder"@en ;
      rdfs:subClassOf :MentalHealthDisorder ;
      <http://purl.org/vocab/vann/example>
              "PTSD"@en .

:negLifeEventsMethod
      a       owl:DatatypeProperty ;
      rdfs:comment "Describes the questionnaire/interview used to assess negative life events from past 6 months (e.g. NLESS, SLESQ)." ;
      rdfs:domain :Covariates ;
      rdfs:label "negative life events method" ;
      rdfs:range xsd:string ;
      rdfs:subPropertyOf :psychopathologicalProperty .

xsd:gYear
      a       rdfs:Datatype .

:hasNumberOfParticipants
      a       owl:DatatypeProperty ;
      rdfs:comment "Describes the number of participants in a cohort group or cohort project"@en ;
      rdfs:domain
              [ a       owl:Class ;
                owl:unionOf (:CohortGroup :CohortProject)
              ] ;
      rdfs:label "has number of participants"@en ;
      rdfs:range xsd:int ;
      <http://purl.org/vocab/vann/example>
              "CohortGroup2 hasNumberOfParticipants 200"@en .

<http://vivoweb.org/ontology/core#Hospital>
      a       owl:Class ;
      rdfs:comment "A hospital contributing to a given ENIGMA project"@en ;
      rdfs:isDefinedBy <http://vivoweb.org/ontology/core> ;
      rdfs:label "Hospital"@en ;
      rdfs:subClassOf <http://xmlns.com/foaf/0.1/Organization> ;
      <http://purl.org/vocab/vann/example>
              "Children's Hospital Los Angeles"@en .

:hasMemorandumOfUnderstanding
      a       owl:DatatypeProperty ;
      rdfs:comment "Describes the memorandum of understanding links of the working group"@en ;
      rdfs:domain :WorkingGroup ;
      rdfs:label "has memorandum of understanding"@en ;
      rdfs:range xsd:string ;
      <http://purl.org/vocab/vann/example>
              "WorkingGroup1 hasMemorandumOfUnderstanding www.mouexample.com"@en .

<http://xmlns.com/foaf/0.1/givenName>
      a       owl:DatatypeProperty ;
      rdfs:comment "The given name of some person."@en ;
      rdfs:domain <http://xmlns.com/foaf/0.1/Person> ;
      rdfs:isDefinedBy <http://xmlns.com/foaf/0.1/> .

:hasDegree
      a       owl:DatatypeProperty ;
      rdfs:comment "Describes what degree a person has (e.g., BsC, PhD, etc.)"@en ;
      rdfs:domain :Person ;
      rdfs:label "has degree"@en ;
      rdfs:range xsd:string ;
      <http://purl.org/vocab/vann/example>
              "JohnSmith hasDegree PhD"@en .

:hasDate_ProposalApproval
      a       owl:DatatypeProperty ;
      rdfs:comment "Describes the date the proposal for a project was approved"@en ;
      rdfs:domain :Project ;
      rdfs:label "has proposal approval date"@en ;
      rdfs:range xsd:date .

:PTSD_Lifetime
      a       owl:DatatypeProperty ;
      rdfs:comment "Describes if the subject had Post-Traumatic Stress Disorder during their lifetime." ;
      rdfs:domain :Covariates ;
      rdfs:label "PTSD lifetime" ;
      rdfs:range xsd:boolean ;
      rdfs:subPropertyOf :psychopathologicalProperty .

:hasNumberOfMaleSex
      a       owl:DatatypeProperty ;
      rdfs:comment "Describing the number of males in a cohort project"@en ;
      rdfs:domain :CohortProject ;
      rdfs:label "has number of males"@en ;
      rdfs:range xsd:nonNegativeInteger ;
      <http://purl.org/vocab/vann/example>
              "CohortGroup2 hasNumberOfMaleSex 12"@en .

:PTSD_Current
      a       owl:DatatypeProperty ;
      rdfs:comment "Describes if the subject currently has Post-Traumatic Stress Disorder." ;
      rdfs:domain :Covariates ;
      rdfs:label "PTSD current" ;
      rdfs:range xsd:boolean ;
      rdfs:subPropertyOf :psychopathologicalProperty .

<http://xmlns.com/foaf/0.1/homepage>
      a       owl:ObjectProperty ;
      rdfs:comment "A homepage for some thing."^^xsd:string ;
      rdfs:isDefinedBy <http://xmlns.com/foaf/0.1/> ;
      rdfs:label "homepage"^^xsd:string .

:race_ethnicity
      a       owl:DatatypeProperty ;
      rdfs:comment "Subject's race/ethnicity." ;
      rdfs:domain :Covariates ;
      rdfs:label "race ethnicity" ;
      rdfs:range xsd:string ;
      rdfs:subPropertyOf :demographicProperty .

:requiresDataType
      a       owl:ObjectProperty ;
      rdfs:comment "Describes which data type is required by a project"@en ;
      rdfs:domain :Project ;
      rdfs:label "requires data type"@en ;
      rdfs:range :DataType .

:hasConflictOfInterest
      a       owl:ObjectProperty ;
      rdfs:comment "Property linking an author with a conflict of interest that the author has on a paper"@en ;
      rdfs:domain :Person ;
      rdfs:label "has conflict of interest"@en ;
      rdfs:range :ConflictOfInterest .

:DiagnosticInstrument
      a       owl:Class ;
      rdfs:comment "The method used to diagnose individuals in a Cohort"@en ;
      rdfs:label "Diagnostic Instrument"@en ;
      <http://purl.org/vocab/vann/example>
              "Consensus Consultant Diagnosis"@en .

<http://vivoweb.org/ontology/core#Consortium>
      a       owl:Class ;
      rdfs:comment "A consortium contributing to a given ENIGMA project"@en ;
      rdfs:isDefinedBy <http://vivoweb.org/ontology/core> ;
      rdfs:label "Consortium"@en ;
      rdfs:subClassOf <http://xmlns.com/foaf/0.1/Organization> ;
      <http://purl.org/vocab/vann/example>
              "ENIGMA"@en .

:hasPersonRole_ProjectContact
      a       owl:ObjectProperty ;
      rdfs:comment "Property that points to the person that is a contact for the project or cohort"@en ;
      rdfs:domain
              [ a       owl:Class ;
                owl:unionOf (:Cohort :Project)
              ] ;
      rdfs:label "has contact"@en ;
      rdfs:range :Person ;
      rdfs:subPropertyOf owl:topObjectProperty ;
      <http://purl.org/vocab/vann/example>
              "BipolarCohort hasPersonRole_ProjectContact JohnSmith"@en .

:studiesDisorder
      a       owl:ObjectProperty ;
      rdfs:comment "Property that indicates which project/working group studies which disorder"@en ;
      rdfs:domain
              [ a       owl:Class ;
                owl:unionOf (:Project :WorkingGroup)
              ] ;
      rdfs:label "studies disorder"@en ;
      rdfs:range :Disorder .

:hasName
      a       owl:DatatypeProperty ;
      rdfs:comment "Name of an item"^^xsd:string ;
      rdfs:domain :Dataset ;
      rdfs:label "has name"^^xsd:string ;
      rdfs:range xsd:string ;
      rdfs:subPropertyOf <https://schema.org/name> .

:typicalAntipsychoticUse_Lifetime
      a       owl:DatatypeProperty ;
      rdfs:comment "Describes if the subject's use of 1st generation (typical) antipsychotics during their lifetime is specified." ;
      rdfs:domain :Covariates ;
      rdfs:label "typical antipsychotic use lifetime" ;
      rdfs:range xsd:boolean ;
      rdfs:subPropertyOf :medicationSomaticProperty .

:alcoholUseDisorder_Lifetime
      a       owl:DatatypeProperty ;
      rdfs:comment "Describes whether the subject's previous lifetime alcohol use disorder (ie: dependence, abuse, none) is specified." ;
      rdfs:domain :Covariates ;
      rdfs:label "alcohol use disorder lifetime" ;
      rdfs:range xsd:boolean ;
      rdfs:subPropertyOf :useDisorderProperty .

:otherSubstanceUseDisorder_Lifetime
      a       owl:DatatypeProperty ;
      rdfs:comment "Describes subject's previous lifetime drug use that meets criteria for lifetime substance abuse disorder  (e.g. cocaine, opiods etc.)" ;
      rdfs:domain :Covariates ;
      rdfs:label "other substance use disorder lifetime" ;
      rdfs:range xsd:string ;
      rdfs:subPropertyOf :useDisorderProperty .

<http://vivoweb.org/ontology/core#Department>
      a       owl:Class ;
      rdfs:comment "A department contributing to a given ENIGMA project"@en ;
      rdfs:isDefinedBy <http://vivoweb.org/ontology/core> ;
      rdfs:label "Department"@en ;
      rdfs:subClassOf <http://xmlns.com/foaf/0.1/Organization> ;
      <http://purl.org/vocab/vann/example>
              "Department of Psychology, USC"@en .

:antiepilepticUse_Current
      a       owl:DatatypeProperty ;
      rdfs:comment "Describes whether the subject's use of antiepileptics at time of scan is specified." ;
      rdfs:domain :Covariates ;
      rdfs:label "antiepileptic use current" ;
      rdfs:range xsd:boolean ;
      rdfs:subPropertyOf :medicationSomaticProperty .

:BD_CurrentState
      a       owl:DatatypeProperty ;
      rdfs:comment "Describes the subject's current Bipolar Disorder state (ie: depressed, hypomanic, manic, eutyhmic, mixed)" ;
      rdfs:domain :Covariates ;
      rdfs:label "BD current state" ;
      rdfs:range xsd:boolean ;
      rdfs:subPropertyOf :psychopathologicalProperty .

:hasDate_TargetStart
      a       owl:DatatypeProperty ;
      rdfs:comment "Describes the start date of the target period of the project"@en ;
      rdfs:domain :Project ;
      rdfs:label "has target start date"@en ;
      rdfs:range xsd:date .

:CohortGroup
      a       owl:Class ;
      rdfs:comment "A subset of Cohort, which either forms the patient group or control group"@en ;
      rdfs:label "Cohort Group"@en ;
      rdfs:subClassOf :Cohort ;
      <http://purl.org/vocab/vann/example>
              "AMCControlGroup is a control cohort group of the AMC cohort"@en .

:Disorder
      a       owl:Class ;
      rdfs:comment "A disorder/disease experienced by members of a cohort"@en ;
      rdfs:label "Disorder"@en .

:lithiumUse_Current
      a       owl:DatatypeProperty ;
      rdfs:comment "Describes if the subject's use of lithium at time of scan is specified." ;
      rdfs:domain :Covariates ;
      rdfs:label "lithium use current" ;
      rdfs:range xsd:boolean ;
      rdfs:subPropertyOf :medicationSomaticProperty .

:MDD_Stage
      a       owl:DatatypeProperty ;
      rdfs:comment "Describes whether the current stage of the subject's Major Depressive Disorder (ie: recurrent or first episode) is specified." ;
      rdfs:domain :Covariates ;
      rdfs:label "MDD stage" ;
      rdfs:range xsd:boolean ;
      rdfs:subPropertyOf :psychopathologicalProperty .

:hasProject
      a       owl:ObjectProperty ;
      rdfs:comment "Describes what projects are worked on by a specific working group"@en ;
      rdfs:domain :WorkingGroup ;
      rdfs:label "has project"@en ;
      rdfs:range :Project ;
      <http://purl.org/vocab/vann/example>
              "BipolarWorkingGroup hasProject BipolarCorticolProject --> The Bipolar Working Group is working on the Bipolar Corticol Project"@en .

:CardiovascularDisorder
      a       owl:Class ;
      rdfs:comment "A subset of vascular disorders affecting the heart"@en ;
      rdfs:label "Cardiovascular Disorder"@en ;
      rdfs:subClassOf :VascularDisorder ;
      <http://purl.org/vocab/vann/example>
              "Coronary Artery Disease"@en .

<http://www.w3.org/2006/vcard/ns#postal-code>
      a       owl:DatatypeProperty .

<http://purl.org/dc/terms/description>
      a       owl:DatatypeProperty , owl:AnnotationProperty .

:otherDx_Lifetime
      a       owl:DatatypeProperty ;
      rdfs:comment "Describes the subject's other psychiatric diagnoses during their lifetime (e.g. borderline personality disorder, ADHD, etc.)" ;
      rdfs:domain :Covariates ;
      rdfs:label "other dx lifetime" ;
      rdfs:range xsd:string ;
      rdfs:subPropertyOf :psychopathologicalProperty .

:BD_AgeofOnset
      a       owl:DatatypeProperty ;
      rdfs:comment "Describes whether the age of onset of the subject's Bipolar Disorder is specified." ;
      rdfs:domain :Covariates ;
      rdfs:label "BD age of onset" ;
      rdfs:range xsd:boolean ;
      rdfs:subPropertyOf :psychopathologicalProperty .

<http://purl.org/vocab/vann/example>
      a       owl:AnnotationProperty .

:Age  a       owl:DatatypeProperty ;
      rdfs:comment "Subject's age in years ." ;
      rdfs:domain :Covariates ;
      rdfs:label "age" ;
      rdfs:range xsd:integer ;
      rdfs:subPropertyOf :demographicProperty .

:hasProjectResults
      a       owl:ObjectProperty ;
      rdfs:comment "Property to link project results to a Cohort Project"^^xsd:string ;
      rdfs:domain :CohortProject ;
      rdfs:label "has project results"^^xsd:string ;
      rdfs:range :DataDownload .

:InfectiousDisorder
      a       owl:Class ;
      rdfs:comment "A disease or disorder caused by the invasion of microorganisms"@en ;
      rdfs:label "Infectious Disorder"@en ;
      rdfs:subClassOf :Disorder ;
      <http://purl.org/vocab/vann/example>
              "HIV"@en .

:smokingStatus_Lifetime
      a       owl:DatatypeProperty ;
      rdfs:comment "Describes if the subject smoked during their lifetime." ;
      rdfs:domain :Covariates ;
      rdfs:label "smoking status lifetime" ;
      rdfs:range xsd:boolean ;
      rdfs:subPropertyOf :useDisorderProperty .

:hasStatistics
      a       owl:ObjectProperty ;
      rdfs:comment "Property used to link a cohort with the summary statistics that may have been  produced after applying a given protocol"@en ;
      rdfs:domain :CohortProject ;
      rdfs:label "has statistics"@en ;
      rdfs:range :Dataset .

:example
      a       owl:AnnotationProperty .

:hasImageAcquisitionProtocol
      a       owl:ObjectProperty ;
      rdfs:comment "Describes the acquisition protocol that was used to scan the data of a cohort"@en , "Describes the acquisition protocol that was used to scan a cohort"@en ;
      rdfs:domain :Cohort ;
      rdfs:domain
              [ a       owl:Class ;
                owl:unionOf (:Cohort :CohortGroup :CohortProject)
              ] ;
      rdfs:label "has image acquisition protocol"@en , "has acquisition protocol"@en ;
      rdfs:range :ImageAcquisitionProtocol ;
      <http://purl.org/vocab/vann/example>
              "Cohort1 hasImageAcquisitionProtocol AcquisitionProtocol1"@en , "Cohort1 hasAcquisitionProtocol AcquiPro3"@en .

:hasAffiliate
      a       owl:ObjectProperty ;
      rdfs:comment "Describes the organization's affiliates"@en , "Points to the person who is an affiliate of an organization"@en ;
      rdfs:domain :Organization ;
      rdfs:label "has affiliate"@en ;
      rdfs:range :Person ;
      rdfs:subPropertyOf <http://xmlns.com/foaf/0.1/member> ;
      <http://purl.org/vocab/vann/example>
              "Harvard hasAffiliate JohnSmith"@en , "HarvardU hasAffiliate JohnSmith"@en .

owl:topDataProperty
      rdfs:domain :Covariates ;
      rdfs:range xsd:boolean .

:medicationSomaticProperty
      a       owl:DatatypeProperty ;
      rdfs:comment "Any Medication use/Somatic Health property" ;
      rdfs:label "Medication use/Somatic Health property" .

:MDD_TotalEpisodes
      a       owl:DatatypeProperty ;
      rdfs:comment "Describes whether the subject's current number of depressive episodes is specified." ;
      rdfs:domain :Covariates ;
      rdfs:label "MDD total episodes" ;
      rdfs:range xsd:boolean ;
      rdfs:subPropertyOf :psychopathologicalProperty .

:hasDescription
      a       owl:DatatypeProperty ;
      rdfs:comment "Description of an item"^^xsd:string ;
      rdfs:domain :Dataset ;
      rdfs:label "has description"^^xsd:string ;
      rdfs:range xsd:string ;
      rdfs:subPropertyOf <https://schema.org/description> .

:hasTotalNumberOfParticipants
      a       owl:DatatypeProperty ;
      rdfs:comment "Describes the total number of participants in the cohort"@en ;
      rdfs:domain :Cohort ;
      rdfs:label "has total number of participants"@en ;
      rdfs:range xsd:positiveInteger ;
      <http://purl.org/vocab/vann/example>
              "Cohort1 hasTotalNumberOfParticipants 500 --> Cohort1 is made up of approximately 500 patients"@en .

:hasGivenName
      a       owl:DatatypeProperty ;
      rdfs:comment "The given name of some person."@en ;
      rdfs:domain :Person ;
      rdfs:label "has given name"@en ;
      rdfs:range xsd:string ;
      rdfs:subPropertyOf <http://xmlns.com/foaf/0.1/givenName> ;
      <http://www.linkedmodel.org/schema/vaem#rationale>
              "Property added to restrict the domain to enigma:Person. This is done for facilitating the interaction with the wiki interface"@en .

:hasEthnicGroup
      a       owl:DatatypeProperty ;
      rdfs:comment "Describes the ethnic group that the participants of the cohort are in"@en ;
      rdfs:domain
              [ a       owl:Class ;
                owl:unionOf (:Cohort :CohortProject)
              ] ;
      rdfs:label "has ethnic group"@en ;
      rdfs:range
              [ a       rdfs:Datatype ;
                owl:oneOf
                        [ a       rdf:List ;
                          rdf:first "African American"^^xsd:string ;
                          rdf:rest
                                  [ a       rdf:List ;
                                    rdf:first "Asian"^^xsd:string ;
                                    rdf:rest
                                            [ a       rdf:List ;
                                              rdf:first "European"^^xsd:string ;
                                              rdf:rest
                                                      [ a       rdf:List ;
                                                        rdf:first "Latino"^^xsd:string ;
                                                        rdf:rest
                                                                [ a       rdf:List ;
                                                                  rdf:first "Two or More Races"^^xsd:string ;
                                                                  rdf:rest ()
                                                                ]
                                                      ]
                                            ]
                                  ]
                        ]
              ] ;
      <http://purl.org/vocab/vann/example>
              "Cohort1 hasEthnicGroup \"European\""@en .

:SignificantGeneralMedicalCondition
      a       owl:Class ;
      rdfs:comment "Blanket term ecompassing serious medical condtions"@en ;
      rdfs:label "Significant General Medical Condition"@en ;
      rdfs:subClassOf :Disorder ;
      <http://purl.org/vocab/vann/example>
              "Cancer"@en .

:VascularDisorder
      a       owl:Class ;
      rdfs:comment "Disorder which affects the body's network of blood vessels"@en ;
      rdfs:label "Vascular Disorder"@en ;
      rdfs:subClassOf :Disorder ;
      <http://purl.org/vocab/vann/example>
              "Coronary Artery Disease"@en .

:PTSD_AgeofOnset
      a       owl:DatatypeProperty ;
      rdfs:comment "Describes if the age of onset of the subject's Post-Traumatic Stress Disorder is specified." ;
      rdfs:domain :Covariates ;
      rdfs:label "PTSD age of onset" ;
      rdfs:range xsd:boolean ;
      rdfs:subPropertyOf :psychopathologicalProperty .

:antidepressantUse_Lifetime
      a       owl:DatatypeProperty ;
      rdfs:comment "Describes if the subject's use of antidepressants during their lifetime is specified." ;
      rdfs:domain :Covariates ;
      rdfs:label "antidepressant use lifetime" ;
      rdfs:range xsd:boolean ;
      rdfs:subPropertyOf :medicationSomaticProperty .

:hasPersonRole_Reviewer
      a       owl:ObjectProperty ;
      rdfs:comment "Property that indicates who contributed to the paper reviewing the initial drafts and providing comments"@en ;
      rdfs:domain
              [ a       owl:Class ;
                owl:unionOf (:AcademicArticle :Project)
              ] ;
      rdfs:label "has reviewer"@en ;
      rdfs:range :Person ;
      rdfs:subPropertyOf :contributor ;
      <http://purl.org/vocab/vann/example>
              "BipolarProject hasPersonRole_Reviewer JohnSmith"@en .

:hasDataProcessingProtocol
      a       owl:ObjectProperty ;
      rdfs:comment "Describes which data processing protocol was used in a project"@en ;
      rdfs:domain :Project ;
      rdfs:label "uses data processing protocol"@en ;
      rdfs:range :Protocol .

:hasCoordinates
      a       owl:DatatypeProperty ;
      rdfs:comment "The coordinates associated with an organization"@en ;
      rdfs:domain :Organization ;
      rdfs:label "has coordinates"@en ;
      rdfs:range xsd:string .

:antidepressantUse_Current
      a       owl:DatatypeProperty ;
      rdfs:comment "Describes if the subject's use of antidepressants at time of scan is specified." ;
      rdfs:domain :Covariates ;
      rdfs:label "antidepressant use current" ;
      rdfs:range xsd:boolean ;
      rdfs:subPropertyOf :medicationSomaticProperty .

:OCD_Current
      a       owl:DatatypeProperty ;
      rdfs:comment "Describes if the subject currently has Obsessive Compulsive Disorder." ;
      rdfs:domain :Covariates ;
      rdfs:label "OCD current" ;
      rdfs:range xsd:boolean ;
      rdfs:subPropertyOf :psychopathologicalProperty .

:hasDataCollectionPeriodStart
      a       owl:DatatypeProperty ;
      rdfs:comment "Describes the start year of the data collection period of the cohort"@en ;
      rdfs:domain
              [ a       owl:Class ;
                owl:unionOf (:Cohort :CohortGroup :CohortProject)
              ] ;
      rdfs:label "has data collection period start"@en ;
      rdfs:range xsd:gYear ;
      <http://purl.org/vocab/vann/example>
              "Cohort1 hasDataCollectionPeriodStart 2005"@en .

:Cohort
      a       owl:Class ;
      rdfs:comment "A group of individuals studied by a working group, limited by certain inclusion and exclusion criteria"@en ;
      rdfs:label "Cohort"@en ;
      <http://purl.org/vocab/vann/example>
              "ADNI: Alzheimer’s Disease Neuroimaging Initiative"@en .

:scoreProperty
      a       owl:DatatypeProperty ;
      rdfs:comment "Any score property" ;
      rdfs:label "score property" .

:barratt_VersionUsed
      a       owl:DatatypeProperty ;
      rdfs:comment "Describes the Barratt Impulsiveness Scale version that was used." ;
      rdfs:domain :Covariates ;
      rdfs:label "barratt version used" ;
      rdfs:range xsd:string ;
      rdfs:subPropertyOf :scoreProperty .

:isPartOfCohort
      a       owl:ObjectProperty ;
      rdfs:comment "Property that indicates the cohort groups and cohort projects which are part of a cohort"@en ;
      rdfs:domain
              [ a       owl:Class ;
                owl:unionOf (:Cohort :CohortGroup :CohortProject)
              ] ;
      rdfs:label "is part of cohort"@en ;
      rdfs:range :Cohort .

<http://purl.org/ontology/bibo/AcademicArticle>
      a       owl:Class ;
      rdfs:isDefinedBy <http://purl.org/ontology/bibo/AcademicArticle> ;
      owl:equivalentClass :AcademicArticle .

:hasCovariates
      a       owl:ObjectProperty ;
      rdfs:domain :Cohort ;
      rdfs:label "has covariates"@en ;
      rdfs:range :Covariates .

:hasOrcidId
      a       owl:ObjectProperty ;
      rdfs:comment "ORCID Id of a Person"@en ;
      rdfs:domain :Person ;
      rdfs:label "has ORCID Id"@en ;
      rdfs:subPropertyOf <http://vivoweb.org/ontology/core#orcidId> ;
      <http://www.linkedmodel.org/schema/vaem#rationale>
              "Property added to facilitate interaction with the wiki, making domains and ranges explicit"@en .

:hasDataType
      a       owl:ObjectProperty ;
      rdfs:comment "Describes the data types that a cohort or project collected"@en ;
      rdfs:domain
              [ a       owl:Class ;
                owl:unionOf (:Cohort :Project)
              ] ;
      rdfs:domain
              [ a       owl:Class ;
                owl:unionOf (:Cohort :Project)
              ] ;
      rdfs:label "has data type"@en ;
      rdfs:range :DataType ;
      <http://purl.org/vocab/vann/example>
              "BipolarProject hasDataType MRIImage"@en , "Cohort1 hasDataType dataType1"@en .

:isPartOfOrganization
      a       owl:ObjectProperty ;
      rdfs:comment "Describes the parent organization which an organization is a part of. An organization may be part of more than one organizations."@en ;
      rdfs:domain :Organization ;
      rdfs:label "is part of organization"@en ;
      rdfs:range :Organization ;
      rdfs:subPropertyOf <http://purl.org/dc/terms/isPartOf> ;
      <http://purl.org/vocab/vann/example>
              "Department of Psychology, USC isPartOfOrganization USC"@en .

:hasControlGroup
      a       owl:ObjectProperty ;
      rdfs:comment "Describes the control group of a cohort"@en ;
      rdfs:domain
              [ a       owl:Class ;
                owl:unionOf (:Cohort :CohortProject)
              ] ;
      rdfs:label "has control group"@en ;
      rdfs:range :CohortGroup ;
      rdfs:subPropertyOf :hasCohortGroup ;
      <http://purl.org/vocab/vann/example>
              "BipolarCohort hasControlGroup BipolarControlGroup"@en .

:education_Years
      a       owl:DatatypeProperty ;
      rdfs:comment "Property to state whether subject's education in years is specified." ;
      rdfs:domain :Covariates ;
      rdfs:label "education years" ;
      rdfs:range xsd:boolean ;
      rdfs:subPropertyOf :demographicProperty .

:author
      a       owl:ObjectProperty ;
      rdfs:comment "Property to describe the author of a publication in the context of an ENIGMA project"@en ;
      rdfs:domain :AcademicArticle ;
      rdfs:label "author"@en ;
      rdfs:range :Person ;
      rdfs:subPropertyOf <http://purl.org/dc/terms/creator> .

:isPartOfCohortGroup
      a       owl:ObjectProperty ;
      rdfs:comment "Property that indicates the projects which are part of a cohort group"@en ;
      rdfs:domain :CohortProject ;
      rdfs:label "is part of cohort group"@en ;
      rdfs:range :CohortGroup .

:Person
      a       owl:Class ;
      rdfs:comment "A person associated with a given organization"@en , "Individual involved with the cohort"@en ;
      rdfs:label "Person"@en ;
      <http://purl.org/vocab/vann/example>
              "Theo van Erp"@en .

:hasProposalForm
      a       owl:DatatypeProperty ;
      rdfs:comment "Describes the approved proposal form link of a project"@en ;
      rdfs:domain :Project ;
      rdfs:label "has approved proposal form"@en ;
      rdfs:range xsd:anyURI ;
      <http://purl.org/vocab/vann/example>
              "Project1 hasProposalForm www.proposalformexample.com"@en .

:usesEncodingFormat
      a       owl:DatatypeProperty ;
      rdfs:comment "Encoding format of an item"@en ;
      rdfs:domain :DataDownload ;
      rdfs:label "uses encoding format"@en ;
      rdfs:range xsd:string ;
      rdfs:subPropertyOf <https://schema.org/encodingFormat> .

<https://schema.org/encodingFormat>
      a       owl:DatatypeProperty ;
      rdfs:isDefinedBy <https://schema.org/> .

:hasRegion
      a       owl:DatatypeProperty ;
      rdfs:comment "The region (e.g. state or province) associated with the address of the object"@en ;
      rdfs:domain :Address ;
      rdfs:label "has region"@en ;
      rdfs:range xsd:string ;
      rdfs:subPropertyOf <http://www.w3.org/2006/vcard/ns#region> .

:alcoholUseDisorder_Current
      a       owl:DatatypeProperty ;
      rdfs:comment "Describes the subject's current alcohol use disorder (ie: dependence, abuse, none)." ;
      rdfs:domain :Covariates ;
      rdfs:label "alcohol use disorder current" ;
      rdfs:range xsd:boolean ;
      rdfs:subPropertyOf :useDisorderProperty .

<https://schema.org/distribution>
      a       owl:ObjectProperty ;
      rdfs:isDefinedBy <https://schema.org/> .

:hasAge_Mean
      a       owl:DatatypeProperty ;
      rdfs:comment "Describes the mean age of the cohort"@en ;
      rdfs:domain
              [ a       owl:Class ;
                owl:unionOf (:CohortGroup :CohortProject)
              ] ;
      rdfs:label "has mean age"@en ;
      rdfs:range xsd:double ;
      <http://purl.org/vocab/vann/example>
              "Cohort1 hasAge_Mean 21.0"@en .

:Cancer
      a       owl:Class ;
      rdfs:comment "A disease characterized by abnormal cell division and growth"@en ;
      rdfs:label "Cancer"@en ;
      rdfs:subClassOf :Disorder ;
      <http://purl.org/vocab/vann/example>
              "CNS Cancer"@en .

:hasAge_Minimum
      a       owl:DatatypeProperty ;
      rdfs:comment "Describes inclusion criteria for minimum age of participants in a Cohort, CohortProject or CohortGroup"@en ;
      rdfs:domain
              [ a       owl:Class ;
                owl:unionOf (:Cohort :CohortGroup :CohortProject)
              ] ;
      rdfs:label "has minimum age"@en ;
      rdfs:range xsd:positiveInteger ;
      <http://purl.org/vocab/vann/example>
              "CohortGroup1 hasAge_Minimum 12"@en .

:hasDiagnosticInstrument
      a       owl:ObjectProperty ;
      rdfs:comment "Describes what instrument is used to diagnose the members of the cohort"@en ;
      rdfs:domain
              [ a       owl:Class ;
                owl:unionOf (:CohortGroup :CohortProject)
              ] ;
      rdfs:label "has diagnostic instrument"@en ;
      rdfs:range :DiagnosticInstrument ;
      <http://purl.org/vocab/vann/example>
              "Cohort1 hasDiagnosticInstrument miniInternationalNeuropychiatricInterview --> The members of Cohort1 are diagnosed with Mini International Neuropychiatric Interview"@en .

:hasDate_TargetEnd
      a       owl:DatatypeProperty ;
      rdfs:comment "Describes the end date of the target period of the project"@en ;
      rdfs:domain :Project ;
      rdfs:label "has target end date"@en ;
      rdfs:range xsd:date ;
      <http://purl.org/vocab/vann/example>
              "BipolarProject hasDate_TargetEnd 2020-03-12"@en .

:Occupation
      a       owl:DatatypeProperty ;
      rdfs:comment "Property which states whether subject's occupation is specified." ;
      rdfs:domain :Covariates ;
      rdfs:label "occupation" ;
      rdfs:range xsd:boolean ;
      rdfs:subPropertyOf :demographicProperty .

:hasDistribution
      a       owl:ObjectProperty ;
      rdfs:comment "Indicates a downloadable form of a dataset at a specific location"^^xsd:string ;
      rdfs:domain :Dataset ;
      rdfs:label "has distribution"^^xsd:string ;
      rdfs:range :DataDownload ;
      rdfs:subPropertyOf <https://schema.org/distribution> .

:hasPrimaryAddress
      a       owl:ObjectProperty ;
      rdfs:comment "Describes the primary address of an organization or person"@en ;
      rdfs:domain
              [ a       owl:Class ;
                owl:unionOf (:Organization :Person)
              ] ;
      rdfs:label "has primary address"@en ;
      rdfs:range :Address ;
      rdfs:subPropertyOf <http://www.w3.org/2006/vcard/ns#hasAddress> ;
      <http://purl.org/vocab/vann/example>
              "USC hasPrimaryAddress \"123 Admiralty Way\""@en .

:otherSubstanceUseDisorder_AgeofOnset
      a       owl:DatatypeProperty ;
      rdfs:comment "Describes whether age of onset of subject's substance use disorder is specified." ;
      rdfs:domain :Covariates ;
      rdfs:label "other substance use disorder age of onset" ;
      rdfs:range xsd:boolean ;
      rdfs:subPropertyOf :useDisorderProperty .

<http://purl.org/dc/terms/creator>
      a       owl:AnnotationProperty , owl:ObjectProperty ;
      rdfs:isDefinedBy <http://purl.org/dc/terms/creator> .

:GAD_Lifetime
      a       owl:DatatypeProperty ;
      rdfs:comment "Describes whether if the subject had Generalized Anxiety Disorder during their lifetime is specified." ;
      rdfs:domain :Covariates ;
      rdfs:label "GAD lifetime" ;
      rdfs:range xsd:boolean ;
      rdfs:subPropertyOf :psychopathologicalProperty .

:isPartOfCohortProject
      a       owl:ObjectProperty ;
      rdfs:comment "Property that indicates the cohort groups which are part of a cohort project"@en ;
      rdfs:domain :CohortGroup ;
      rdfs:label "is part of cohort project"@en ;
      rdfs:range :CohortProject .

:otherMedUse_Lifetime
      a       owl:DatatypeProperty ;
      rdfs:comment "Describes the subject's other medication use during their lifetime." ;
      rdfs:domain :Covariates ;
      rdfs:label "other medication use lifetime" ;
      rdfs:range xsd:string ;
      rdfs:subPropertyOf :medicationSomaticProperty .
